<?xml version="1.0"?>
<rdf:RDF xmlns="http://www.semanticweb.org/2021/ontologies/calcio#"
     xml:base="http://www.semanticweb.org/2021/ontologies/calcio"
     xmlns:dc="http://purl.org/dc/elements/1.1/"
     xmlns:c21="http://www.semanticweb.org/2021/ontologies/calcio#"
     xmlns:dbr="http://dbpedia.org/resource/"
     xmlns:owl="http://www.w3.org/2002/07/owl#"
     xmlns:rdf="http://www.w3.org/1999/02/22-rdf-syntax-ns#"
     xmlns:xml="http://www.w3.org/XML/1998/namespace"
     xmlns:xsd="http://www.w3.org/2001/XMLSchema#"
     xmlns:foaf="http://xmlns.com/foaf/0.1/"
     xmlns:rdfs="http://www.w3.org/2000/01/rdf-schema#"
     xmlns:swrl="http://www.w3.org/2003/11/swrl#"
     xmlns:vann="http://purl.org/vocab/vann/"
     xmlns:swrla="http://swrl.stanford.edu/ontologies/3.3/swrla.owl#"
     xmlns:swrlb="http://www.w3.org/2003/11/swrlb#"
     xmlns:schema="http://schema.org/"
     xmlns:wikidata="https://www.wikidata.org/wiki/">
    <owl:Ontology rdf:about="http://www.semanticweb.org/2021/ontologies/calcio">
        <dc:creator rdf:datatype="http://www.w3.org/2001/XMLSchema#string">Giulio Piazza</dc:creator>
        <dc:creator rdf:datatype="http://www.w3.org/2001/XMLSchema#string">Walter Maltese</dc:creator>
        <dc:date>2021-01-26</dc:date>
        <dc:description xml:lang="it">L&apos;ontologia &quot;Calcio 2021&quot; è un&apos;ontologia dedicata alla descrizione delle componenti principali dell&apos;omonimo sport, descrivendone relazioni e proprietà fra gli individui di riferimento.</dc:description>
        <dc:title xml:lang="it">Calcio 2021</dc:title>
        <vann:preferredNamespacePrefix>c21</vann:preferredNamespacePrefix>
        <vann:preferredNamespaceUri>http://www.semanticweb.org/2021/ontologies/calcio#</vann:preferredNamespaceUri>
        <rdfs:comment xml:lang="it">Ontologia dedicata alle squadre, tornei di club e nazione, e altri membri dello sport del Calcio</rdfs:comment>
        <rdfs:label xml:lang="it">Calcio</rdfs:label>
    </owl:Ontology>
    


    <!-- 
    ///////////////////////////////////////////////////////////////////////////////////////
    //
    // Annotation properties
    //
    ///////////////////////////////////////////////////////////////////////////////////////
     -->

    


    <!-- http://purl.org/dc/elements/1.1/creator -->

    <owl:AnnotationProperty rdf:about="http://purl.org/dc/elements/1.1/creator"/>
    


    <!-- http://purl.org/dc/elements/1.1/date -->

    <owl:AnnotationProperty rdf:about="http://purl.org/dc/elements/1.1/date"/>
    


    <!-- http://purl.org/dc/elements/1.1/description -->

    <owl:AnnotationProperty rdf:about="http://purl.org/dc/elements/1.1/description"/>
    


    <!-- http://purl.org/dc/elements/1.1/title -->

    <owl:AnnotationProperty rdf:about="http://purl.org/dc/elements/1.1/title"/>
    


    <!-- http://purl.org/vocab/vann/preferredNamespacePrefix -->

    <owl:AnnotationProperty rdf:about="http://purl.org/vocab/vann/preferredNamespacePrefix"/>
    


    <!-- http://purl.org/vocab/vann/preferredNamespaceUri -->

    <owl:AnnotationProperty rdf:about="http://purl.org/vocab/vann/preferredNamespaceUri"/>
    


    <!-- http://swrl.stanford.edu/ontologies/3.3/swrla.owl#isRuleEnabled -->

    <owl:AnnotationProperty rdf:about="http://swrl.stanford.edu/ontologies/3.3/swrla.owl#isRuleEnabled"/>
    


    <!-- 
    ///////////////////////////////////////////////////////////////////////////////////////
    //
    // Object Properties
    //
    ///////////////////////////////////////////////////////////////////////////////////////
     -->

    


    <!-- http://www.semanticweb.org/2021/ontologies/calcio#allenaSquadra -->

    <owl:ObjectProperty rdf:about="http://www.semanticweb.org/2021/ontologies/calcio#allenaSquadra">
        <owl:inverseOf rdf:resource="http://www.semanticweb.org/2021/ontologies/calcio#èAllenataDa"/>
        <rdf:type rdf:resource="http://www.w3.org/2002/07/owl#FunctionalProperty"/>
        <rdfs:domain rdf:resource="http://xmlns.com/foaf/0.1/Person"/>
        <rdfs:range rdf:resource="http://www.semanticweb.org/2021/ontologies/calcio#Squadra"/>
        <rdfs:comment xml:lang="en">Person who coach a football team.</rdfs:comment>
        <rdfs:comment xml:lang="it">Persona che allena una squadra di calcio.</rdfs:comment>
        <rdfs:label xml:lang="it">allenaSquadra</rdfs:label>
        <rdfs:label xml:lang="en">coachTeam</rdfs:label>
    </owl:ObjectProperty>
    


    <!-- http://www.semanticweb.org/2021/ontologies/calcio#allenaSquadraDiClub -->

    <owl:ObjectProperty rdf:about="http://www.semanticweb.org/2021/ontologies/calcio#allenaSquadraDiClub">
        <rdfs:subPropertyOf rdf:resource="http://www.semanticweb.org/2021/ontologies/calcio#allenaSquadra"/>
        <rdf:type rdf:resource="http://www.w3.org/2002/07/owl#FunctionalProperty"/>
        <rdfs:domain rdf:resource="http://www.semanticweb.org/2021/ontologies/calcio#allenatoreDiClub"/>
        <rdfs:range rdf:resource="http://www.semanticweb.org/2021/ontologies/calcio#squadraDiClub"/>
        <owl:propertyDisjointWith rdf:resource="http://www.semanticweb.org/2021/ontologies/calcio#allenaSquadraNazionale"/>
        <rdfs:comment xml:lang="en">Person who coach a Club team.</rdfs:comment>
        <rdfs:comment xml:lang="it">Persona che allena una squadra di Club.</rdfs:comment>
        <rdfs:label xml:lang="it">allenaSquadraDiClub</rdfs:label>
        <rdfs:label xml:lang="en">coachClubTeam</rdfs:label>
    </owl:ObjectProperty>
    


    <!-- http://www.semanticweb.org/2021/ontologies/calcio#allenaSquadraNazionale -->

    <owl:ObjectProperty rdf:about="http://www.semanticweb.org/2021/ontologies/calcio#allenaSquadraNazionale">
        <rdfs:subPropertyOf rdf:resource="http://www.semanticweb.org/2021/ontologies/calcio#allenaSquadra"/>
        <rdf:type rdf:resource="http://www.w3.org/2002/07/owl#FunctionalProperty"/>
        <rdfs:domain rdf:resource="http://www.semanticweb.org/2021/ontologies/calcio#allenatoreDiNazionale"/>
        <rdfs:range rdf:resource="http://www.semanticweb.org/2021/ontologies/calcio#squadraNazionale"/>
        <rdfs:comment xml:lang="en">Person who coach a National team.</rdfs:comment>
        <rdfs:comment xml:lang="it">Persona che allena una squadra Nazionale.</rdfs:comment>
        <rdfs:label xml:lang="it">allenaSquadraNazionale</rdfs:label>
        <rdfs:label xml:lang="en">coachNationalTeam</rdfs:label>
    </owl:ObjectProperty>
    


    <!-- http://www.semanticweb.org/2021/ontologies/calcio#allenatoDa -->

    <owl:ObjectProperty rdf:about="http://www.semanticweb.org/2021/ontologies/calcio#allenatoDa">
        <rdfs:domain rdf:resource="http://www.semanticweb.org/2021/ontologies/calcio#Calciatore"/>
        <rdfs:range rdf:resource="http://www.semanticweb.org/2021/ontologies/calcio#Allenatore"/>
        <owl:propertyChainAxiom rdf:parseType="Collection">
            <rdf:Description rdf:about="http://www.semanticweb.org/2021/ontologies/calcio#giocaPer"/>
            <rdf:Description rdf:about="http://www.semanticweb.org/2021/ontologies/calcio#èAllenataDa"/>
        </owl:propertyChainAxiom>
        <rdfs:comment xml:lang="it">Calaciatore allenato da uno specifico allenatore.</rdfs:comment>
        <rdfs:comment xml:lang="en">Calaciatore trained by a specific coach.</rdfs:comment>
        <rdfs:label xml:lang="it">allenatoDa</rdfs:label>
        <rdfs:label xml:lang="en">coachedBy</rdfs:label>
    </owl:ObjectProperty>
    


    <!-- http://www.semanticweb.org/2021/ontologies/calcio#appartieneALega -->

    <owl:ObjectProperty rdf:about="http://www.semanticweb.org/2021/ontologies/calcio#appartieneALega">
        <owl:inverseOf rdf:resource="http://www.semanticweb.org/2021/ontologies/calcio#contieneSquadra"/>
        <rdf:type rdf:resource="http://www.w3.org/2002/07/owl#FunctionalProperty"/>
        <rdfs:domain rdf:resource="http://www.semanticweb.org/2021/ontologies/calcio#squadraDiClub"/>
        <rdfs:range rdf:resource="http://www.semanticweb.org/2021/ontologies/calcio#Lega"/>
        <rdfs:comment xml:lang="en">Club team competing in a league.</rdfs:comment>
        <rdfs:comment xml:lang="it">Squadra di club che compete in una lega.</rdfs:comment>
        <rdfs:label xml:lang="it">appartieneALega</rdfs:label>
        <rdfs:label xml:lang="en">belongsToLeague</rdfs:label>
    </owl:ObjectProperty>
    


    <!-- http://www.semanticweb.org/2021/ontologies/calcio#arbitraIn -->

    <owl:ObjectProperty rdf:about="http://www.semanticweb.org/2021/ontologies/calcio#arbitraIn">
        <rdf:type rdf:resource="http://www.w3.org/2002/07/owl#FunctionalProperty"/>
        <rdfs:domain rdf:resource="http://xmlns.com/foaf/0.1/Person"/>
        <rdfs:range rdf:resource="http://www.semanticweb.org/2021/ontologies/calcio#Lega"/>
        <rdfs:comment xml:lang="en">Person who referees in a league.</rdfs:comment>
        <rdfs:comment xml:lang="it">Persona che arbitra in una lega.</rdfs:comment>
        <rdfs:label xml:lang="it">arbitraIn</rdfs:label>
        <rdfs:label xml:lang="en">refereesIn</rdfs:label>
    </owl:ObjectProperty>
    


    <!-- http://www.semanticweb.org/2021/ontologies/calcio#calciatoreGiocaInStadio -->

    <owl:ObjectProperty rdf:about="http://www.semanticweb.org/2021/ontologies/calcio#calciatoreGiocaInStadio">
        <rdfs:domain rdf:resource="http://www.semanticweb.org/2021/ontologies/calcio#Calciatore"/>
        <rdfs:range rdf:resource="http://www.semanticweb.org/2021/ontologies/calcio#Stadio"/>
        <owl:propertyChainAxiom rdf:parseType="Collection">
            <rdf:Description rdf:about="http://www.semanticweb.org/2021/ontologies/calcio#giocaPer"/>
            <rdf:Description rdf:about="http://www.semanticweb.org/2021/ontologies/calcio#giocaInStadio"/>
        </owl:propertyChainAxiom>
        <rdfs:comment xml:lang="en">Relationship between footballer and his team&apos;s home stadium.</rdfs:comment>
        <rdfs:comment xml:lang="it">Relazione tra calciatore e lo stadio di Casa della sua squadra.</rdfs:comment>
        <rdfs:label xml:lang="en">SoccerPlayerPlaysInStadium</rdfs:label>
        <rdfs:label xml:lang="it">calciatoreGiocaInStadio</rdfs:label>
    </owl:ObjectProperty>
    


    <!-- http://www.semanticweb.org/2021/ontologies/calcio#collegaDi -->

    <owl:ObjectProperty rdf:about="http://www.semanticweb.org/2021/ontologies/calcio#collegaDi">
        <rdfs:subPropertyOf rdf:resource="http://xmlns.com/foaf/0.1/knows"/>
        <rdf:type rdf:resource="http://www.w3.org/2002/07/owl#SymmetricProperty"/>
        <rdf:type rdf:resource="http://www.w3.org/2002/07/owl#TransitiveProperty"/>
        <rdfs:domain rdf:resource="http://xmlns.com/foaf/0.1/Person"/>
        <rdfs:range rdf:resource="http://xmlns.com/foaf/0.1/Person"/>
        <rdfs:comment xml:lang="it">la persona che è collega di un&apos;altra persona</rdfs:comment>
        <rdfs:comment xml:lang="en">the person who is a colleague of another person</rdfs:comment>
        <rdfs:label xml:lang="en">colleagueOf</rdfs:label>
        <rdfs:label xml:lang="it">collegaDi</rdfs:label>
    </owl:ObjectProperty>
    


    <!-- http://www.semanticweb.org/2021/ontologies/calcio#compagnoDi -->

    <owl:ObjectProperty rdf:about="http://www.semanticweb.org/2021/ontologies/calcio#compagnoDi">
        <rdfs:subPropertyOf rdf:resource="http://xmlns.com/foaf/0.1/knows"/>
        <rdf:type rdf:resource="http://www.w3.org/2002/07/owl#SymmetricProperty"/>
        <rdf:type rdf:resource="http://www.w3.org/2002/07/owl#TransitiveProperty"/>
        <rdfs:domain rdf:resource="http://www.semanticweb.org/2021/ontologies/calcio#Calciatore"/>
        <rdfs:range rdf:resource="http://www.semanticweb.org/2021/ontologies/calcio#Calciatore"/>
        <rdfs:comment xml:lang="it">il Calciatore che è compgano di un altro Calciatore.</rdfs:comment>
        <rdfs:comment xml:lang="en">the player who is a partner of another player.</rdfs:comment>
        <rdfs:label xml:lang="it">compagnoDi</rdfs:label>
        <rdfs:label xml:lang="en">teammatesOf</rdfs:label>
    </owl:ObjectProperty>
    


    <!-- http://www.semanticweb.org/2021/ontologies/calcio#contieneSquadra -->

    <owl:ObjectProperty rdf:about="http://www.semanticweb.org/2021/ontologies/calcio#contieneSquadra">
        <rdfs:domain rdf:resource="http://www.semanticweb.org/2021/ontologies/calcio#Lega"/>
        <rdfs:range rdf:resource="http://www.semanticweb.org/2021/ontologies/calcio#squadraDiClub"/>
        <rdfs:comment xml:lang="en">Relationship between a league and a participating team.</rdfs:comment>
        <rdfs:comment xml:lang="it">Relazione fra una lega e una squadra partecipante.</rdfs:comment>
        <rdfs:label xml:lang="it">contieneSquadra</rdfs:label>
        <rdfs:label xml:lang="en">hasTeam</rdfs:label>
    </owl:ObjectProperty>
    


    <!-- http://www.semanticweb.org/2021/ontologies/calcio#detieneCalciatore -->

    <owl:ObjectProperty rdf:about="http://www.semanticweb.org/2021/ontologies/calcio#detieneCalciatore">
        <owl:inverseOf rdf:resource="http://www.semanticweb.org/2021/ontologies/calcio#giocaPer"/>
        <rdfs:domain rdf:resource="http://www.semanticweb.org/2021/ontologies/calcio#Squadra"/>
        <rdfs:range rdf:resource="http://www.semanticweb.org/2021/ontologies/calcio#Calciatore"/>
        <rdfs:comment xml:lang="it">Squadra che &quot;possiede&quot; un determinato calciatore.</rdfs:comment>
        <rdfs:comment xml:lang="en">Team that &quot;owns&quot; a particular soccer player.</rdfs:comment>
        <rdfs:label xml:lang="it">detieneCalciatore</rdfs:label>
        <rdfs:label xml:lang="en">hasSoccerPlayer</rdfs:label>
    </owl:ObjectProperty>
    


    <!-- http://www.semanticweb.org/2021/ontologies/calcio#giocaInLega -->

    <owl:ObjectProperty rdf:about="http://www.semanticweb.org/2021/ontologies/calcio#giocaInLega">
        <rdfs:domain rdf:resource="http://www.semanticweb.org/2021/ontologies/calcio#Calciatore"/>
        <rdfs:range rdf:resource="http://www.semanticweb.org/2021/ontologies/calcio#Lega"/>
        <owl:propertyChainAxiom rdf:parseType="Collection">
            <rdf:Description rdf:about="http://www.semanticweb.org/2021/ontologies/calcio#giocaPer"/>
            <rdf:Description rdf:about="http://www.semanticweb.org/2021/ontologies/calcio#appartieneALega"/>
        </owl:propertyChainAxiom>
        <rdfs:comment xml:lang="it">Il Calciatore che gioca in una determinata lega.</rdfs:comment>
        <rdfs:comment xml:lang="en">The player who plays in a particular league.</rdfs:comment>
        <rdfs:label xml:lang="it">giocaInLega</rdfs:label>
        <rdfs:label xml:lang="en">playsInLeague</rdfs:label>
    </owl:ObjectProperty>
    


    <!-- http://www.semanticweb.org/2021/ontologies/calcio#giocaInStadio -->

    <owl:ObjectProperty rdf:about="http://www.semanticweb.org/2021/ontologies/calcio#giocaInStadio">
        <owl:inverseOf rdf:resource="http://www.semanticweb.org/2021/ontologies/calcio#ospitaSquadra"/>
        <rdf:type rdf:resource="http://www.w3.org/2002/07/owl#FunctionalProperty"/>
        <rdfs:domain rdf:resource="http://www.semanticweb.org/2021/ontologies/calcio#Squadra"/>
        <rdfs:range rdf:resource="http://www.semanticweb.org/2021/ontologies/calcio#Stadio"/>
        <rdfs:comment xml:lang="en">Relationship between team and home stadium.</rdfs:comment>
        <rdfs:comment xml:lang="it">Relazione tra squadra e lo stadio di casa.</rdfs:comment>
        <rdfs:label xml:lang="it">giocaInStadio</rdfs:label>
        <rdfs:label xml:lang="en">playsInStadium</rdfs:label>
    </owl:ObjectProperty>
    


    <!-- http://www.semanticweb.org/2021/ontologies/calcio#giocaPer -->

    <owl:ObjectProperty rdf:about="http://www.semanticweb.org/2021/ontologies/calcio#giocaPer">
        <rdfs:domain rdf:resource="http://www.semanticweb.org/2021/ontologies/calcio#Calciatore"/>
        <rdfs:range rdf:resource="http://www.semanticweb.org/2021/ontologies/calcio#Squadra"/>
        <rdfs:comment xml:lang="it">Il calciatore che gioca in una determinata squadra.</rdfs:comment>
        <rdfs:comment xml:lang="en">The footballer who plays for a particular team.</rdfs:comment>
        <rdfs:label xml:lang="it">giocaPer</rdfs:label>
        <rdfs:label xml:lang="en">playsFor</rdfs:label>
    </owl:ObjectProperty>
    


    <!-- http://www.semanticweb.org/2021/ontologies/calcio#haRuolo -->

    <owl:ObjectProperty rdf:about="http://www.semanticweb.org/2021/ontologies/calcio#haRuolo">
        <owl:inverseOf rdf:resource="http://www.semanticweb.org/2021/ontologies/calcio#èRuoloDi"/>
        <rdfs:domain rdf:resource="http://www.semanticweb.org/2021/ontologies/calcio#Calciatore"/>
        <rdfs:range rdf:resource="http://www.semanticweb.org/2021/ontologies/calcio#RuoloCalciatore"/>
        <rdfs:comment xml:lang="en">Role of a footballer.</rdfs:comment>
        <rdfs:comment xml:lang="it">Ruolo di un calciatore.</rdfs:comment>
        <rdfs:label xml:lang="it">haRuolo</rdfs:label>
        <rdfs:label xml:lang="en">hasRole</rdfs:label>
    </owl:ObjectProperty>
    


    <!-- http://www.semanticweb.org/2021/ontologies/calcio#haRuoloInSquadra -->

    <owl:ObjectProperty rdf:about="http://www.semanticweb.org/2021/ontologies/calcio#haRuoloInSquadra">
        <rdfs:domain rdf:resource="http://www.semanticweb.org/2021/ontologies/calcio#Calciatore"/>
        <rdfs:range rdf:resource="http://www.semanticweb.org/2021/ontologies/calcio#Squadra"/>
        <owl:propertyChainAxiom rdf:parseType="Collection">
            <rdf:Description rdf:about="http://www.semanticweb.org/2021/ontologies/calcio#haRuolo"/>
            <rdf:Description rdf:about="http://www.semanticweb.org/2021/ontologies/calcio#ruoloInSquadra"/>
        </owl:propertyChainAxiom>
        <rdfs:comment xml:lang="en">Role of a footballer in his team.</rdfs:comment>
        <rdfs:comment xml:lang="it">Ruolo di un calciatore nella sua squadra.</rdfs:comment>
        <rdfs:label xml:lang="it">haRuoloInSquadra</rdfs:label>
        <rdfs:label xml:lang="en">hasRoleInTeam</rdfs:label>
    </owl:ObjectProperty>
    


    <!-- http://www.semanticweb.org/2021/ontologies/calcio#haVinto -->

    <owl:ObjectProperty rdf:about="http://www.semanticweb.org/2021/ontologies/calcio#haVinto">
        <owl:inverseOf rdf:resource="http://www.semanticweb.org/2021/ontologies/calcio#vintoDa"/>
        <rdfs:domain rdf:resource="http://www.semanticweb.org/2021/ontologies/calcio#Squadra"/>
        <rdfs:range rdf:resource="http://www.semanticweb.org/2021/ontologies/calcio#Trofeo"/>
        <rdfs:comment xml:lang="en">Relationship between team and a given trophy.</rdfs:comment>
        <rdfs:comment xml:lang="it">Relazione tra squadra e un determinato trofeo.</rdfs:comment>
        <rdfs:label xml:lang="en">Won</rdfs:label>
        <rdfs:label xml:lang="it">haVinto</rdfs:label>
    </owl:ObjectProperty>
    


    <!-- http://www.semanticweb.org/2021/ontologies/calcio#haVintoClub -->

    <owl:ObjectProperty rdf:about="http://www.semanticweb.org/2021/ontologies/calcio#haVintoClub">
        <rdfs:subPropertyOf rdf:resource="http://www.semanticweb.org/2021/ontologies/calcio#haVinto"/>
        <owl:inverseOf rdf:resource="http://www.semanticweb.org/2021/ontologies/calcio#vintoDaClub"/>
        <rdfs:domain rdf:resource="http://www.semanticweb.org/2021/ontologies/calcio#squadraDiClub"/>
        <rdfs:range rdf:resource="http://www.semanticweb.org/2021/ontologies/calcio#trofeoDiClub"/>
        <owl:propertyDisjointWith rdf:resource="http://www.semanticweb.org/2021/ontologies/calcio#haVintoNazionale"/>
        <rdfs:comment xml:lang="en">Relationship between a Club team and a given trophy.</rdfs:comment>
        <rdfs:comment xml:lang="it">Relazione tra squadra di club e un determinato trofeo.</rdfs:comment>
        <rdfs:label xml:lang="it">haVintoClub</rdfs:label>
        <rdfs:label xml:lang="en">wonClub</rdfs:label>
    </owl:ObjectProperty>
    


    <!-- http://www.semanticweb.org/2021/ontologies/calcio#haVintoNazionale -->

    <owl:ObjectProperty rdf:about="http://www.semanticweb.org/2021/ontologies/calcio#haVintoNazionale">
        <rdfs:subPropertyOf rdf:resource="http://www.semanticweb.org/2021/ontologies/calcio#haVinto"/>
        <owl:inverseOf rdf:resource="http://www.semanticweb.org/2021/ontologies/calcio#vintoDaNazionale"/>
        <rdfs:domain rdf:resource="http://www.semanticweb.org/2021/ontologies/calcio#squadraNazionale"/>
        <rdfs:range rdf:resource="http://www.semanticweb.org/2021/ontologies/calcio#trofeoDiNazione"/>
        <rdfs:comment xml:lang="en">Relationship between a national team and a given trophy.</rdfs:comment>
        <rdfs:comment xml:lang="it">Relazione tra squadra nazionale e un determinato trofeo.</rdfs:comment>
        <rdfs:label xml:lang="it">haVintoNazionale</rdfs:label>
        <rdfs:label xml:lang="en">wonNational</rdfs:label>
    </owl:ObjectProperty>
    


    <!-- http://www.semanticweb.org/2021/ontologies/calcio#lavoraPer -->

    <owl:ObjectProperty rdf:about="http://www.semanticweb.org/2021/ontologies/calcio#lavoraPer">
        <rdf:type rdf:resource="http://www.w3.org/2002/07/owl#FunctionalProperty"/>
        <rdfs:domain rdf:resource="http://xmlns.com/foaf/0.1/Person"/>
        <rdfs:range rdf:resource="http://www.semanticweb.org/2021/ontologies/calcio#Squadra"/>
        <rdfs:comment xml:lang="en">Person who works for a football team</rdfs:comment>
        <rdfs:comment xml:lang="it">Persona che lavora per una squadra di calcio</rdfs:comment>
        <rdfs:label xml:lang="it">lavoraPer</rdfs:label>
        <rdfs:label xml:lang="en">worksFor</rdfs:label>
    </owl:ObjectProperty>
    


    <!-- http://www.semanticweb.org/2021/ontologies/calcio#ospitaSquadra -->

    <owl:ObjectProperty rdf:about="http://www.semanticweb.org/2021/ontologies/calcio#ospitaSquadra">
        <rdfs:domain rdf:resource="http://www.semanticweb.org/2021/ontologies/calcio#Stadio"/>
        <rdfs:range rdf:resource="http://www.semanticweb.org/2021/ontologies/calcio#Squadra"/>
        <rdfs:comment xml:lang="en">Relationship between home stadium and its team.</rdfs:comment>
        <rdfs:comment xml:lang="it">Relazione tra stadio di casa e la sua squadra.</rdfs:comment>
        <rdfs:label xml:lang="en">hostsTeam</rdfs:label>
        <rdfs:label xml:lang="it">ospitaSquadra</rdfs:label>
    </owl:ObjectProperty>
    


    <!-- http://www.semanticweb.org/2021/ontologies/calcio#ruoloInSquadra -->

    <owl:ObjectProperty rdf:about="http://www.semanticweb.org/2021/ontologies/calcio#ruoloInSquadra">
        <rdfs:domain rdf:resource="http://www.semanticweb.org/2021/ontologies/calcio#RuoloCalciatore"/>
        <rdfs:range rdf:resource="http://www.semanticweb.org/2021/ontologies/calcio#Squadra"/>
        <rdfs:comment xml:lang="it">il ruolo che assume un giocatore in una squadra di calcio.</rdfs:comment>
        <rdfs:comment xml:lang="en">the role a player takes on a football team.</rdfs:comment>
        <rdfs:label xml:lang="en">roleInTeam</rdfs:label>
        <rdfs:label xml:lang="it">ruoloInSquadra</rdfs:label>
    </owl:ObjectProperty>
    


    <!-- http://www.semanticweb.org/2021/ontologies/calcio#vintoDa -->

    <owl:ObjectProperty rdf:about="http://www.semanticweb.org/2021/ontologies/calcio#vintoDa">
        <rdf:type rdf:resource="http://www.w3.org/2002/07/owl#FunctionalProperty"/>
        <rdfs:domain rdf:resource="http://www.semanticweb.org/2021/ontologies/calcio#Trofeo"/>
        <rdfs:range rdf:resource="http://www.semanticweb.org/2021/ontologies/calcio#Squadra"/>
        <rdfs:comment xml:lang="en">Relationship between the trophy and the team that won it.</rdfs:comment>
        <rdfs:comment xml:lang="it">Relazione tra trofeo e la squadra che l&apos;ha vinto.</rdfs:comment>
        <rdfs:label xml:lang="it">vintoDa</rdfs:label>
        <rdfs:label xml:lang="en">wonBy</rdfs:label>
    </owl:ObjectProperty>
    


    <!-- http://www.semanticweb.org/2021/ontologies/calcio#vintoDaClub -->

    <owl:ObjectProperty rdf:about="http://www.semanticweb.org/2021/ontologies/calcio#vintoDaClub">
        <rdfs:subPropertyOf rdf:resource="http://www.semanticweb.org/2021/ontologies/calcio#vintoDa"/>
        <rdf:type rdf:resource="http://www.w3.org/2002/07/owl#FunctionalProperty"/>
        <rdfs:domain rdf:resource="http://www.semanticweb.org/2021/ontologies/calcio#trofeoDiClub"/>
        <rdfs:range rdf:resource="http://www.semanticweb.org/2021/ontologies/calcio#squadraDiClub"/>
        <owl:propertyDisjointWith rdf:resource="http://www.semanticweb.org/2021/ontologies/calcio#vintoDaNazionale"/>
        <rdfs:comment xml:lang="en">Relationship between the trophy and the Club team that won it.</rdfs:comment>
        <rdfs:comment xml:lang="it">Relazione tra trofeo e la squadra di club che l&apos;ha vinto.</rdfs:comment>
        <rdfs:label xml:lang="it">vintoDaClub</rdfs:label>
        <rdfs:label xml:lang="en">wonByClub</rdfs:label>
    </owl:ObjectProperty>
    


    <!-- http://www.semanticweb.org/2021/ontologies/calcio#vintoDaNazionale -->

    <owl:ObjectProperty rdf:about="http://www.semanticweb.org/2021/ontologies/calcio#vintoDaNazionale">
        <rdfs:subPropertyOf rdf:resource="http://www.semanticweb.org/2021/ontologies/calcio#vintoDa"/>
        <rdf:type rdf:resource="http://www.w3.org/2002/07/owl#FunctionalProperty"/>
        <rdfs:domain rdf:resource="http://www.semanticweb.org/2021/ontologies/calcio#trofeoDiNazione"/>
        <rdfs:range rdf:resource="http://www.semanticweb.org/2021/ontologies/calcio#squadraNazionale"/>
        <rdfs:comment xml:lang="en">Relationship between the trophy and the national team that won it.</rdfs:comment>
        <rdfs:comment xml:lang="it">Relazione tra trofeo e la squadra nazionale che l&apos;ha vinto.</rdfs:comment>
        <rdfs:label xml:lang="it">vintoDaNazionale</rdfs:label>
        <rdfs:label xml:lang="en">wonByNationalTeam</rdfs:label>
    </owl:ObjectProperty>
    


    <!-- http://www.semanticweb.org/2021/ontologies/calcio#èAllenataDa -->

    <owl:ObjectProperty rdf:about="http://www.semanticweb.org/2021/ontologies/calcio#èAllenataDa">
        <rdf:type rdf:resource="http://www.w3.org/2002/07/owl#FunctionalProperty"/>
        <rdfs:domain rdf:resource="http://www.semanticweb.org/2021/ontologies/calcio#Squadra"/>
        <rdfs:range rdf:resource="http://www.semanticweb.org/2021/ontologies/calcio#Allenatore"/>
        <rdfs:comment xml:lang="en">Relationship between team and its coach.</rdfs:comment>
        <rdfs:comment xml:lang="it">Relazione tra squadra e il suo allenatore.</rdfs:comment>
        <rdfs:label xml:lang="en">isCoachedBy</rdfs:label>
        <rdfs:label xml:lang="it">èAllenataDa</rdfs:label>
    </owl:ObjectProperty>
    


    <!-- http://www.semanticweb.org/2021/ontologies/calcio#èAllenataDaClub -->

    <owl:ObjectProperty rdf:about="http://www.semanticweb.org/2021/ontologies/calcio#èAllenataDaClub">
        <rdfs:subPropertyOf rdf:resource="http://www.semanticweb.org/2021/ontologies/calcio#èAllenataDa"/>
        <rdf:type rdf:resource="http://www.w3.org/2002/07/owl#FunctionalProperty"/>
        <rdfs:domain rdf:resource="http://www.semanticweb.org/2021/ontologies/calcio#squadraDiClub"/>
        <rdfs:range rdf:resource="http://www.semanticweb.org/2021/ontologies/calcio#allenatoreDiClub"/>
        <owl:propertyDisjointWith rdf:resource="http://www.semanticweb.org/2021/ontologies/calcio#èAllenataDaNazionale"/>
        <rdfs:comment xml:lang="en">Relationship between club team and its coach.</rdfs:comment>
        <rdfs:comment xml:lang="it">Relazione tra squadra di club e il suo allenatore.</rdfs:comment>
        <rdfs:label xml:lang="en">isCoachedByClub</rdfs:label>
        <rdfs:label xml:lang="it">èAllenataDaClub</rdfs:label>
    </owl:ObjectProperty>
    


    <!-- http://www.semanticweb.org/2021/ontologies/calcio#èAllenataDaNazionale -->

    <owl:ObjectProperty rdf:about="http://www.semanticweb.org/2021/ontologies/calcio#èAllenataDaNazionale">
        <rdfs:subPropertyOf rdf:resource="http://www.semanticweb.org/2021/ontologies/calcio#èAllenataDa"/>
        <rdf:type rdf:resource="http://www.w3.org/2002/07/owl#FunctionalProperty"/>
        <rdfs:domain rdf:resource="http://www.semanticweb.org/2021/ontologies/calcio#squadraNazionale"/>
        <rdfs:range rdf:resource="http://www.semanticweb.org/2021/ontologies/calcio#allenatoreDiNazionale"/>
        <rdfs:comment xml:lang="en">Relationship between national team and its coach.</rdfs:comment>
        <rdfs:comment xml:lang="it">Relazione tra squadra nazionale e il suo allenatore.</rdfs:comment>
        <rdfs:label xml:lang="en">isCoachedByNationalTeam</rdfs:label>
        <rdfs:label xml:lang="it">èAllenataDaNazionale</rdfs:label>
    </owl:ObjectProperty>
    


    <!-- http://www.semanticweb.org/2021/ontologies/calcio#èRuoloDi -->

    <owl:ObjectProperty rdf:about="http://www.semanticweb.org/2021/ontologies/calcio#èRuoloDi">
        <rdfs:domain rdf:resource="http://www.semanticweb.org/2021/ontologies/calcio#RuoloCalciatore"/>
        <rdfs:range rdf:resource="http://www.semanticweb.org/2021/ontologies/calcio#Calciatore"/>
        <rdfs:comment xml:lang="en">Relation between the role a player has in a team and the player himself.</rdfs:comment>
        <rdfs:comment xml:lang="it">Relazione tra il ruolo che un giocatore ha in una squadra e il calciatore stesso.</rdfs:comment>
        <rdfs:label xml:lang="en">isRoleOf</rdfs:label>
        <rdfs:label xml:lang="it">èRuoloDi</rdfs:label>
    </owl:ObjectProperty>
    


    <!-- http://xmlns.com/foaf/0.1/knows -->

    <owl:ObjectProperty rdf:about="http://xmlns.com/foaf/0.1/knows">
        <rdf:type rdf:resource="http://www.w3.org/2002/07/owl#SymmetricProperty"/>
    </owl:ObjectProperty>
    


    <!-- 
    ///////////////////////////////////////////////////////////////////////////////////////
    //
    // Data properties
    //
    ///////////////////////////////////////////////////////////////////////////////////////
     -->

    


    <!-- http://www.semanticweb.org/2021/ontologies/calcio#calciatoreHaValoreDiMercato -->

    <owl:DatatypeProperty rdf:about="http://www.semanticweb.org/2021/ontologies/calcio#calciatoreHaValoreDiMercato">
        <rdf:type rdf:resource="http://www.w3.org/2002/07/owl#FunctionalProperty"/>
        <rdfs:domain rdf:resource="http://www.semanticweb.org/2021/ontologies/calcio#Calciatore"/>
        <rdfs:range rdf:resource="http://www.w3.org/2001/XMLSchema#long"/>
        <rdfs:comment xml:lang="it">il valore di mercato attuale di un singolo giocatore.</rdfs:comment>
        <rdfs:comment xml:lang="en">the current market value of a single soccer player.</rdfs:comment>
        <rdfs:label xml:lang="it">calciatoreHaValoredDiMercato</rdfs:label>
        <rdfs:label xml:lang="en">soccerPlayerHasMarketValue</rdfs:label>
    </owl:DatatypeProperty>
    


    <!-- http://www.semanticweb.org/2021/ontologies/calcio#dataUltimoTrasferimento -->

    <owl:DatatypeProperty rdf:about="http://www.semanticweb.org/2021/ontologies/calcio#dataUltimoTrasferimento">
        <rdf:type rdf:resource="http://www.w3.org/2002/07/owl#FunctionalProperty"/>
        <rdfs:domain rdf:resource="http://www.semanticweb.org/2021/ontologies/calcio#Calciatore"/>
        <rdfs:range rdf:resource="http://www.w3.org/2001/XMLSchema#dateTime"/>
        <rdfs:comment xml:lang="it">la data in cui il giocatore è stato trasferito nel team attuale.</rdfs:comment>
        <rdfs:comment xml:lang="en">the date the player was transferred to the current team.</rdfs:comment>
        <rdfs:label xml:lang="it">dataUltimoTrasferimento</rdfs:label>
        <rdfs:label xml:lang="en">lastTransferDate</rdfs:label>
    </owl:DatatypeProperty>
    


    <!-- http://www.semanticweb.org/2021/ontologies/calcio#haCapienza -->

    <owl:DatatypeProperty rdf:about="http://www.semanticweb.org/2021/ontologies/calcio#haCapienza">
        <rdf:type rdf:resource="http://www.w3.org/2002/07/owl#FunctionalProperty"/>
        <rdfs:domain rdf:resource="http://www.semanticweb.org/2021/ontologies/calcio#Stadio"/>
        <rdfs:range rdf:resource="http://www.w3.org/2001/XMLSchema#int"/>
        <rdfs:comment xml:lang="it">la capienza di uno stadio di calcio.</rdfs:comment>
        <rdfs:comment xml:lang="en">the capacity of a football stadium.</rdfs:comment>
        <rdfs:label xml:lang="it">haCapienza</rdfs:label>
        <rdfs:label xml:lang="en">hasCapacity</rdfs:label>
    </owl:DatatypeProperty>
    


    <!-- http://www.semanticweb.org/2021/ontologies/calcio#haEtà -->

    <owl:DatatypeProperty rdf:about="http://www.semanticweb.org/2021/ontologies/calcio#haEtà">
        <rdf:type rdf:resource="http://www.w3.org/2002/07/owl#FunctionalProperty"/>
        <rdfs:domain rdf:resource="http://xmlns.com/foaf/0.1/Person"/>
        <rdfs:range rdf:resource="http://www.w3.org/2001/XMLSchema#int"/>
        <rdfs:comment xml:lang="it">l&apos;età attuale di una persona del mondo del calcio.</rdfs:comment>
        <rdfs:comment xml:lang="en">the current age of a person from the world of soccer.</rdfs:comment>
        <rdfs:label xml:lang="it">haEtà</rdfs:label>
        <rdfs:label xml:lang="en">hasAge</rdfs:label>
    </owl:DatatypeProperty>
    


    <!-- http://www.semanticweb.org/2021/ontologies/calcio#haEtàMedia -->

    <owl:DatatypeProperty rdf:about="http://www.semanticweb.org/2021/ontologies/calcio#haEtàMedia">
        <rdf:type rdf:resource="http://www.w3.org/2002/07/owl#FunctionalProperty"/>
        <rdfs:domain rdf:resource="http://www.semanticweb.org/2021/ontologies/calcio#Squadra"/>
        <rdfs:range rdf:resource="http://www.w3.org/2001/XMLSchema#float"/>
        <rdfs:comment xml:lang="it">l&apos;età media di una squadra di calcio calcolata a partire dall&apos;età dei singoli giocatori.</rdfs:comment>
        <rdfs:comment xml:lang="en">the average age of a football team calculated from the age of the individual players.</rdfs:comment>
        <rdfs:label xml:lang="it">haEtàMedia</rdfs:label>
        <rdfs:label xml:lang="en">hasAverageAge</rdfs:label>
    </owl:DatatypeProperty>
    


    <!-- http://www.semanticweb.org/2021/ontologies/calcio#haNazionalità -->

    <owl:DatatypeProperty rdf:about="http://www.semanticweb.org/2021/ontologies/calcio#haNazionalità">
        <rdfs:domain rdf:resource="http://xmlns.com/foaf/0.1/Person"/>
        <rdfs:range rdf:resource="http://www.w3.org/2001/XMLSchema#string"/>
        <rdfs:comment xml:lang="it">la Nazionalità di una persona del mondo del calcio.</rdfs:comment>
        <rdfs:comment xml:lang="en">the Nationality of a person from the world of soccer.</rdfs:comment>
        <rdfs:label xml:lang="it">haNazionalità</rdfs:label>
        <rdfs:label xml:lang="en">hasNationality</rdfs:label>
    </owl:DatatypeProperty>
    


    <!-- http://www.semanticweb.org/2021/ontologies/calcio#haNome -->

    <owl:DatatypeProperty rdf:about="http://www.semanticweb.org/2021/ontologies/calcio#haNome">
        <rdf:type rdf:resource="http://www.w3.org/2002/07/owl#FunctionalProperty"/>
        <rdfs:domain rdf:resource="http://xmlns.com/foaf/0.1/Person"/>
        <rdfs:range rdf:resource="http://www.w3.org/2001/XMLSchema#string"/>
        <rdfs:comment xml:lang="it">Il nome di una persona del mondo del calcio.</rdfs:comment>
        <rdfs:comment xml:lang="en">The name of a person from the world of soccer.</rdfs:comment>
        <rdfs:label xml:lang="it">haNome</rdfs:label>
        <rdfs:label xml:lang="en">hasName</rdfs:label>
    </owl:DatatypeProperty>
    


    <!-- http://www.semanticweb.org/2021/ontologies/calcio#haNumeroCalciatori -->

    <owl:DatatypeProperty rdf:about="http://www.semanticweb.org/2021/ontologies/calcio#haNumeroCalciatori">
        <rdf:type rdf:resource="http://www.w3.org/2002/07/owl#FunctionalProperty"/>
        <rdfs:domain rdf:resource="http://www.semanticweb.org/2021/ontologies/calcio#Squadra"/>
        <rdfs:range rdf:resource="http://www.w3.org/2001/XMLSchema#int"/>
        <rdfs:comment xml:lang="en">Number of players belonging to a soccer team.</rdfs:comment>
        <rdfs:comment xml:lang="it">Numero di giocatori appertenenti ad una squadra calcistica.</rdfs:comment>
        <rdfs:label xml:lang="it">haNumeroCalciatori</rdfs:label>
        <rdfs:label xml:lang="en">hasNumberOfSoccerPlayers</rdfs:label>
    </owl:DatatypeProperty>
    


    <!-- http://www.semanticweb.org/2021/ontologies/calcio#numeroSquadre -->

    <owl:DatatypeProperty rdf:about="http://www.semanticweb.org/2021/ontologies/calcio#numeroSquadre">
        <rdf:type rdf:resource="http://www.w3.org/2002/07/owl#FunctionalProperty"/>
        <rdfs:domain rdf:resource="http://www.semanticweb.org/2021/ontologies/calcio#Lega"/>
        <rdfs:range rdf:resource="http://www.w3.org/2001/XMLSchema#int"/>
        <rdfs:comment xml:lang="en">Number of teams that make up a league.</rdfs:comment>
        <rdfs:comment xml:lang="it">Numero di squadre che compongono una lega.</rdfs:comment>
        <rdfs:label xml:lang="en">numberOfTeams</rdfs:label>
        <rdfs:label xml:lang="it">numeroSquadre</rdfs:label>
    </owl:DatatypeProperty>
    


    <!-- http://www.semanticweb.org/2021/ontologies/calcio#numeroSquadreRetrocesse -->

    <owl:DatatypeProperty rdf:about="http://www.semanticweb.org/2021/ontologies/calcio#numeroSquadreRetrocesse">
        <rdf:type rdf:resource="http://www.w3.org/2002/07/owl#FunctionalProperty"/>
        <rdfs:domain rdf:resource="http://www.semanticweb.org/2021/ontologies/calcio#Lega"/>
        <rdfs:range rdf:resource="http://www.w3.org/2001/XMLSchema#int"/>
        <rdfs:comment xml:lang="en">Number of teams that will be relegated at the end of the season.</rdfs:comment>
        <rdfs:comment xml:lang="it">Numero di squadre che verranno retrocesse a fine stagione.</rdfs:comment>
        <rdfs:label xml:lang="en">numberOfRelegatedTeams</rdfs:label>
        <rdfs:label xml:lang="it">numeroSquadreRetrocesse</rdfs:label>
    </owl:DatatypeProperty>
    


    <!-- http://www.semanticweb.org/2021/ontologies/calcio#numeroSquadreTop -->

    <owl:DatatypeProperty rdf:about="http://www.semanticweb.org/2021/ontologies/calcio#numeroSquadreTop">
        <rdf:type rdf:resource="http://www.w3.org/2002/07/owl#FunctionalProperty"/>
        <rdfs:domain rdf:resource="http://www.semanticweb.org/2021/ontologies/calcio#Lega"/>
        <rdfs:range rdf:resource="http://www.w3.org/2001/XMLSchema#int"/>
        <rdfs:comment xml:lang="en">Number of teams that have finished in the top positions of the championship.</rdfs:comment>
        <rdfs:comment xml:lang="it">Numero di squadre che si sono classificate nelle prime posizioni del campionato.</rdfs:comment>
        <rdfs:label xml:lang="en">numberTeamsTop</rdfs:label>
        <rdfs:label xml:lang="it">numeroSquadreTop</rdfs:label>
    </owl:DatatypeProperty>
    


    <!-- http://www.semanticweb.org/2021/ontologies/calcio#rappresentaNazione -->

    <owl:DatatypeProperty rdf:about="http://www.semanticweb.org/2021/ontologies/calcio#rappresentaNazione">
        <rdf:type rdf:resource="http://www.w3.org/2002/07/owl#FunctionalProperty"/>
        <rdfs:domain rdf:resource="http://www.semanticweb.org/2021/ontologies/calcio#squadraNazionale"/>
        <rdfs:range rdf:resource="http://www.w3.org/2001/XMLSchema#string"/>
        <rdfs:comment xml:lang="it">La Nazione rappresentata dalla squadra di calcio nazionale.</rdfs:comment>
        <rdfs:comment xml:lang="en">The nation represented by the national football team.</rdfs:comment>
        <rdfs:label xml:lang="en">isCountry</rdfs:label>
        <rdfs:label xml:lang="it">rappresentaNazione</rdfs:label>
    </owl:DatatypeProperty>
    


    <!-- http://www.semanticweb.org/2021/ontologies/calcio#squadraHaValoreDiMercato -->

    <owl:DatatypeProperty rdf:about="http://www.semanticweb.org/2021/ontologies/calcio#squadraHaValoreDiMercato">
        <rdf:type rdf:resource="http://www.w3.org/2002/07/owl#FunctionalProperty"/>
        <rdfs:domain rdf:resource="http://www.semanticweb.org/2021/ontologies/calcio#Squadra"/>
        <rdfs:range rdf:resource="http://www.w3.org/2001/XMLSchema#long"/>
        <rdfs:comment xml:lang="en">Market value of the team obtained starting from the single market values of the players that compose it.</rdfs:comment>
        <rdfs:comment xml:lang="it">Valore di mercato della squadra ottenuto a partire dai singolo valori di merccato dei giocatori che la compongono.</rdfs:comment>
        <rdfs:label xml:lang="it">squadraHaValoreDiMercato</rdfs:label>
        <rdfs:label xml:lang="en">teamHasMarketValue</rdfs:label>
    </owl:DatatypeProperty>
    


    <!-- http://www.semanticweb.org/2021/ontologies/calcio#stipendioCorrente -->

    <owl:DatatypeProperty rdf:about="http://www.semanticweb.org/2021/ontologies/calcio#stipendioCorrente">
        <rdf:type rdf:resource="http://www.w3.org/2002/07/owl#FunctionalProperty"/>
        <rdfs:domain rdf:resource="http://xmlns.com/foaf/0.1/Person"/>
        <rdfs:range rdf:resource="http://www.w3.org/2001/XMLSchema#long"/>
        <rdfs:comment xml:lang="en">Current salary of the player</rdfs:comment>
        <rdfs:comment xml:lang="it">Stipendio attuale del calciatore.</rdfs:comment>
        <rdfs:label xml:lang="en">currentSalary</rdfs:label>
        <rdfs:label xml:lang="it">stipendioCorrente</rdfs:label>
    </owl:DatatypeProperty>
    


    <!-- http://www.semanticweb.org/2021/ontologies/calcio#trofeoHaNome -->

    <owl:DatatypeProperty rdf:about="http://www.semanticweb.org/2021/ontologies/calcio#trofeoHaNome">
        <rdfs:domain rdf:resource="http://www.semanticweb.org/2021/ontologies/calcio#Trofeo"/>
        <rdfs:range rdf:resource="http://www.w3.org/2001/XMLSchema#string"/>
        <rdfs:comment xml:lang="en">Name with which a cup / trophy is identified.</rdfs:comment>
        <rdfs:comment xml:lang="it">Nome con cui viene identificata una coppa/trofeo.</rdfs:comment>
        <rdfs:label xml:lang="it">trofeoHaNome</rdfs:label>
        <rdfs:label xml:lang="en">trophyHasName</rdfs:label>
    </owl:DatatypeProperty>
    


    <!-- 
    ///////////////////////////////////////////////////////////////////////////////////////
    //
    // Classes
    //
    ///////////////////////////////////////////////////////////////////////////////////////
     -->

    


    <!-- http://dbpedia.org/ontology/SoccerPlayer -->

    <owl:Class rdf:about="http://dbpedia.org/ontology/SoccerPlayer">
        <owl:equivalentClass rdf:resource="http://www.semanticweb.org/2021/ontologies/calcio#Calciatore"/>
    </owl:Class>
    


    <!-- http://www.semanticweb.org/2021/ontologies/calcio#Allenatore -->

    <owl:Class rdf:about="http://www.semanticweb.org/2021/ontologies/calcio#Allenatore">
        <owl:equivalentClass>
            <owl:Restriction>
                <owl:onProperty rdf:resource="http://www.semanticweb.org/2021/ontologies/calcio#allenaSquadra"/>
                <owl:qualifiedCardinality rdf:datatype="http://www.w3.org/2001/XMLSchema#nonNegativeInteger">1</owl:qualifiedCardinality>
                <owl:onClass rdf:resource="http://www.semanticweb.org/2021/ontologies/calcio#Squadra"/>
            </owl:Restriction>
        </owl:equivalentClass>
        <rdfs:subClassOf rdf:resource="http://xmlns.com/foaf/0.1/Person"/>
        <owl:disjointUnionOf rdf:parseType="Collection">
            <rdf:Description rdf:about="http://www.semanticweb.org/2021/ontologies/calcio#allenatoreDiClub"/>
            <rdf:Description rdf:about="http://www.semanticweb.org/2021/ontologies/calcio#allenatoreDiNazionale"/>
        </owl:disjointUnionOf>
        <rdfs:comment xml:lang="en">In sports, a coach is a person involved in the direction, instruction and training of the operations of a sports team or of individual sportspeople. A coach may also be a teacher.</rdfs:comment>
        <rdfs:comment xml:lang="it">L&apos;allenatore è la figura sportiva che si occupa della preparazione degli atleti.</rdfs:comment>
        <rdfs:label xml:lang="it">Allenatore</rdfs:label>
        <rdfs:label xml:lang="en">Coach</rdfs:label>
    </owl:Class>
    


    <!-- http://www.semanticweb.org/2021/ontologies/calcio#Arbitro -->

    <owl:Class rdf:about="http://www.semanticweb.org/2021/ontologies/calcio#Arbitro">
        <owl:equivalentClass>
            <owl:Restriction>
                <owl:onProperty rdf:resource="http://www.semanticweb.org/2021/ontologies/calcio#arbitraIn"/>
                <owl:someValuesFrom rdf:resource="http://www.semanticweb.org/2021/ontologies/calcio#Lega"/>
            </owl:Restriction>
        </owl:equivalentClass>
        <rdfs:subClassOf rdf:resource="http://xmlns.com/foaf/0.1/Person"/>
        <rdfs:comment xml:lang="it">L&apos;arbitro, noto anche con i termini di direttore di gara o ufficiale di gara, è una figura sportiva ed è colui che durante una partita di calcio, &quot;arbitra&quot; (dirige) l&apos;incontro e assicura che essa si svolga regolarmente ed avvenga il rispetto delle regole del gioco, stabilite dall&apos;IFAB, dalla FIFA e dalle varie federazioni calcistiche continentali e nazionali.</rdfs:comment>
        <rdfs:comment xml:lang="en">The referee is the person responsible for enforcing the Laws of the Game (LOTG) during an association football [a] match. He or she is the final decision-making authority on all facts connected with play, and is the only official on the pitch with the authority to start and stop play and impose disciplinary action against players during a match. At most levels of play the referee is assisted by two assistant referees (formerly known as linesmen), who are empowered to advise the referee in certain situations such as the ball leaving play or infringements of the Laws of the Game occurring out of the view of the referee; however, the assistant referees&apos; decisions are not binding and the referee has authority to overrule an assistant referee. At higher levels of play the referee may also be assisted by a fourth official who supervises the teams&apos; technical areas and assists the referee with administrative tasks, and, at the very highest levels, additional assistant referees and/or video assistant referees.</rdfs:comment>
        <rdfs:label xml:lang="it">Arbitro</rdfs:label>
        <rdfs:label xml:lang="en">Referee</rdfs:label>
    </owl:Class>
    


    <!-- http://www.semanticweb.org/2021/ontologies/calcio#Attaccante -->

    <owl:Class rdf:about="http://www.semanticweb.org/2021/ontologies/calcio#Attaccante">
        <rdfs:subClassOf rdf:resource="http://www.semanticweb.org/2021/ontologies/calcio#RuoloCalciatore"/>
        <rdfs:comment xml:lang="en">Forwards are the players on an association football team who play nearest to the opposing team&apos;s goal, and are therefore most responsible for scoring goals.
Their advanced position and limited defensive responsibilities mean forwards normally score more goals on behalf of their team than other players.
Modern team formations generally include one to three forwards; for example, the common 4–2–3–1 formation includes one forward.</rdfs:comment>
        <rdfs:comment xml:lang="it">È definito attaccante il calciatore con l&apos;obiettivo primario di realizzare gol per la propria squadra.</rdfs:comment>
        <rdfs:label xml:lang="it">Attaccante</rdfs:label>
        <rdfs:label xml:lang="en">Forward</rdfs:label>
    </owl:Class>
    


    <!-- http://www.semanticweb.org/2021/ontologies/calcio#Calciatore -->

    <owl:Class rdf:about="http://www.semanticweb.org/2021/ontologies/calcio#Calciatore">
        <owl:equivalentClass>
            <owl:Restriction>
                <owl:onProperty rdf:resource="http://www.semanticweb.org/2021/ontologies/calcio#giocaPer"/>
                <owl:someValuesFrom rdf:resource="http://www.semanticweb.org/2021/ontologies/calcio#Squadra"/>
            </owl:Restriction>
        </owl:equivalentClass>
        <rdfs:subClassOf rdf:resource="http://xmlns.com/foaf/0.1/Person"/>
        <rdfs:comment xml:lang="en">A football player or footballer is a sport person who plays one of the different types of football. The main types of football are association football, American football, Canadian football, Australian rules football, Gaelic football, rugby league and rugby union.</rdfs:comment>
        <rdfs:comment xml:lang="it">Il calciatore è un atleta che pratica lo sport del calcio.</rdfs:comment>
        <rdfs:label xml:lang="it">Calciatore</rdfs:label>
        <rdfs:label xml:lang="en">SoccerPlayer</rdfs:label>
    </owl:Class>
    


    <!-- http://www.semanticweb.org/2021/ontologies/calcio#Centrocampista -->

    <owl:Class rdf:about="http://www.semanticweb.org/2021/ontologies/calcio#Centrocampista">
        <rdfs:subClassOf rdf:resource="http://www.semanticweb.org/2021/ontologies/calcio#RuoloCalciatore"/>
        <rdfs:comment xml:lang="en">A midfielder is an association football position. Midfielders are generally positioned on the field between their team&apos;s defenders and forwards. Some midfielders play a disciplined defensive role, breaking up attacks, and are otherwise known as defensive midfielders. Others blur the boundaries, being more mobile and efficient in passing: they are commonly referred to as deep-lying midfielders, play-makers, box-to-box, or holding midfielders. The number of midfielders on a team and their assigned roles depends on the team&apos;s formation; the collective group of these players on the field is sometimes referred to as the midfield.</rdfs:comment>
        <rdfs:comment xml:lang="it">Il centrocampista è un ruolo presente in alcuni sport di squadra, in particolar modo calcio e football australiano.</rdfs:comment>
        <rdfs:label xml:lang="it">Centrocampista</rdfs:label>
        <rdfs:label xml:lang="en">Midfielder</rdfs:label>
    </owl:Class>
    


    <!-- http://www.semanticweb.org/2021/ontologies/calcio#Difensore -->

    <owl:Class rdf:about="http://www.semanticweb.org/2021/ontologies/calcio#Difensore">
        <rdfs:subClassOf rdf:resource="http://www.semanticweb.org/2021/ontologies/calcio#RuoloCalciatore"/>
        <rdfs:comment xml:lang="en">In the sport of association football, a defender is an outfield player whose primary roles are to stop attacks during the game and prevent the opposing team from scoring goals.
Centre backs are usually in pairs, with 2 full-backs to their left and right, but can come in threes with no full backs.
There are four types of defenders: centre-back, sweeper, full-back, and wing-back. The centre-back and full-back positions are essential in most modern formations. The sweeper and wing-back roles are more specialized for certain formations.</rdfs:comment>
        <rdfs:comment xml:lang="it">È definito difensore il calciatore con l&apos;obiettivo principale di proteggere la propria squadra dall&apos;offensiva avversaria.</rdfs:comment>
        <rdfs:label xml:lang="en">Defender</rdfs:label>
        <rdfs:label xml:lang="it">Difensore</rdfs:label>
    </owl:Class>
    


    <!-- http://www.semanticweb.org/2021/ontologies/calcio#Dirigente -->

    <owl:Class rdf:about="http://www.semanticweb.org/2021/ontologies/calcio#Dirigente">
        <owl:equivalentClass>
            <owl:Restriction>
                <owl:onProperty rdf:resource="http://www.semanticweb.org/2021/ontologies/calcio#lavoraPer"/>
                <owl:someValuesFrom rdf:resource="http://www.semanticweb.org/2021/ontologies/calcio#Squadra"/>
            </owl:Restriction>
        </owl:equivalentClass>
        <rdfs:subClassOf rdf:resource="http://xmlns.com/foaf/0.1/Person"/>
        <rdfs:comment xml:lang="en">An executive is a public or private employee who is part of the management of a public or private organization; the term is often used as a synonym for manager.</rdfs:comment>
        <rdfs:comment xml:lang="it">Un dirigente è un lavoratore dipendente pubblico o privato che fa parte della direzione di un&apos;organizzazione pubblica o privata; il termine viene spesso utilizzato come sinonimo di manager.</rdfs:comment>
        <rdfs:label xml:lang="it">Dirigente</rdfs:label>
        <rdfs:label xml:lang="en">Executive</rdfs:label>
    </owl:Class>
    


    <!-- http://www.semanticweb.org/2021/ontologies/calcio#Lega -->

    <owl:Class rdf:about="http://www.semanticweb.org/2021/ontologies/calcio#Lega">
        <rdfs:comment xml:lang="it">Il campionato è una manifestazione, o torneo, cui prendono parte singoli atleti oppure squadre per contendersi il titolo di &quot;campione&quot;.</rdfs:comment>
        <rdfs:comment xml:lang="en">In sport, a championship is a competition in which the aim is to decide which individual or team is the champion.</rdfs:comment>
        <rdfs:label xml:lang="en">League</rdfs:label>
        <rdfs:label xml:lang="it">Lega</rdfs:label>
    </owl:Class>
    


    <!-- http://www.semanticweb.org/2021/ontologies/calcio#Portiere -->

    <owl:Class rdf:about="http://www.semanticweb.org/2021/ontologies/calcio#Portiere">
        <rdfs:subClassOf rdf:resource="http://www.semanticweb.org/2021/ontologies/calcio#RuoloCalciatore"/>
        <rdfs:comment xml:lang="it">Nel calcio, il portiere è il giocatore che ha l&apos;obiettivo di difendere la porta della propria squadra. A tale scopo, è l&apos;unico calciatore cui è permesso giocare il pallone con qualsiasi parte del suo corpo, incluse le mani. Tale concessione è tuttavia valida solo all&apos;interno della propria area di rigore: fuori da essa, al portiere vengono applicate le norme valide per i giocatori di movimento.</rdfs:comment>
        <rdfs:comment xml:lang="en">The goalkeeper, often shortened to keeper or goalie, is one of the major positions of association football. It is the most specialised position in the sport. The goalkeeper&apos;s primary role is to prevent the opposing team from scoring (moving the ball over the defended goal-line within the frame of the goal). This is accomplished by the goalkeeper moving into the path of the ball and either catching it or directing it away from the vicinity of the goal line. Within the penalty area goalkeepers are able to use their hands, making them (outside throw-ins) the only players on the field permitted to handle the ball. The special status of goalkeepers is indicated by them wearing different coloured kits from their teammates.</rdfs:comment>
        <rdfs:label xml:lang="en">Goalkepeer</rdfs:label>
        <rdfs:label xml:lang="it">Portiere</rdfs:label>
    </owl:Class>
    


    <!-- http://www.semanticweb.org/2021/ontologies/calcio#RuoloCalciatore -->

    <owl:Class rdf:about="http://www.semanticweb.org/2021/ontologies/calcio#RuoloCalciatore">
        <rdfs:comment xml:lang="en">A Concept that classifies an Object &quot;Calciatore&quot;</rdfs:comment>
        <rdfs:comment xml:lang="it">Un concetto che classifica un oggetto &quot;Calciatore&quot;</rdfs:comment>
        <rdfs:label xml:lang="it">Ruolo calciatore</rdfs:label>
        <rdfs:label xml:lang="en">SoccerPlayer&apos;s role</rdfs:label>
    </owl:Class>
    


    <!-- http://www.semanticweb.org/2021/ontologies/calcio#Squadra -->

    <owl:Class rdf:about="http://www.semanticweb.org/2021/ontologies/calcio#Squadra">
        <owl:disjointUnionOf rdf:parseType="Collection">
            <rdf:Description rdf:about="http://www.semanticweb.org/2021/ontologies/calcio#squadraDiClub"/>
            <rdf:Description rdf:about="http://www.semanticweb.org/2021/ontologies/calcio#squadraNazionale"/>
        </owl:disjointUnionOf>
        <rdfs:comment xml:lang="en">A football team is a group of players selected to play together in the various team sports known as football. Such teams could be selected to play in a match against an opposing team, to represent a football club, group, state or nation, an all-star team or even selected as a hypothetical team (such as a Dream Team or Team of the Century) and never play an actual match.</rdfs:comment>
        <rdfs:comment xml:lang="it">Una squadra di calcio (in inglese: football club) è un&apos;associazione con finalità sportive, il cui scopo è l&apos;insegnamento e la pratica del gioco del calcio.
Denominata anche &quot;società calcistica&quot; oppure &quot;club calcistico&quot;, l&apos;espressione include in sé anche tutti quegli aspetti di organizzazione sportiva, amministrativa e dirigenziale legati all&apos;esistenza e alla gestione della società.
In genere, analogamente agli altri sport, si distingue tra club dilettantistici e club professionistici.
Un club può occuparsi solo di calcio oppure essere parte di una più ampia società polisportiva.</rdfs:comment>
        <rdfs:label xml:lang="en">Football Team</rdfs:label>
        <rdfs:label xml:lang="it">Squadra</rdfs:label>
    </owl:Class>
    


    <!-- http://www.semanticweb.org/2021/ontologies/calcio#Stadio -->

    <owl:Class rdf:about="http://www.semanticweb.org/2021/ontologies/calcio#Stadio">
        <owl:disjointUnionOf rdf:parseType="Collection">
            <rdf:Description rdf:about="http://www.semanticweb.org/2021/ontologies/calcio#stadioMedio"/>
            <rdf:Description rdf:about="http://www.semanticweb.org/2021/ontologies/calcio#stadioPiccolo"/>
            <rdf:Description rdf:about="http://www.semanticweb.org/2021/ontologies/calcio#stadioTop"/>
        </owl:disjointUnionOf>
        <rdfs:comment xml:lang="it">Lo stadio di calcio è un impianto sportivo destinato al gioco del calcio, costituito dal campo di gioco, dalle tribune e dalle ulteriori strutture complementari. Talvolta uno stadio viene utilizzato per altri sport, ad esempio il rugby, oppure per eventi come concerti.</rdfs:comment>
        <rdfs:comment xml:lang="en">Soccer-specific stadium is a term used mainly in the United States and Canada[1] to refer to a sports stadium either purpose-built or fundamentally redesigned for soccer and whose primary function is to host soccer matches, as opposed to a multi-purpose stadium which is for a variety of sports. A soccer-specific stadium may host other sporting events (such as lacrosse, American football and rugby) and concerts, but the design and purpose of a soccer-specific stadium is primarily for soccer.</rdfs:comment>
        <rdfs:label xml:lang="en">Soccer-specific stadium</rdfs:label>
        <rdfs:label xml:lang="it">Stadio</rdfs:label>
    </owl:Class>
    


    <!-- http://www.semanticweb.org/2021/ontologies/calcio#Trofeo -->

    <owl:Class rdf:about="http://www.semanticweb.org/2021/ontologies/calcio#Trofeo">
        <owl:disjointUnionOf rdf:parseType="Collection">
            <rdf:Description rdf:about="http://www.semanticweb.org/2021/ontologies/calcio#trofeoDiClub"/>
            <rdf:Description rdf:about="http://www.semanticweb.org/2021/ontologies/calcio#trofeoDiNazione"/>
        </owl:disjointUnionOf>
        <rdfs:comment xml:lang="en">A trophy is a tangible, durable reminder of a specific achievement, and serves as a recognition or evidence of merit. Trophies are often awarded for sporting events, from youth sports to professional level athletics. In many sports medals (or, in North America, rings) are often given out either as the trophy or along with more traditional trophies.</rdfs:comment>
        <rdfs:comment xml:lang="it">Il trofeo è un premio che viene assegnato o dedicato per un particolare merito. Nella sua accezione originaria, indicava la pratica dei guerrieri di rientrare in patria con le armi e le spoglie del nemico in seguito alla vittoria.</rdfs:comment>
        <rdfs:label xml:lang="it">Trofeo</rdfs:label>
        <rdfs:label xml:lang="en">Trophy</rdfs:label>
    </owl:Class>
    


    <!-- http://www.semanticweb.org/2021/ontologies/calcio#allenatoreDiClub -->

    <owl:Class rdf:about="http://www.semanticweb.org/2021/ontologies/calcio#allenatoreDiClub">
        <owl:equivalentClass>
            <owl:Restriction>
                <owl:onProperty rdf:resource="http://www.semanticweb.org/2021/ontologies/calcio#allenaSquadra"/>
                <owl:qualifiedCardinality rdf:datatype="http://www.w3.org/2001/XMLSchema#nonNegativeInteger">1</owl:qualifiedCardinality>
                <owl:onClass rdf:resource="http://www.semanticweb.org/2021/ontologies/calcio#squadraDiClub"/>
            </owl:Restriction>
        </owl:equivalentClass>
        <rdfs:subClassOf rdf:resource="http://www.semanticweb.org/2021/ontologies/calcio#Allenatore"/>
        <owl:disjointWith rdf:resource="http://www.semanticweb.org/2021/ontologies/calcio#allenatoreDiNazionale"/>
        <rdfs:comment xml:lang="it">L&apos;allenatore di club è un allenatore che allena una squadra di club.</rdfs:comment>
        <rdfs:comment xml:lang="en">The club manager is a manager who trains a club team.</rdfs:comment>
        <rdfs:label xml:lang="it">Allenatore di club</rdfs:label>
        <rdfs:label xml:lang="en">Club&apos;s manager</rdfs:label>
    </owl:Class>
    


    <!-- http://www.semanticweb.org/2021/ontologies/calcio#allenatoreDiClubFamoso -->

    <owl:Class rdf:about="http://www.semanticweb.org/2021/ontologies/calcio#allenatoreDiClubFamoso">
        <rdfs:subClassOf rdf:resource="http://www.semanticweb.org/2021/ontologies/calcio#allenatoreDiClub"/>
        <rdfs:comment xml:lang="it">L&apos;allenatore di club è un allenatore che allena una squadra di club famosa.</rdfs:comment>
        <rdfs:comment xml:lang="en">The club manager is a manager who trains a famous club team.</rdfs:comment>
        <rdfs:label xml:lang="it">Allenatore di club famoso</rdfs:label>
        <rdfs:label xml:lang="en">Famous club&apos;s manager</rdfs:label>
    </owl:Class>
    


    <!-- http://www.semanticweb.org/2021/ontologies/calcio#allenatoreDiNazionale -->

    <owl:Class rdf:about="http://www.semanticweb.org/2021/ontologies/calcio#allenatoreDiNazionale">
        <owl:equivalentClass>
            <owl:Restriction>
                <owl:onProperty rdf:resource="http://www.semanticweb.org/2021/ontologies/calcio#allenaSquadra"/>
                <owl:qualifiedCardinality rdf:datatype="http://www.w3.org/2001/XMLSchema#nonNegativeInteger">1</owl:qualifiedCardinality>
                <owl:onClass rdf:resource="http://www.semanticweb.org/2021/ontologies/calcio#squadraNazionale"/>
            </owl:Restriction>
        </owl:equivalentClass>
        <rdfs:subClassOf rdf:resource="http://www.semanticweb.org/2021/ontologies/calcio#Allenatore"/>
        <rdfs:comment xml:lang="it">Allenatore che allena una squadra Nazionale.</rdfs:comment>
        <rdfs:comment xml:lang="en">Coach who trains a national team.</rdfs:comment>
        <rdfs:label xml:lang="it">Allenatore di Nazionale</rdfs:label>
        <rdfs:label xml:lang="en">National&apos;s Team Manager</rdfs:label>
    </owl:Class>
    


    <!-- http://www.semanticweb.org/2021/ontologies/calcio#calciatoreMoltoPagato -->

    <owl:Class rdf:about="http://www.semanticweb.org/2021/ontologies/calcio#calciatoreMoltoPagato">
        <rdfs:subClassOf rdf:resource="http://www.semanticweb.org/2021/ontologies/calcio#Calciatore"/>
        <rdfs:comment xml:lang="it">Calciatore il cui stipendio è molto elevato.</rdfs:comment>
        <rdfs:comment xml:lang="en">Footballer whose salary is very high.</rdfs:comment>
        <rdfs:label xml:lang="it">Calaciatore molto pagato</rdfs:label>
        <rdfs:label xml:lang="en">Highly paid footballer</rdfs:label>
    </owl:Class>
    


    <!-- http://www.semanticweb.org/2021/ontologies/calcio#calciatoreTop -->

    <owl:Class rdf:about="http://www.semanticweb.org/2021/ontologies/calcio#calciatoreTop">
        <owl:equivalentClass>
            <owl:Restriction>
                <owl:onProperty rdf:resource="http://www.semanticweb.org/2021/ontologies/calcio#calciatoreHaValoreDiMercato"/>
                <owl:someValuesFrom>
                    <rdfs:Datatype>
                        <owl:onDatatype rdf:resource="http://www.w3.org/2001/XMLSchema#long"/>
                        <owl:withRestrictions rdf:parseType="Collection">
                            <rdf:Description>
                                <xsd:minInclusive rdf:datatype="http://www.w3.org/2001/XMLSchema#long">80000000</xsd:minInclusive>
                            </rdf:Description>
                        </owl:withRestrictions>
                    </rdfs:Datatype>
                </owl:someValuesFrom>
            </owl:Restriction>
        </owl:equivalentClass>
        <rdfs:subClassOf rdf:resource="http://xmlns.com/foaf/0.1/Person"/>
        <rdfs:comment xml:lang="it">Calciatore il cui valore di mercato è molto elevato.</rdfs:comment>
        <rdfs:comment xml:lang="en">Footballer whose market value is very high.</rdfs:comment>
        <rdfs:label xml:lang="it">Calaciatore top</rdfs:label>
        <rdfs:label xml:lang="en">Top SoccerPlayer</rdfs:label>
    </owl:Class>
    


    <!-- http://www.semanticweb.org/2021/ontologies/calcio#legheFrancesi -->

    <owl:Class rdf:about="http://www.semanticweb.org/2021/ontologies/calcio#legheFrancesi">
        <owl:equivalentClass>
            <owl:Class>
                <owl:oneOf rdf:parseType="Collection">
                    <rdf:Description rdf:about="http://www.semanticweb.org/2021/ontologies/calcio#Ligue1"/>
                    <rdf:Description rdf:about="http://www.semanticweb.org/2021/ontologies/calcio#Ligue2"/>
                </owl:oneOf>
            </owl:Class>
        </owl:equivalentClass>
        <rdfs:subClassOf rdf:resource="http://www.semanticweb.org/2021/ontologies/calcio#Lega"/>
        <rdfs:comment xml:lang="it">Campionati di calcio disputati in &quot;Francia&quot;.</rdfs:comment>
        <rdfs:comment xml:lang="en">Football championships held in &quot;France&quot;.</rdfs:comment>
        <rdfs:label xml:lang="en">French leagues</rdfs:label>
        <rdfs:label xml:lang="it">Leghe Francesi</rdfs:label>
    </owl:Class>
    


    <!-- http://www.semanticweb.org/2021/ontologies/calcio#legheInglesi -->

    <owl:Class rdf:about="http://www.semanticweb.org/2021/ontologies/calcio#legheInglesi">
        <owl:equivalentClass>
            <owl:Class>
                <owl:oneOf rdf:parseType="Collection">
                    <rdf:Description rdf:about="http://www.semanticweb.org/2021/ontologies/calcio#Championship"/>
                    <rdf:Description rdf:about="http://www.semanticweb.org/2021/ontologies/calcio#PremierLeague"/>
                </owl:oneOf>
            </owl:Class>
        </owl:equivalentClass>
        <rdfs:subClassOf rdf:resource="http://www.semanticweb.org/2021/ontologies/calcio#Lega"/>
        <rdfs:comment xml:lang="it">Campionati di calcio svolti in &quot;Inghilterra&quot;.</rdfs:comment>
        <rdfs:comment xml:lang="en">Football championships held in &quot;England&quot;.</rdfs:comment>
        <rdfs:label xml:lang="en">English&apos;s Leagues</rdfs:label>
        <rdfs:label xml:lang="it">Leghe Inglesi</rdfs:label>
    </owl:Class>
    


    <!-- http://www.semanticweb.org/2021/ontologies/calcio#legheItaliane -->

    <owl:Class rdf:about="http://www.semanticweb.org/2021/ontologies/calcio#legheItaliane">
        <owl:equivalentClass>
            <owl:Class>
                <owl:oneOf rdf:parseType="Collection">
                    <rdf:Description rdf:about="http://www.semanticweb.org/2021/ontologies/calcio#SerieA"/>
                    <rdf:Description rdf:about="http://www.semanticweb.org/2021/ontologies/calcio#SerieB"/>
                    <rdf:Description rdf:about="http://www.semanticweb.org/2021/ontologies/calcio#SerieC"/>
                </owl:oneOf>
            </owl:Class>
        </owl:equivalentClass>
        <rdfs:subClassOf rdf:resource="http://www.semanticweb.org/2021/ontologies/calcio#Lega"/>
        <rdfs:comment xml:lang="it">Campionati di calcio svolti in &quot;Italia&quot;.</rdfs:comment>
        <rdfs:comment xml:lang="en">Football championships held in &quot;Italy&quot;.</rdfs:comment>
        <rdfs:label xml:lang="en">Italian leagues</rdfs:label>
        <rdfs:label xml:lang="it">Leghe Italiane</rdfs:label>
    </owl:Class>
    


    <!-- http://www.semanticweb.org/2021/ontologies/calcio#legheSpagnole -->

    <owl:Class rdf:about="http://www.semanticweb.org/2021/ontologies/calcio#legheSpagnole">
        <owl:equivalentClass>
            <owl:Class>
                <owl:oneOf rdf:parseType="Collection">
                    <rdf:Description rdf:about="http://www.semanticweb.org/2021/ontologies/calcio#LaLiga"/>
                    <rdf:Description rdf:about="http://www.semanticweb.org/2021/ontologies/calcio#SegundaDivisión"/>
                </owl:oneOf>
            </owl:Class>
        </owl:equivalentClass>
        <rdfs:subClassOf rdf:resource="http://www.semanticweb.org/2021/ontologies/calcio#Lega"/>
        <rdfs:comment xml:lang="it">Campionati di calcio svolti in &quot;Spagna&quot;.</rdfs:comment>
        <rdfs:comment xml:lang="en">Football championships held in &quot;Spain&quot;.</rdfs:comment>
        <rdfs:label xml:lang="it">Leghe Spagnole</rdfs:label>
        <rdfs:label xml:lang="en">Spanish leagues</rdfs:label>
    </owl:Class>
    


    <!-- http://www.semanticweb.org/2021/ontologies/calcio#legheTedesche -->

    <owl:Class rdf:about="http://www.semanticweb.org/2021/ontologies/calcio#legheTedesche">
        <owl:equivalentClass>
            <owl:Class>
                <owl:oneOf rdf:parseType="Collection">
                    <rdf:Description rdf:about="http://www.semanticweb.org/2021/ontologies/calcio#Bundesliga"/>
                    <rdf:Description rdf:about="http://www.semanticweb.org/2021/ontologies/calcio#2.Bundesliga"/>
                </owl:oneOf>
            </owl:Class>
        </owl:equivalentClass>
        <rdfs:subClassOf rdf:resource="http://www.semanticweb.org/2021/ontologies/calcio#Lega"/>
        <rdfs:comment xml:lang="it">Campionati di calcio svolti in &quot;Germania&quot;.</rdfs:comment>
        <rdfs:comment xml:lang="en">Football championships held in &quot;Germany&quot;.</rdfs:comment>
        <rdfs:label xml:lang="en">German leagues</rdfs:label>
        <rdfs:label xml:lang="it">Leghe Tedesche</rdfs:label>
    </owl:Class>
    


    <!-- http://www.semanticweb.org/2021/ontologies/calcio#squadraDiClub -->

    <owl:Class rdf:about="http://www.semanticweb.org/2021/ontologies/calcio#squadraDiClub">
        <owl:equivalentClass>
            <owl:Restriction>
                <owl:onProperty rdf:resource="http://www.semanticweb.org/2021/ontologies/calcio#appartieneALega"/>
                <owl:qualifiedCardinality rdf:datatype="http://www.w3.org/2001/XMLSchema#nonNegativeInteger">1</owl:qualifiedCardinality>
                <owl:onClass rdf:resource="http://www.semanticweb.org/2021/ontologies/calcio#Lega"/>
            </owl:Restriction>
        </owl:equivalentClass>
        <rdfs:subClassOf rdf:resource="http://www.semanticweb.org/2021/ontologies/calcio#Squadra"/>
        <owl:disjointWith rdf:resource="http://www.semanticweb.org/2021/ontologies/calcio#squadraNazionale"/>
        <rdfs:comment xml:lang="en">Soccer team competing in a club championship.</rdfs:comment>
        <rdfs:comment xml:lang="it">Squadra di calcio che gareggia in un campionato per club.</rdfs:comment>
        <rdfs:label xml:lang="en">Club Team</rdfs:label>
        <rdfs:label xml:lang="it">Squadra di Club</rdfs:label>
    </owl:Class>
    


    <!-- http://www.semanticweb.org/2021/ontologies/calcio#squadraDiClubTop -->

    <owl:Class rdf:about="http://www.semanticweb.org/2021/ontologies/calcio#squadraDiClubTop">
        <owl:equivalentClass>
            <owl:Class>
                <owl:intersectionOf rdf:parseType="Collection">
                    <owl:Restriction>
                        <owl:onProperty rdf:resource="http://www.semanticweb.org/2021/ontologies/calcio#haVintoClub"/>
                        <owl:minQualifiedCardinality rdf:datatype="http://www.w3.org/2001/XMLSchema#nonNegativeInteger">7</owl:minQualifiedCardinality>
                        <owl:onClass rdf:resource="http://www.semanticweb.org/2021/ontologies/calcio#trofeoDiClub"/>
                    </owl:Restriction>
                    <owl:Restriction>
                        <owl:onProperty rdf:resource="http://www.semanticweb.org/2021/ontologies/calcio#squadraHaValoreDiMercato"/>
                        <owl:someValuesFrom>
                            <rdfs:Datatype>
                                <owl:onDatatype rdf:resource="http://www.w3.org/2001/XMLSchema#long"/>
                                <owl:withRestrictions rdf:parseType="Collection">
                                    <rdf:Description>
                                        <xsd:minInclusive rdf:datatype="http://www.w3.org/2001/XMLSchema#long">400000000</xsd:minInclusive>
                                    </rdf:Description>
                                </owl:withRestrictions>
                            </rdfs:Datatype>
                        </owl:someValuesFrom>
                    </owl:Restriction>
                </owl:intersectionOf>
            </owl:Class>
        </owl:equivalentClass>
        <rdfs:subClassOf rdf:resource="http://www.semanticweb.org/2021/ontologies/calcio#Squadra"/>
        <rdfs:comment xml:lang="en">Club team that has won at least seven club trophies and has a high market value.</rdfs:comment>
        <rdfs:comment xml:lang="it">Squadra di club che ha vinto minimo sette trofei di club ed ha un valore di mercato elevato.</rdfs:comment>
        <rdfs:label xml:lang="it">Squadra di club top</rdfs:label>
        <rdfs:label xml:lang="en">Top Club Team</rdfs:label>
    </owl:Class>
    


    <!-- http://www.semanticweb.org/2021/ontologies/calcio#squadraFrancese -->

    <owl:Class rdf:about="http://www.semanticweb.org/2021/ontologies/calcio#squadraFrancese">
        <owl:equivalentClass>
            <owl:Restriction>
                <owl:onProperty rdf:resource="http://www.semanticweb.org/2021/ontologies/calcio#appartieneALega"/>
                <owl:qualifiedCardinality rdf:datatype="http://www.w3.org/2001/XMLSchema#nonNegativeInteger">1</owl:qualifiedCardinality>
                <owl:onClass rdf:resource="http://www.semanticweb.org/2021/ontologies/calcio#legheFrancesi"/>
            </owl:Restriction>
        </owl:equivalentClass>
        <rdfs:subClassOf rdf:resource="http://www.semanticweb.org/2021/ontologies/calcio#squadraDiClub"/>
        <rdfs:comment xml:lang="en">Football team competing in a French league.</rdfs:comment>
        <rdfs:comment xml:lang="it">Squadra di calcio che gareggia in un campionato francese.</rdfs:comment>
        <rdfs:label xml:lang="en">French Team</rdfs:label>
        <rdfs:label xml:lang="it">Squadra Francese</rdfs:label>
    </owl:Class>
    


    <!-- http://www.semanticweb.org/2021/ontologies/calcio#squadraInglese -->

    <owl:Class rdf:about="http://www.semanticweb.org/2021/ontologies/calcio#squadraInglese">
        <owl:equivalentClass>
            <owl:Restriction>
                <owl:onProperty rdf:resource="http://www.semanticweb.org/2021/ontologies/calcio#appartieneALega"/>
                <owl:qualifiedCardinality rdf:datatype="http://www.w3.org/2001/XMLSchema#nonNegativeInteger">1</owl:qualifiedCardinality>
                <owl:onClass rdf:resource="http://www.semanticweb.org/2021/ontologies/calcio#legheInglesi"/>
            </owl:Restriction>
        </owl:equivalentClass>
        <rdfs:subClassOf rdf:resource="http://www.semanticweb.org/2021/ontologies/calcio#squadraDiClub"/>
        <rdfs:comment xml:lang="en">Football team competing in a English league.</rdfs:comment>
        <rdfs:comment xml:lang="it">Squadra di calcio che gareggia in un campionato inglese.</rdfs:comment>
        <rdfs:label xml:lang="en">English Team</rdfs:label>
        <rdfs:label xml:lang="it">Squadra Inglese</rdfs:label>
    </owl:Class>
    


    <!-- http://www.semanticweb.org/2021/ontologies/calcio#squadraItaliana -->

    <owl:Class rdf:about="http://www.semanticweb.org/2021/ontologies/calcio#squadraItaliana">
        <owl:equivalentClass>
            <owl:Restriction>
                <owl:onProperty rdf:resource="http://www.semanticweb.org/2021/ontologies/calcio#appartieneALega"/>
                <owl:qualifiedCardinality rdf:datatype="http://www.w3.org/2001/XMLSchema#nonNegativeInteger">1</owl:qualifiedCardinality>
                <owl:onClass rdf:resource="http://www.semanticweb.org/2021/ontologies/calcio#legheItaliane"/>
            </owl:Restriction>
        </owl:equivalentClass>
        <rdfs:subClassOf rdf:resource="http://www.semanticweb.org/2021/ontologies/calcio#squadraDiClub"/>
        <rdfs:comment xml:lang="en">Football team competing in an Italian league.</rdfs:comment>
        <rdfs:comment xml:lang="it">Squadra di calcio che gareggia in un campionato italiano.</rdfs:comment>
        <rdfs:label xml:lang="en">Italian Team</rdfs:label>
        <rdfs:label xml:lang="it">Squadra Italiana</rdfs:label>
    </owl:Class>
    


    <!-- http://www.semanticweb.org/2021/ontologies/calcio#squadraNazionale -->

    <owl:Class rdf:about="http://www.semanticweb.org/2021/ontologies/calcio#squadraNazionale">
        <rdfs:subClassOf rdf:resource="http://www.semanticweb.org/2021/ontologies/calcio#Squadra"/>
        <rdfs:comment xml:lang="en">Soccer team represents a nation.</rdfs:comment>
        <rdfs:comment xml:lang="it">Squadra di calcio rappresentate una nazione.</rdfs:comment>
        <rdfs:label xml:lang="en">National Team</rdfs:label>
        <rdfs:label xml:lang="it">Squadra Nazionale</rdfs:label>
    </owl:Class>
    


    <!-- http://www.semanticweb.org/2021/ontologies/calcio#squadraNazionaleTop -->

    <owl:Class rdf:about="http://www.semanticweb.org/2021/ontologies/calcio#squadraNazionaleTop">
        <owl:equivalentClass>
            <owl:Restriction>
                <owl:onProperty rdf:resource="http://www.semanticweb.org/2021/ontologies/calcio#haVintoNazionale"/>
                <owl:minQualifiedCardinality rdf:datatype="http://www.w3.org/2001/XMLSchema#nonNegativeInteger">5</owl:minQualifiedCardinality>
                <owl:onClass rdf:resource="http://www.semanticweb.org/2021/ontologies/calcio#trofeoDiNazione"/>
            </owl:Restriction>
        </owl:equivalentClass>
        <rdfs:subClassOf rdf:resource="http://www.semanticweb.org/2021/ontologies/calcio#Squadra"/>
        <rdfs:comment xml:lang="en">National team that has won at least five national trophies.</rdfs:comment>
        <rdfs:label xml:lang="en">Squadra Nazionale che ha vinto minimo cinque trofei nazionali.</rdfs:label>
        <rdfs:label xml:lang="it">Squadra nazionale top</rdfs:label>
        <rdfs:label xml:lang="en">Top National Team</rdfs:label>
    </owl:Class>
    


    <!-- http://www.semanticweb.org/2021/ontologies/calcio#squadraSpagnola -->

    <owl:Class rdf:about="http://www.semanticweb.org/2021/ontologies/calcio#squadraSpagnola">
        <owl:equivalentClass>
            <owl:Restriction>
                <owl:onProperty rdf:resource="http://www.semanticweb.org/2021/ontologies/calcio#appartieneALega"/>
                <owl:qualifiedCardinality rdf:datatype="http://www.w3.org/2001/XMLSchema#nonNegativeInteger">1</owl:qualifiedCardinality>
                <owl:onClass rdf:resource="http://www.semanticweb.org/2021/ontologies/calcio#legheSpagnole"/>
            </owl:Restriction>
        </owl:equivalentClass>
        <rdfs:subClassOf rdf:resource="http://www.semanticweb.org/2021/ontologies/calcio#squadraDiClub"/>
        <rdfs:comment xml:lang="en">Football team competing in a Spanish league.</rdfs:comment>
        <rdfs:comment xml:lang="it">Squadra di calcio che gareggia in un campionato spagnola.</rdfs:comment>
        <rdfs:label xml:lang="en">Spanish Team</rdfs:label>
        <rdfs:label xml:lang="it">Squadra Spagnola</rdfs:label>
    </owl:Class>
    


    <!-- http://www.semanticweb.org/2021/ontologies/calcio#squadraTedesca -->

    <owl:Class rdf:about="http://www.semanticweb.org/2021/ontologies/calcio#squadraTedesca">
        <owl:equivalentClass>
            <owl:Restriction>
                <owl:onProperty rdf:resource="http://www.semanticweb.org/2021/ontologies/calcio#appartieneALega"/>
                <owl:qualifiedCardinality rdf:datatype="http://www.w3.org/2001/XMLSchema#nonNegativeInteger">1</owl:qualifiedCardinality>
                <owl:onClass rdf:resource="http://www.semanticweb.org/2021/ontologies/calcio#legheTedesche"/>
            </owl:Restriction>
        </owl:equivalentClass>
        <rdfs:subClassOf rdf:resource="http://www.semanticweb.org/2021/ontologies/calcio#squadraDiClub"/>
        <rdfs:comment xml:lang="en">Football team competing in a German league.</rdfs:comment>
        <rdfs:comment xml:lang="it">Squadra di calcio che gareggia in un campionato tedesca.</rdfs:comment>
        <rdfs:label xml:lang="en">German Team</rdfs:label>
        <rdfs:label xml:lang="it">Squadra Tedesca</rdfs:label>
    </owl:Class>
    


    <!-- http://www.semanticweb.org/2021/ontologies/calcio#stadioMedio -->

    <owl:Class rdf:about="http://www.semanticweb.org/2021/ontologies/calcio#stadioMedio">
        <owl:equivalentClass>
            <owl:Restriction>
                <owl:onProperty rdf:resource="http://www.semanticweb.org/2021/ontologies/calcio#haCapienza"/>
                <owl:someValuesFrom>
                    <rdfs:Datatype>
                        <owl:onDatatype rdf:resource="http://www.w3.org/2001/XMLSchema#int"/>
                        <owl:withRestrictions rdf:parseType="Collection">
                            <rdf:Description>
                                <xsd:minInclusive rdf:datatype="http://www.w3.org/2001/XMLSchema#int">30000</xsd:minInclusive>
                            </rdf:Description>
                            <rdf:Description>
                                <xsd:maxInclusive rdf:datatype="http://www.w3.org/2001/XMLSchema#int">69999</xsd:maxInclusive>
                            </rdf:Description>
                        </owl:withRestrictions>
                    </rdfs:Datatype>
                </owl:someValuesFrom>
            </owl:Restriction>
        </owl:equivalentClass>
        <rdfs:comment xml:lang="en">Football stadium with an average seating capacity.</rdfs:comment>
        <rdfs:comment xml:lang="it">Stadio di calcio con una capacità di posti media.</rdfs:comment>
        <rdfs:label xml:lang="en">Medium-Size Soccer Stadium</rdfs:label>
        <rdfs:label xml:lang="it">Stadio Medio</rdfs:label>
    </owl:Class>
    


    <!-- http://www.semanticweb.org/2021/ontologies/calcio#stadioPiccolo -->

    <owl:Class rdf:about="http://www.semanticweb.org/2021/ontologies/calcio#stadioPiccolo">
        <owl:equivalentClass>
            <owl:Restriction>
                <owl:onProperty rdf:resource="http://www.semanticweb.org/2021/ontologies/calcio#haCapienza"/>
                <owl:someValuesFrom>
                    <rdfs:Datatype>
                        <owl:onDatatype rdf:resource="http://www.w3.org/2001/XMLSchema#int"/>
                        <owl:withRestrictions rdf:parseType="Collection">
                            <rdf:Description>
                                <xsd:minInclusive rdf:datatype="http://www.w3.org/2001/XMLSchema#int">1000</xsd:minInclusive>
                            </rdf:Description>
                            <rdf:Description>
                                <xsd:maxInclusive rdf:datatype="http://www.w3.org/2001/XMLSchema#int">29999</xsd:maxInclusive>
                            </rdf:Description>
                        </owl:withRestrictions>
                    </rdfs:Datatype>
                </owl:someValuesFrom>
            </owl:Restriction>
        </owl:equivalentClass>
        <rdfs:comment xml:lang="en">Football stadium with a small seating capacity.</rdfs:comment>
        <rdfs:comment xml:lang="it">Stadio di calcio con una capacità di posti piccola.</rdfs:comment>
        <rdfs:label xml:lang="en">Small-Size Soccer Stadium</rdfs:label>
        <rdfs:label xml:lang="it">Stadio Piccolo</rdfs:label>
    </owl:Class>
    


    <!-- http://www.semanticweb.org/2021/ontologies/calcio#stadioTop -->

    <owl:Class rdf:about="http://www.semanticweb.org/2021/ontologies/calcio#stadioTop">
        <owl:equivalentClass>
            <owl:Restriction>
                <owl:onProperty rdf:resource="http://www.semanticweb.org/2021/ontologies/calcio#haCapienza"/>
                <owl:someValuesFrom>
                    <rdfs:Datatype>
                        <owl:onDatatype rdf:resource="http://www.w3.org/2001/XMLSchema#int"/>
                        <owl:withRestrictions rdf:parseType="Collection">
                            <rdf:Description>
                                <xsd:minInclusive rdf:datatype="http://www.w3.org/2001/XMLSchema#int">70000</xsd:minInclusive>
                            </rdf:Description>
                            <rdf:Description>
                                <xsd:maxInclusive rdf:datatype="http://www.w3.org/2001/XMLSchema#int">200000</xsd:maxInclusive>
                            </rdf:Description>
                        </owl:withRestrictions>
                    </rdfs:Datatype>
                </owl:someValuesFrom>
            </owl:Restriction>
        </owl:equivalentClass>
        <rdfs:comment xml:lang="en">Football stadium with a big seating capacity.</rdfs:comment>
        <rdfs:comment xml:lang="it">Stadio di calcio con una capacità di posti grande.</rdfs:comment>
        <rdfs:label xml:lang="en">Large-Size Soccer Stadium</rdfs:label>
        <rdfs:label xml:lang="it">Stadio Grande</rdfs:label>
    </owl:Class>
    


    <!-- http://www.semanticweb.org/2021/ontologies/calcio#topLega -->

    <owl:Class rdf:about="http://www.semanticweb.org/2021/ontologies/calcio#topLega">
        <owl:equivalentClass>
            <owl:Class>
                <owl:oneOf rdf:parseType="Collection">
                    <rdf:Description rdf:about="http://www.semanticweb.org/2021/ontologies/calcio#Bundesliga"/>
                    <rdf:Description rdf:about="http://www.semanticweb.org/2021/ontologies/calcio#LaLiga"/>
                    <rdf:Description rdf:about="http://www.semanticweb.org/2021/ontologies/calcio#Ligue1"/>
                    <rdf:Description rdf:about="http://www.semanticweb.org/2021/ontologies/calcio#PremierLeague"/>
                    <rdf:Description rdf:about="http://www.semanticweb.org/2021/ontologies/calcio#SerieA"/>
                </owl:oneOf>
            </owl:Class>
        </owl:equivalentClass>
        <rdfs:subClassOf rdf:resource="http://www.semanticweb.org/2021/ontologies/calcio#Lega"/>
        <rdfs:comment xml:lang="en">First-class league.</rdfs:comment>
        <rdfs:comment xml:lang="it">Lega di massima categoria.</rdfs:comment>
        <rdfs:label xml:lang="it">Lega Top</rdfs:label>
        <rdfs:label xml:lang="en">Top&apos;s League</rdfs:label>
    </owl:Class>
    


    <!-- http://www.semanticweb.org/2021/ontologies/calcio#trofeoDiClub -->

    <owl:Class rdf:about="http://www.semanticweb.org/2021/ontologies/calcio#trofeoDiClub">
        <owl:equivalentClass>
            <owl:Class>
                <owl:intersectionOf rdf:parseType="Collection">
                    <rdf:Description rdf:about="http://www.semanticweb.org/2021/ontologies/calcio#Trofeo"/>
                    <owl:Restriction>
                        <owl:onProperty rdf:resource="http://www.semanticweb.org/2021/ontologies/calcio#vintoDa"/>
                        <owl:allValuesFrom rdf:resource="http://www.semanticweb.org/2021/ontologies/calcio#squadraDiClub"/>
                    </owl:Restriction>
                </owl:intersectionOf>
            </owl:Class>
        </owl:equivalentClass>
        <rdfs:subClassOf rdf:resource="http://www.semanticweb.org/2021/ontologies/calcio#Trofeo"/>
        <owl:disjointWith rdf:resource="http://www.semanticweb.org/2021/ontologies/calcio#trofeoDiNazione"/>
        <owl:disjointUnionOf rdf:parseType="Collection">
            <rdf:Description rdf:about="http://www.semanticweb.org/2021/ontologies/calcio#trofeoInternazionali"/>
            <rdf:Description rdf:about="http://www.semanticweb.org/2021/ontologies/calcio#trofeoNazionali"/>
        </owl:disjointUnionOf>
        <rdfs:comment xml:lang="it">Trofeo vinto da squadre di club.</rdfs:comment>
        <rdfs:comment xml:lang="en">Trophy won by club teams.</rdfs:comment>
        <rdfs:label xml:lang="en">Club&apos;s Trophy</rdfs:label>
        <rdfs:label xml:lang="it">Trofeo di Club</rdfs:label>
    </owl:Class>
    


    <!-- http://www.semanticweb.org/2021/ontologies/calcio#trofeoDiNazione -->

    <owl:Class rdf:about="http://www.semanticweb.org/2021/ontologies/calcio#trofeoDiNazione">
        <owl:equivalentClass>
            <owl:Class>
                <owl:intersectionOf rdf:parseType="Collection">
                    <rdf:Description rdf:about="http://www.semanticweb.org/2021/ontologies/calcio#Trofeo"/>
                    <owl:Restriction>
                        <owl:onProperty rdf:resource="http://www.semanticweb.org/2021/ontologies/calcio#vintoDa"/>
                        <owl:allValuesFrom rdf:resource="http://www.semanticweb.org/2021/ontologies/calcio#squadraNazionale"/>
                    </owl:Restriction>
                </owl:intersectionOf>
            </owl:Class>
        </owl:equivalentClass>
        <rdfs:subClassOf rdf:resource="http://www.semanticweb.org/2021/ontologies/calcio#Trofeo"/>
        <rdfs:comment xml:lang="it">Trofeo vinto da squadre Nazionali.</rdfs:comment>
        <rdfs:comment xml:lang="en">Trophy won by national teams.</rdfs:comment>
        <rdfs:label xml:lang="en">Nation&apos;s Trophy</rdfs:label>
        <rdfs:label xml:lang="it">Trofeo di Nazione</rdfs:label>
    </owl:Class>
    


    <!-- http://www.semanticweb.org/2021/ontologies/calcio#trofeoInternazionali -->

    <owl:Class rdf:about="http://www.semanticweb.org/2021/ontologies/calcio#trofeoInternazionali">
        <rdfs:subClassOf rdf:resource="http://www.semanticweb.org/2021/ontologies/calcio#trofeoDiClub"/>
        <owl:disjointWith rdf:resource="http://www.semanticweb.org/2021/ontologies/calcio#trofeoNazionali"/>
        <rdfs:comment xml:lang="en">Club trophy awarded internationally.</rdfs:comment>
        <rdfs:comment xml:lang="it">Trofeo di club conferito a livello internazionale.</rdfs:comment>
        <rdfs:label xml:lang="en">International&apos;s Trophy</rdfs:label>
        <rdfs:label xml:lang="it">Trofeo Internazionale</rdfs:label>
    </owl:Class>
    


    <!-- http://www.semanticweb.org/2021/ontologies/calcio#trofeoNazionali -->

    <owl:Class rdf:about="http://www.semanticweb.org/2021/ontologies/calcio#trofeoNazionali">
        <rdfs:subClassOf rdf:resource="http://www.semanticweb.org/2021/ontologies/calcio#trofeoDiClub"/>
        <rdfs:comment xml:lang="en">Club trophy awarded nationally.</rdfs:comment>
        <rdfs:comment xml:lang="it">Trofeo di club conferito a livello nazionale.</rdfs:comment>
        <rdfs:label xml:lang="en">National&apos;s Trophy</rdfs:label>
        <rdfs:label xml:lang="it">Trofeo Nazionale</rdfs:label>
    </owl:Class>
    


    <!-- http://www.semanticweb.org/2021/ontologies/calcio#trofeoUEFA -->

    <owl:Class rdf:about="http://www.semanticweb.org/2021/ontologies/calcio#trofeoUEFA">
        <rdfs:subClassOf rdf:resource="http://www.semanticweb.org/2021/ontologies/calcio#Trofeo"/>
        <rdfs:comment xml:lang="it">Trofeo conferito dall&apos;associazione sportiva UEFA.</rdfs:comment>
        <rdfs:comment xml:lang="en">Trophy awarded by the UEFA sports association.</rdfs:comment>
        <rdfs:label xml:lang="it">Trofeo UEFA</rdfs:label>
        <rdfs:label xml:lang="en">UEFA&apos;s Trophy</rdfs:label>
    </owl:Class>
    


    <!-- http://xmlns.com/foaf/0.1/Person -->

    <owl:Class rdf:about="http://xmlns.com/foaf/0.1/Person"/>
    


    <!-- 
    ///////////////////////////////////////////////////////////////////////////////////////
    //
    // Individuals
    //
    ///////////////////////////////////////////////////////////////////////////////////////
     -->

    


    <!-- http://dbpedia.org/resource/Serie_A -->

    <owl:NamedIndividual rdf:about="http://dbpedia.org/resource/Serie_A">
        <rdfs:comment xml:lang="it">(dbpedia) La Serie A, ufficialmente chiamata Serie A TIM per ragioni di sponsorizzazione, è il più alto livello professionistico del campionato italiano di calcio. Viene gestito dalla Lega Nazionale Professionisti Serie A. Posta sotto l&apos;egida della FIGC, la prima edizione del torneo risale al 1898; l&apos;attuale formula (a girone unico) nacque poi nel 1929. La squadra più titolata è la Juventus, vincitrice del campionato per 35 volte; l&apos;Inter è invece la formazione più presente nel girone unico, avendone disputata ogni stagione.</rdfs:comment>
        <rdfs:comment xml:lang="en">(dbpedia) Serie A (Italian pronunciation: [ˈsɛːrje ˈa]), also called Serie A TIM due to sponsorship by TIM, is a professional league competition for football clubs located at the top of the Italian football league system and the winner is awarded the Scudetto and the Coppa Campioni d&apos;Italia. It has been operating as a round-robin tournament for over ninety years since the 1929–30 season. It had been organized by the Direttorio Divisioni Superiori until 1943 and the Lega Calcio until 2010, when the Lega Serie A was created for the 2010–11 season. Serie A is regarded as one of the best football leagues in the world and it is often depicted as the most tactical and defensively sound national league. Serie A was the world&apos;s second-strongest national league in 2014 according to IFFHS. Serie A is ranked f</rdfs:comment>
        <rdfs:label xml:lang="en">Serie A</rdfs:label>
        <rdfs:label xml:lang="it">Serie A</rdfs:label>
    </owl:NamedIndividual>
    


    <!-- http://dbpedia.org/resource/Serie_B -->

    <owl:NamedIndividual rdf:about="http://dbpedia.org/resource/Serie_B">
        <rdfs:comment xml:lang="it">(dbpedia) La Serie B, ufficialmente nota come Serie BKT per ragioni di sponsorizzazione, è il secondo livello professionistico del campionato italiano di calcio, gestito dalla Lega Nazionale Professionisti B.</rdfs:comment>
        <rdfs:comment xml:lang="en">(dbpedia) Serie B (Italian pronunciation: [ˈsɛːrje ˈbi]), currently named Serie BKT for sponsorship reasons, is the second-highest division in the Italian football league system after the Serie A. It has been operating for over eighty years since the 1929–30 season. It had been organized by Lega Calcio until 2010, when the Lega Serie B was created for the 2010–11 season. Common nicknames for the league are campionato cadetto and cadetteria, as cadetto is the Italian for junior or cadet.</rdfs:comment>
        <rdfs:label xml:lang="en">Serie B</rdfs:label>
        <rdfs:label xml:lang="it">Serie B</rdfs:label>
    </owl:NamedIndividual>
    


    <!-- http://dbpedia.org/resource/Serie_C -->

    <owl:NamedIndividual rdf:about="http://dbpedia.org/resource/Serie_C">
        <rdfs:comment xml:lang="it">(dbpedia) La Serie C è la lega italiana di calcio di terzo livello, dopo la Serie A e la Serie B</rdfs:comment>
        <rdfs:comment xml:lang="en">(dbpedia) Serie C (Italian pronunciation: [ˈsɛːrje ˈci]), is the third-highest division in the Italian football league system after the Serie A and the Serie B</rdfs:comment>
        <rdfs:label xml:lang="en">Serie C</rdfs:label>
        <rdfs:label xml:lang="it">Serie C</rdfs:label>
    </owl:NamedIndividual>
    


    <!-- http://www.semanticweb.org/2021/ontologies/calcio#ACMilan -->

    <owl:NamedIndividual rdf:about="http://www.semanticweb.org/2021/ontologies/calcio#ACMilan">
        <owl:sameAs rdf:resource="http://www.wikidata.org/entity/Q1543"/>
        <appartieneALega rdf:resource="http://www.semanticweb.org/2021/ontologies/calcio#SerieA"/>
        <detieneCalciatore rdf:resource="http://www.semanticweb.org/2021/ontologies/calcio#Gianluigi_Donnarumma"/>
        <detieneCalciatore rdf:resource="http://www.semanticweb.org/2021/ontologies/calcio#Hakan_Çalhanoğlu"/>
        <detieneCalciatore rdf:resource="http://www.semanticweb.org/2021/ontologies/calcio#Theo_Hernández"/>
        <detieneCalciatore rdf:resource="http://www.semanticweb.org/2021/ontologies/calcio#Zlatan_Ibrahimović"/>
        <giocaInStadio rdf:resource="http://www.semanticweb.org/2021/ontologies/calcio#San_Siro"/>
        <haVintoClub rdf:resource="http://www.semanticweb.org/2021/ontologies/calcio#ChampionsLeague_2003"/>
        <haVintoClub rdf:resource="http://www.semanticweb.org/2021/ontologies/calcio#ChampionsLeague_2007"/>
        <haVintoClub rdf:resource="http://www.semanticweb.org/2021/ontologies/calcio#ChampionsLeague_63"/>
        <haVintoClub rdf:resource="http://www.semanticweb.org/2021/ontologies/calcio#ChampionsLeague_69"/>
        <haVintoClub rdf:resource="http://www.semanticweb.org/2021/ontologies/calcio#ChampionsLeague_89"/>
        <haVintoClub rdf:resource="http://www.semanticweb.org/2021/ontologies/calcio#ChampionsLeague_90"/>
        <haVintoClub rdf:resource="http://www.semanticweb.org/2021/ontologies/calcio#ChampionsLeague_94"/>
        <èAllenataDa rdf:resource="http://www.semanticweb.org/2021/ontologies/calcio#Stefano_Pioli"/>
        <haEtàMedia rdf:datatype="http://www.w3.org/2001/XMLSchema#float">24.6</haEtàMedia>
        <haNumeroCalciatori rdf:datatype="http://www.w3.org/2001/XMLSchema#integer">27</haNumeroCalciatori>
        <squadraHaValoreDiMercato rdf:datatype="http://www.w3.org/2001/XMLSchema#long">489300000</squadraHaValoreDiMercato>
        <rdfs:comment xml:lang="en">Associazione Calcio Milan (Italian pronunciation: [assotʃatˈtsjoːne ˈkaltʃo ˈmiːlan]), commonly referred to as A.C. Milan or simply Milan, is a professional football club in Milan, Italy, founded in 1899. The club has spent its entire history, with the exception of the 1980–81 and 1982–83 seasons, in the top flight of Italian football, known as Serie A since 1929–30. The club is one of the wealthiest in Italian and world football. It was a founding member of the now-defunct G-14 group of Europe&apos;s leading football clubs as well as its replacement, the European Club Association.</rdfs:comment>
        <rdfs:comment xml:lang="it">L&apos;Associazione Calcio Milan, meglio nota come A.C. Milan o anche Milan, è una società calcistica italiana fondata nel 1899 con sede nella città di Milano.</rdfs:comment>
        <rdfs:label xml:lang="en">A.C. Milan</rdfs:label>
        <rdfs:label xml:lang="it">AC Milan</rdfs:label>
    </owl:NamedIndividual>
    


    <!-- http://www.semanticweb.org/2021/ontologies/calcio#Alessio_Romagnoli -->

    <owl:NamedIndividual rdf:about="http://www.semanticweb.org/2021/ontologies/calcio#Alessio_Romagnoli">
        <giocaPer rdf:resource="http://www.semanticweb.org/2021/ontologies/calcio#ACMilan"/>
        <rdfs:comment xml:lang="en">Alessio Romagnoli (Italian pronunciation: [aˈlɛssjo romaɲˈɲɔːli]; born 12 January 1995) is an Italian professional footballer who plays as a centre back for Serie A club Milan, for which he is captain, and the Italian national team.</rdfs:comment>
        <rdfs:comment xml:lang="it">Alessio Romagnoli è un calciatore italiano, difensore del Milan, di cui è capitano, e della nazionale italiana.</rdfs:comment>
        <rdfs:label xml:lang="en">Alessio Romagnoli</rdfs:label>
        <rdfs:label xml:lang="it">Alessio Romagnoli</rdfs:label>
    </owl:NamedIndividual>
    


    <!-- http://www.semanticweb.org/2021/ontologies/calcio#Alexis_Saelemaekers -->

    <owl:NamedIndividual rdf:about="http://www.semanticweb.org/2021/ontologies/calcio#Alexis_Saelemaekers">
        <giocaPer rdf:resource="http://www.semanticweb.org/2021/ontologies/calcio#ACMilan"/>
        <rdfs:comment xml:lang="it">Alexis Jesse Saelemaekers (Berchem-Sainte-Agathe, 27 giugno 1999) è un calciatore belga, centrocampista del Milan e della nazionale belga.</rdfs:comment>
        <rdfs:comment xml:lang="en">Alexis Jesse Saelemaekers is a Belgian professional footballer who plays as a midfielder for Italian Serie A club Milan and Belgium national football team. Although he primarily plays in midfield, he can also play in defence.</rdfs:comment>
        <rdfs:label xml:lang="en">Alexis Saelemaekers</rdfs:label>
        <rdfs:label xml:lang="it">Alexis Saelemaekers</rdfs:label>
    </owl:NamedIndividual>
    


    <!-- http://www.semanticweb.org/2021/ontologies/calcio#Andrea_Conti -->

    <owl:NamedIndividual rdf:about="http://www.semanticweb.org/2021/ontologies/calcio#Andrea_Conti">
        <dataUltimoTrasferimento rdf:datatype="http://www.w3.org/2001/XMLSchema#dateTime">2021-01-20T00:00:00</dataUltimoTrasferimento>
        <rdfs:comment xml:lang="en">Andrea Conti (Italian pronunciation: [anˈdrɛːa ˈkonti]; born 2 March 1994) is an Italian professional footballer who plays as a right-back for Serie A club Parma, on loan from Milan, and the Italy national team.</rdfs:comment>
        <rdfs:comment xml:lang="it">Andrea Conti è un calciatore italiano, difensore del Parma in prestito dal Milan.</rdfs:comment>
        <rdfs:label xml:lang="en">Andrea Conti</rdfs:label>
        <rdfs:label xml:lang="it">Andrea Conti</rdfs:label>
    </owl:NamedIndividual>
    


    <!-- http://www.semanticweb.org/2021/ontologies/calcio#Andrea_Pirlo -->

    <owl:NamedIndividual rdf:about="http://www.semanticweb.org/2021/ontologies/calcio#Andrea_Pirlo">
        <allenaSquadra rdf:resource="http://www.semanticweb.org/2021/ontologies/calcio#Juventus"/>
        <rdfs:comment xml:lang="it">Andrea Pirlo (Flero, 19 maggio 1979) è un allenatore di calcio ed ex calciatore italiano, di ruolo centrocampista, tecnico della Juventus, campione del mondo nel 2006 e vicecampione d&apos;Europa nel 2012 con la nazionale italiana.</rdfs:comment>
        <rdfs:comment xml:lang="en">Andrea Pirlo (Italian pronunciation: [anˈdrɛːa ˈpirlo]; born 19 May 1979) is an Italian professional football coach and former player who is the head coach of Serie A club Juventus. Considered to be one of the greatest deep-lying playmakers of all time, Pirlo was renowned for his vision, ball control, technique, creativity, passing, and free-kick ability.</rdfs:comment>
        <rdfs:label xml:lang="en">Andrea Pirlo</rdfs:label>
        <rdfs:label xml:lang="it">Andrea Pirlo</rdfs:label>
    </owl:NamedIndividual>
    


    <!-- http://www.semanticweb.org/2021/ontologies/calcio#Anfield -->

    <owl:NamedIndividual rdf:about="http://www.semanticweb.org/2021/ontologies/calcio#Anfield">
        <rdf:type rdf:resource="http://www.semanticweb.org/2021/ontologies/calcio#Stadio"/>
        <haCapienza rdf:datatype="http://www.w3.org/2001/XMLSchema#integer">53394</haCapienza>
        <rdfs:comment xml:lang="en">Anfield is a football stadium in Anfield, Liverpool, Merseyside, England, which has a seating capacity of 53,394, making it the seventh largest football stadium in England. It has been the home of Liverpool Football Club since their formation in 1892.</rdfs:comment>
        <rdfs:comment xml:lang="it">Anfield è uno stadio calcistico inglese di Liverpool, che dal 1892 ospita le gare casalinghe del Liverpool Football Club. Prende il nome da una spianata costeggiata da una strada nota come Anfield Road, in seguito di molto ridotta in quanto nel 1992 fu occupata dall&apos;ampliamento di una tribuna oggi nota come Anfield Road Stand.</rdfs:comment>
        <rdfs:label xml:lang="en">Anfield</rdfs:label>
        <rdfs:label xml:lang="it">Anfield</rdfs:label>
    </owl:NamedIndividual>
    


    <!-- http://www.semanticweb.org/2021/ontologies/calcio#Ansu_Fati -->

    <owl:NamedIndividual rdf:about="http://www.semanticweb.org/2021/ontologies/calcio#Ansu_Fati">
        <compagnoDi rdf:resource="http://www.semanticweb.org/2021/ontologies/calcio#Antoine_Griezmann"/>
        <rdfs:comment xml:lang="en">Anssumane &quot;Ansu&quot; Fati Vieira (born 31 October 2002) is a Spanish professional footballer who plays as a left winger for Barcelona and the Spain national team. He was born in Guinea-Bissau but represents Spain internationally. He is widely considered one of Spain&apos;s most exciting football talents, and one of the best young players in the world.</rdfs:comment>
        <rdfs:comment xml:lang="it">Anssumane Fati Vieira, detto Ansu Fati, è un calciatore guineense naturalizzato spagnolo, attaccante del Barcellona e della nazionale spagnola.</rdfs:comment>
        <rdfs:comment xml:lang="en">Ansu Fati</rdfs:comment>
        <rdfs:label xml:lang="it">Ansu Fati</rdfs:label>
    </owl:NamedIndividual>
    


    <!-- http://www.semanticweb.org/2021/ontologies/calcio#Ante_Rebić -->

    <owl:NamedIndividual rdf:about="http://www.semanticweb.org/2021/ontologies/calcio#Ante_Rebić">
        <giocaPer rdf:resource="http://www.semanticweb.org/2021/ontologies/calcio#ACMilan"/>
        <rdfs:comment xml:lang="it">Ante Rebić</rdfs:comment>
        <rdfs:comment xml:lang="it">Ante Rebić (Spalato, 21 settembre 1993) è un calciatore croato, attaccante del Milan e della nazionale croata, con la quale si è laureato vice-campione del mondo nel 2018.</rdfs:comment>
        <rdfs:comment xml:lang="en">Ante Rebić is a Croatian professional footballer who plays as a winger for Serie A club Milan and the Croatia national team. He can play on both wings, as well as a second striker. He began his senior career at RNK Split, and in 2013 signed for Serie A club Fiorentina for an undisclosed fee.</rdfs:comment>
        <rdfs:label xml:lang="en">Ante Rebić</rdfs:label>
    </owl:NamedIndividual>
    


    <!-- http://www.semanticweb.org/2021/ontologies/calcio#Antoine_Griezmann -->

    <owl:NamedIndividual rdf:about="http://www.semanticweb.org/2021/ontologies/calcio#Antoine_Griezmann">
        <compagnoDi rdf:resource="http://www.semanticweb.org/2021/ontologies/calcio#Lionel_Messi"/>
        <rdfs:comment xml:lang="it">Antoine Griezmann (Mâcon, 21 marzo 1991) è un calciatore francese, attaccante del Barcellona e della nazionale francese, con cui si è laureato vicecampione d&apos;Europa nel 2016 e campione del mondo nel 2018.

Soprannominato Le petit diable, è considerato uno dei calciatori più forti al mondo, nel 2012 è stato inserito nella lista dei migliori calciatori nati dopo il 1991 stilata da Don Balón. È primatista di reti con l&apos;Atlético Madrid (27) nelle competizioni calcistiche europee.</rdfs:comment>
        <rdfs:comment xml:lang="en">Antoine Griezmann is a French professional footballer who plays as a forward for Spanish club Barcelona and the France national team.</rdfs:comment>
        <rdfs:label xml:lang="it">Antoine Griezmann</rdfs:label>
    </owl:NamedIndividual>
    


    <!-- http://www.semanticweb.org/2021/ontologies/calcio#Antonio_Conte -->

    <owl:NamedIndividual rdf:about="http://www.semanticweb.org/2021/ontologies/calcio#Antonio_Conte">
        <rdf:type rdf:resource="http://www.semanticweb.org/2021/ontologies/calcio#Allenatore"/>
        <rdfs:comment xml:lang="en">Antonio Conte is an Italian professional football manager and former player. He is the head coach at Serie A club Inter Milan.</rdfs:comment>
        <rdfs:comment xml:lang="it">Antonio Conte è un allenatore di calcio ed ex calciatore italiano, di ruolo centrocampista, tecnico dell&apos;Inter.</rdfs:comment>
        <rdfs:label xml:lang="en">Antonio Conte</rdfs:label>
        <rdfs:label xml:lang="it">Antonio Conte</rdfs:label>
    </owl:NamedIndividual>
    


    <!-- http://www.semanticweb.org/2021/ontologies/calcio#Argentina -->

    <owl:NamedIndividual rdf:about="http://www.semanticweb.org/2021/ontologies/calcio#Argentina">
        <rdf:type rdf:resource="http://www.semanticweb.org/2021/ontologies/calcio#squadraNazionale"/>
        <rdfs:comment xml:lang="it">La nazionale di calcio dell&apos;Argentina è la squadra di calcio che rappresenta l&apos;Argentina ed è posta sotto l&apos;egida della Asociación del Fútbol Argentino. Il palmarès della Selección o Albiceleste annovera 14 Coppe America e 2 Coppe del mondo.</rdfs:comment>
        <rdfs:comment xml:lang="en">The Argentina national football team (Spanish: Selección de fútbol de Argentina) represents Argentina in men&apos;s international football and is administered by the Argentine Football Association, the governing body for football in Argentina. Argentina&apos;s home stadium is Estadio Monumental Antonio Vespucio Liberti in Buenos Aires.</rdfs:comment>
        <rdfs:label xml:lang="en">Argentina national football team</rdfs:label>
        <rdfs:label xml:lang="it">Nazionale di calcio dell&apos;Argentina</rdfs:label>
    </owl:NamedIndividual>
    


    <!-- http://www.semanticweb.org/2021/ontologies/calcio#AtleticoMadrid -->

    <owl:NamedIndividual rdf:about="http://www.semanticweb.org/2021/ontologies/calcio#AtleticoMadrid">
        <rdf:type rdf:resource="http://www.semanticweb.org/2021/ontologies/calcio#squadraDiClub"/>
        <rdfs:comment xml:lang="en">Club Atlético de Madrid, S.A.D., commonly referred to as Atlético de Madrid in English or simply as Atlético, Atléti, or Atleti, is a Spanish professional football club based in Madrid, that play in La Liga. The club play their home games at the Wanda Metropolitano Stadium, which has a capacity of 68,456.</rdfs:comment>
        <rdfs:comment xml:lang="it">Il Club Atlético de Madrid, conosciuto come Atlético Madrid (in Spagna anche come Atleti), è una società calcistica spagnola con sede a Madrid e milita in Primera División, la divisione di vertice del campionato spagnolo di calcio.</rdfs:comment>
        <rdfs:label xml:lang="en">Atlético Madrid</rdfs:label>
        <rdfs:label xml:lang="it">Club Atlético de Madrid</rdfs:label>
    </owl:NamedIndividual>
    


    <!-- http://www.semanticweb.org/2021/ontologies/calcio#Barcellona -->

    <owl:NamedIndividual rdf:about="http://www.semanticweb.org/2021/ontologies/calcio#Barcellona">
        <owl:sameAs rdf:resource="http://www.wikidata.org/entity/Q7156"/>
        <appartieneALega rdf:resource="http://www.semanticweb.org/2021/ontologies/calcio#LaLiga"/>
        <detieneCalciatore rdf:resource="http://www.semanticweb.org/2021/ontologies/calcio#Lionel_Messi"/>
        <giocaInStadio rdf:resource="http://www.semanticweb.org/2021/ontologies/calcio#Camp_Nou"/>
        <èAllenataDa rdf:resource="http://www.semanticweb.org/2021/ontologies/calcio#Ronald_Koeman"/>
        <rdfs:comment xml:lang="en">Futbol Club Barcelona, commonly referred to as Barcelona and colloquially known as Barça, is a Spanish professional football club based in Barcelona, that competes in La Liga, the top flight of Spanish football</rdfs:comment>
        <rdfs:comment xml:lang="it">Il Futbol Club Barcelona (pronuncia spagnola: [ˈfutβol ˌkluβ baɾθeˈlona], catalana: [fuδˈβɔɫ ˌklup bəɾsəˈlonə]), conosciuto semplicemente come Barcelona (spesso abbreviato in Barça, pronuncia spagnola: [ˈbaɾθa], catalana: [ˈbaɾsə]) e in italiano come Barcellona, è una società polisportiva spagnola con sede nella città di Barcellona, nota soprattutto per la sua sezione calcistica. Fu fondata a Barcellona nel 1899 da un gruppo di calciatori svizzeri e britannici guidati da Hans Gamper.</rdfs:comment>
        <rdfs:label xml:lang="en">FC Barcellona</rdfs:label>
        <rdfs:label xml:lang="it">Futbol Club Barcelona</rdfs:label>
    </owl:NamedIndividual>
    


    <!-- http://www.semanticweb.org/2021/ontologies/calcio#BayernMonaco -->

    <owl:NamedIndividual rdf:about="http://www.semanticweb.org/2021/ontologies/calcio#BayernMonaco">
        <rdf:type rdf:resource="http://www.semanticweb.org/2021/ontologies/calcio#Squadra"/>
        <appartieneALega rdf:resource="http://www.semanticweb.org/2021/ontologies/calcio#Bundesliga"/>
        <rdfs:comment xml:lang="en">Fußball-Club Bayern München e.V. (German pronunciation: [ˈfuːsbalˌklʊp ˈbaɪɐn ˈmʏnçn̩]), commonly known as FC Bayern München (German pronunciation: [ʔɛf tseː ˈbaɪɐn ˈmʏnçn̩]), FCB, Bayern Munich, or FC Bayern, is a German professional sports club based in Munich, Bavaria. It is best known for its professional football team, which plays in the Bundesliga, the top tier of the German football league system, and is the most successful club in German football history, having won a record 30 national titles, including eight consecutively since 2013, and 20 national cups, along with numerous European honours.</rdfs:comment>
        <rdfs:comment xml:lang="it">Il Fußball-Club Bayern München AG, noto internazionalmente come Bayern München e in lingua italiana come Bayern Monaco, è una società polisportiva tedesca avente sede a Monaco di Baviera, celebre per la propria sezione calcistica, che milita nella Bundesliga, la massima divisione del campionato tedesco di calcio. Fondata nel 1900 da alcuni membri del MTV 1879 München, la polisportiva comprende sezioni di scacchi, pallavolo, pallacanestro, ginnastica, pallamano, bowling, tennis tavolo e squadre di calcio. È il club sportivo con il maggior numero di affiliati al mondo (293 000 al novembre 2019).</rdfs:comment>
        <rdfs:label xml:lang="en">FC Bayern Munich</rdfs:label>
        <rdfs:label xml:lang="it">Fußball-Club Bayern München</rdfs:label>
    </owl:NamedIndividual>
    


    <!-- http://www.semanticweb.org/2021/ontologies/calcio#BorussiaDortmund -->

    <owl:NamedIndividual rdf:about="http://www.semanticweb.org/2021/ontologies/calcio#BorussiaDortmund">
        <appartieneALega rdf:resource="http://www.semanticweb.org/2021/ontologies/calcio#Bundesliga"/>
        <rdfs:comment xml:lang="en">Ballspielverein Borussia 09 e.V. Dortmund, commonly known as Borussia Dortmund [boˈʁʊsi̯aː ˈdɔɐ̯tmʊnt],[2] BVB, or simply Dortmund, is a German professional sports club based in Dortmund, North Rhine-Westphalia. It is best known for its men&apos;s professional football team, which plays in the Bundesliga, the top tier of the German football league system. The club have won eight league championships, four DFB-Pokals, one UEFA Champions League, one Intercontinental Cup, and one UEFA Cup Winners&apos; Cup.</rdfs:comment>
        <rdfs:comment xml:lang="it">Il Ballspielverein Borussia 09 e.V. Dortmund, meglio noto come Borussia Dortmund o con la sigla BVB, è una società polisportiva tedesca con sede nella città di Dortmund. È nota soprattutto per la sua sezione calcistica, che milita nella Bundesliga, la divisione di vertice del campionato tedesco di calcio.</rdfs:comment>
        <rdfs:label xml:lang="it">BV Borussia 09 Dortmund</rdfs:label>
        <rdfs:label xml:lang="en">Borussia Dortmund</rdfs:label>
    </owl:NamedIndividual>
    


    <!-- http://www.semanticweb.org/2021/ontologies/calcio#Brahim_Díaz -->

    <owl:NamedIndividual rdf:about="http://www.semanticweb.org/2021/ontologies/calcio#Brahim_Díaz">
        <giocaPer rdf:resource="http://www.semanticweb.org/2021/ontologies/calcio#ACMilan"/>
        <rdfs:comment xml:lang="it">Brahim Abdelkader Díaz (Malaga, 3 agosto 1999) è un calciatore spagnolo di origini marocchine, centrocampista o attaccante del Milan, in prestito dal Real Madrid e della nazionale Under-21 spagnola.</rdfs:comment>
        <rdfs:comment xml:lang="en">Brahim Abdelkader Díaz (Spanish pronunciation: [bɾaˈin ˈdi.aθ]; born 3 August 1999), known as Brahim,[2] is a Spanish professional footballer who plays as a forward for Serie A club Milan, on loan from Real Madrid of La Liga.</rdfs:comment>
        <rdfs:label xml:lang="en">Brahim Díaz</rdfs:label>
        <rdfs:label xml:lang="it">Brahim Díaz</rdfs:label>
    </owl:NamedIndividual>
    


    <!-- http://www.semanticweb.org/2021/ontologies/calcio#Brasile -->

    <owl:NamedIndividual rdf:about="http://www.semanticweb.org/2021/ontologies/calcio#Brasile">
        <rdf:type rdf:resource="http://www.semanticweb.org/2021/ontologies/calcio#Squadra"/>
        <rdfs:comment xml:lang="it">La nazionale di calcio del Brasile (port. Seleção Brasileira de Futebol, per questo nota informalmente come Seleção) è la rappresentativa calcistica del Brasile ed è posta sotto l&apos;egida della Confederação Brasileira de Futebol.</rdfs:comment>
        <rdfs:comment xml:lang="en">The Brazil national football team (Portuguese: Seleção Brasileira de Futebol) represents Brazil in men&apos;s international football and is administered by the Brazilian Football Confederation (CBF), the governing body for football in Brazil. They have been a member of FIFA since 1923 and a member of CONMEBOL since 1916.</rdfs:comment>
        <rdfs:label xml:lang="en">Brazil national football team</rdfs:label>
        <rdfs:label xml:lang="it">Nazionale di calcio del Brasile</rdfs:label>
    </owl:NamedIndividual>
    


    <!-- http://www.semanticweb.org/2021/ontologies/calcio#Bundesliga -->

    <owl:NamedIndividual rdf:about="http://www.semanticweb.org/2021/ontologies/calcio#Bundesliga">
        <rdfs:comment xml:lang="it">La 1. Fußball-Bundesliga (dal tedesco: Prima lega calcistica federale), nota semplicemente come Bundesliga, è la massima serie professionistica del campionato tedesco di calcio. Dipende organizzativamente dalla Deutsche Fußball Liga GmbH e disciplinarmente dalla Deutscher Fußball-Bund, la federcalcio tedesca. Comprende attualmente 18 squadre.</rdfs:comment>
        <rdfs:comment xml:lang="en">The Bundesliga (German: [ˈbʊndəsˌliːɡa] (About this soundlisten); lit. &apos;Federal League&apos;), sometimes referred to as the Fußball-Bundesliga ([ˌfuːsbal-]) or 1. Bundesliga ([ˌeːɐ̯stə-]), is a professional association football league in Germany. At the top of the German football league system, the Bundesliga is Germany&apos;s primary football competition. The Bundesliga comprises 18 teams and operates on a system of promotion and relegation with the 2. Bundesliga. Seasons run from August to May. Most games are played on Saturdays and Sundays, with a few games played on weekdays. All of the Bundesliga clubs qualify for the DFB-Pokal. The winner of the Bundesliga qualifies for the DFL-Supercup.</rdfs:comment>
        <rdfs:label xml:lang="en">Bundesliga</rdfs:label>
        <rdfs:label xml:lang="it">Bundesliga</rdfs:label>
    </owl:NamedIndividual>
    


    <!-- http://www.semanticweb.org/2021/ontologies/calcio#Camp_Nou -->

    <owl:NamedIndividual rdf:about="http://www.semanticweb.org/2021/ontologies/calcio#Camp_Nou">
        <haCapienza rdf:datatype="http://www.w3.org/2001/XMLSchema#integer">99354</haCapienza>
        <rdfs:comment xml:lang="en">Camp Nou (Catalan pronunciation: [ˌkamˈnɔw], meaning new field, often referred to in English as the Nou Camp)[5][6] is a football stadium in Barcelona, Spain. It opened in 1957 and has been the home stadium of FC Barcelona since its completion.</rdfs:comment>
        <rdfs:comment xml:lang="it">Il Camp Nou è un impianto calcistico ubicato nel quartiere Les Corts della città spagnola di Barcellona.

Di proprietà del Futbol Club Barcelona, ospita gli incontri casalinghi della sua prima squadra dal 1957. Con una capacità di 99 354 spettatori, è l&apos;impianto più capiente di Spagna e d&apos;Europa[1], davanti al nuovo Wembley di Londra (90 000) e allo stadio San Siro di Milano (81 277).</rdfs:comment>
        <rdfs:label xml:lang="en">Camp Nou</rdfs:label>
        <rdfs:label xml:lang="it">Camp Nou</rdfs:label>
    </owl:NamedIndividual>
    


    <!-- http://www.semanticweb.org/2021/ontologies/calcio#ChampionsLeague_2003 -->

    <owl:NamedIndividual rdf:about="http://www.semanticweb.org/2021/ontologies/calcio#ChampionsLeague_2003">
        <trofeoHaNome rdf:datatype="http://www.w3.org/2001/XMLSchema#string">UEFA Champions League 2002-2003</trofeoHaNome>
        <rdfs:comment xml:lang="it">La UEFA Champions League 2002-2003 fu la 48ª edizione della massima competizione calcistica per club europei maschili.

La coppa fu vinta dal Milan, che affrontò in finale una storica rivale, la Juventus, nella prima finale del torneo tra due squadre italiane. I rossoneri si imposero sui bianconeri per 3-2 ai rigori. Per il Milan fu la sesta vittoria nella massima competizione europea e la prima dopo nove anni. I detentori del Real Madrid furono eliminati in semifinale dalla Juventus.

Per il secondo anno di fila capocannoniere del torneo fu l&apos;olandese Ruud van Nistelrooy del Manchester Utd, autore di 12 reti (più 2 nei turni preliminari).</rdfs:comment>
        <rdfs:comment xml:lang="en">The 2002–03 UEFA Champions League was the 11th season of UEFA&apos;s premier European club football tournament, the UEFA Champions League, since its rebranding in 1992, and the 48th European Cup tournament overall. The competition was won by Milan, who beat Juventus on penalties in the European Cup&apos;s first ever all-Italian final, to win their sixth European title, and its first in nine years. Manchester United&apos;s Ruud van Nistelrooy was again the top scorer, scoring 12 goals over the two group stages and knockout stage, in addition to two goals he had scored in the qualifying phase, although his side bowed out in the quarter-finals and missed out on the chance of playing in a final at their own stadium.

Real Madrid were the defending champions, but were eliminated by Juventus in the semi-finals.</rdfs:comment>
        <rdfs:label xml:lang="en">2002–03 UEFA Champions League</rdfs:label>
        <rdfs:label xml:lang="it">UEFA Champions League 2002-2003</rdfs:label>
    </owl:NamedIndividual>
    


    <!-- http://www.semanticweb.org/2021/ontologies/calcio#ChampionsLeague_2007 -->

    <owl:NamedIndividual rdf:about="http://www.semanticweb.org/2021/ontologies/calcio#ChampionsLeague_2007">
        <rdf:type rdf:resource="http://www.semanticweb.org/2021/ontologies/calcio#trofeoDiClub"/>
        <trofeoHaNome rdf:datatype="http://www.w3.org/2001/XMLSchema#string">UEFA Champions League 2006-2007</trofeoHaNome>
        <rdfs:comment xml:lang="it">La UEFA Champions League 2006-2007 è stata la 52ª edizione, la 15ª con la denominazione attuale, del massimo torneo di calcio europeo per squadre di club maggiori maschili organizzato dall&apos;UEFA.

Il trofeo è stato vinto dal Milan, che nella finale disputata il 23 maggio 2007 allo Stadio Olimpico di Atene ha battuto il Liverpool per 2-1 con una doppietta di Filippo Inzaghi, cui ha fatto seguito un gol di Dirk Kuijt.

Come squadra vincitrice, il Milan ha ottenuto anche il diritto di partecipare alla Supercoppa UEFA 2007 e alla Coppa del mondo per club FIFA 2007.</rdfs:comment>
        <rdfs:comment xml:lang="en">The 2006–07 UEFA Champions League was the 15th season of UEFA&apos;s premier European club football tournament, the UEFA Champions League, since it was rebranded from the European Cup, and the 52nd season overall. The final was contested by Milan and Liverpool on 23 May 2007. Beforehand, the match was billed as a repeat of the 2005 final, the only difference being that the 2007 final was to be played at the Olympic Stadium in Athens, Greece. Milan won the match 2–1 to claim their seventh European Cup, with both goals coming from Filippo Inzaghi. Dirk Kuyt scored for Liverpool.

Barcelona were the defending champions, but were eliminated by Liverpool in the first knockout round.</rdfs:comment>
        <rdfs:label xml:lang="en">2006–07 UEFA Champions League</rdfs:label>
        <rdfs:label xml:lang="it">UEFA Champions League 2006-2007</rdfs:label>
    </owl:NamedIndividual>
    


    <!-- http://www.semanticweb.org/2021/ontologies/calcio#ChampionsLeague_63 -->

    <owl:NamedIndividual rdf:about="http://www.semanticweb.org/2021/ontologies/calcio#ChampionsLeague_63">
        <rdf:type rdf:resource="http://www.semanticweb.org/2021/ontologies/calcio#trofeoDiClub"/>
        <rdfs:comment xml:lang="it">La Coppa dei Campioni 1962-1963, ottava edizione del torneo, vede la partecipazione di 30 squadre, tra cui per la prima volta i campioni dell’Albania. Il torneo venne vinto dal Milan, che sconfisse in finale i portoghesi del Benfica, vincitori delle ultime due edizioni e divenne la prima squadra italiana a vincere il trofeo.</rdfs:comment>
        <rdfs:comment xml:lang="en">The 1962–63 European Cup was the eighth season of the European Cup, a football competition for European clubs. The competition was won by Milan, who beat two-time defending champions Benfica in the final at Wembley Stadium in London. Milan&apos;s victory was the first by an Italian club.

Albania entered its champion for the first time this season</rdfs:comment>
        <rdfs:label xml:lang="en">1962–63 European Cup</rdfs:label>
        <rdfs:label xml:lang="it">Coppa dei Campioni 1962-1963</rdfs:label>
    </owl:NamedIndividual>
    


    <!-- http://www.semanticweb.org/2021/ontologies/calcio#ChampionsLeague_69 -->

    <owl:NamedIndividual rdf:about="http://www.semanticweb.org/2021/ontologies/calcio#ChampionsLeague_69">
        <rdf:type rdf:resource="http://www.semanticweb.org/2021/ontologies/calcio#trofeoDiClub"/>
        <rdfs:comment xml:lang="it">La stagione 1968-1969 è stata la quattordicesima edizione della Coppa dei Campioni, massima competizione organizzata dalla UEFA. Essa vide la partecipazione di 27 squadre.</rdfs:comment>
        <rdfs:comment xml:lang="en">The 1968–69 season of the European Cup football club tournament was won by Milan, who beat Ajax 4–1 in the final, giving Milan its first European Cup title since 1963, and its second overall. A number of Eastern Bloc clubs withdrew from the first two rounds when UEFA paired up all of the Eastern Bloc clubs against one another in the aftermath of the Soviet invasion of Czechoslovakia.

Substitutions of two players at any game time were allowed; obligatory match dates were introduced (two weeks between the legs) and fixed on Wednesdays; the away goal rule was extended to the first and second rounds.

Manchester United, the defending champions, were eliminated by Milan in the semi-finals.</rdfs:comment>
        <rdfs:label xml:lang="en">1968–69 European Cup</rdfs:label>
        <rdfs:label xml:lang="it">Coppa dei Campioni 1968-1969</rdfs:label>
    </owl:NamedIndividual>
    


    <!-- http://www.semanticweb.org/2021/ontologies/calcio#ChampionsLeague_89 -->

    <owl:NamedIndividual rdf:about="http://www.semanticweb.org/2021/ontologies/calcio#ChampionsLeague_89">
        <rdf:type rdf:resource="http://www.semanticweb.org/2021/ontologies/calcio#trofeoDiClub"/>
        <rdfs:comment xml:lang="it">La Coppa dei Campioni 1988-1989, trentaquattresima edizione del torneo, vide la partecipazione di 31 squadre. Il torneo venne vinto per la terza volta dal Milan, che sconfisse in finale la Steaua Bucarest a sedici anni dal suo ultimo successo internazionale, e a venti dal suo ultimo titolo continentale.</rdfs:comment>
        <rdfs:comment xml:lang="en">The 1988–89 European Cup was the 34th season of the European Cup football club tournament. The competition was won for the first time since 1969, and third time overall, by Milan comfortably in the final against former winners Steaua București.

As the defending champions, PSV Eindhoven received a bye to the second round, but were eliminated by Real Madrid in the quarter-finals. English clubs were still banned, following the Heysel Stadium disaster of 1985, so Liverpool were denied a place in the competition.</rdfs:comment>
        <rdfs:label xml:lang="en">1988–89 European Cup</rdfs:label>
        <rdfs:label xml:lang="it">Coppa dei Campioni 1988-1989</rdfs:label>
    </owl:NamedIndividual>
    


    <!-- http://www.semanticweb.org/2021/ontologies/calcio#ChampionsLeague_90 -->

    <owl:NamedIndividual rdf:about="http://www.semanticweb.org/2021/ontologies/calcio#ChampionsLeague_90">
        <rdf:type rdf:resource="http://www.semanticweb.org/2021/ontologies/calcio#trofeoDiClub"/>
        <rdfs:comment xml:lang="it">La Coppa dei Campioni 1989-1990, trentacinquesima edizione del torneo, vede la partecipazione di 32 squadre. Il torneo fu vinto per la quarta volta dal Milan, che sconfisse in finale il Benfica. Fu l’ultima volta che dei campioni in carica riuscirono a difendere il titolo fino al 2017.</rdfs:comment>
        <rdfs:comment xml:lang="en">The 1989–90 European Cup was the 35th edition of Europe&apos;s premier club football tournament, the European Cup. The final was played at the Praterstadion in Vienna on 23 May 1990. The final was contested by Italian defending champions Milan and Portuguese two-time former winners Benfica. Milan successfully defended their title with a 1–0 victory, securing their fourth European Cup trophy. Milan remained the last team to successfully defend their trophy until Real Madrid did it again in 2017. Arsenal were denied a place in the competition, as this was the last year of a ban from European competitions for English clubs following the Heysel Stadium disaster of 1985.</rdfs:comment>
        <rdfs:label xml:lang="en">1989–90 European Cup</rdfs:label>
        <rdfs:label xml:lang="it">Coppa dei Campioni 1989-1990</rdfs:label>
    </owl:NamedIndividual>
    


    <!-- http://www.semanticweb.org/2021/ontologies/calcio#ChampionsLeague_94 -->

    <owl:NamedIndividual rdf:about="http://www.semanticweb.org/2021/ontologies/calcio#ChampionsLeague_94">
        <rdf:type rdf:resource="http://www.semanticweb.org/2021/ontologies/calcio#trofeoDiClub"/>
        <trofeoHaNome rdf:datatype="http://www.w3.org/2001/XMLSchema#string">UEFA Champions League 1993-1994</trofeoHaNome>
        <rdfs:comment xml:lang="it">La UEFA Champions League 1993-1994 fu la trentanovesima edizione della massima competizione continentale di calcio. Fu vinta dal Milan, che sconfisse in finale il Barcellona di Johan Cruijff per 4-0 ad Atene, aggiudicandosi la quinta Coppa dei Campioni della propria storia dopo aver perso la finale dell&apos;anno prima contro l&apos;Olympique Marsiglia.

Per la prima volta nella storia del torneo, la squadra campione uscente, nello specifico l&apos;Olympique Marsiglia, non partecipò alla manifestazione. Il club francese fu, infatti, sostituito dal Monaco a causa della squalifica per illecito sportivo (coinvolgimento nell&apos;affaire VA-OM).

La vittoria del Milan in finale rappresenta il più ampio scarto in una finale di UEFA Champions League. Per i rossoneri fu il quinto trionfo nella competizione.</rdfs:comment>
        <rdfs:comment xml:lang="en">The 1993–94 UEFA Champions League was the 39th season of the UEFA Champions League, UEFA&apos;s premier club football tournament, and the second season with the UEFA Champions League logo (it was adopted in the group stage and semi-finals, the rest of the tournament continued to be called &quot;European Champion Clubs&apos; Cup&quot; or &quot;European Cup&quot;). The competition was won by Milan, their fifth title, beating Barcelona 4–0 in the final. Marseille were the defending champions, but were not allowed to enter the competition due their involvement in a match-fixing scandal in Division 1 the season prior. This saw them stripped of their league title and demoted to Division 2 at the end of 1993–94. This was the first and only time which the defending champions did not participate in the following season of the competition. Third-placed Monaco took the vacated French berth (second-placed Paris Saint-Germain, who refused the defaulted French title, competed in the Cup Winners&apos; Cup instead as Coupe de France winners).</rdfs:comment>
        <rdfs:label xml:lang="en">1993–94 UEFA Champions League</rdfs:label>
        <rdfs:label xml:lang="it">UEFA Champions League 1993-1994</rdfs:label>
    </owl:NamedIndividual>
    


    <!-- http://www.semanticweb.org/2021/ontologies/calcio#Championship -->

    <owl:NamedIndividual rdf:about="http://www.semanticweb.org/2021/ontologies/calcio#Championship">
        <rdfs:comment xml:lang="it">La Football League Championship, nota anche come Sky Bet Championship per motivi di sponsorizzazione, è la seconda divisione del campionato di calcio inglese. Rappresenta il massimo livello della Football League, dato che la Premier League (prima divisione inglese) non ne fa parte.</rdfs:comment>
        <rdfs:comment xml:lang="en">The English Football League Championship (often referred to as the Championship for short or the Sky Bet Championship for sponsorship reasons, and known as the Football League Championship from 2004 until 2016)[1] is the highest division of the English Football League (EFL) and second-highest overall in the English football league system after the Premier League. The league is contested by 24 clubs. Each season, the two top-finishing teams in the Championship are automatically promoted to the Premier League. The teams that finish the season in 3rd to 6th place enter a playoff tournament, with the winner also gaining promotion to the Premier League. The three lowest-finishing teams in the Championship are relegated to League One.</rdfs:comment>
        <rdfs:label xml:lang="en">EFL Championship</rdfs:label>
        <rdfs:label xml:lang="it">Football League Championship</rdfs:label>
    </owl:NamedIndividual>
    


    <!-- http://www.semanticweb.org/2021/ontologies/calcio#Chelsea -->

    <owl:NamedIndividual rdf:about="http://www.semanticweb.org/2021/ontologies/calcio#Chelsea">
        <rdf:type rdf:resource="http://www.semanticweb.org/2021/ontologies/calcio#Squadra"/>
        <appartieneALega rdf:resource="http://www.semanticweb.org/2021/ontologies/calcio#PremierLeague"/>
        <rdfs:comment xml:lang="en">Chelsea Football Club is an English professional football club based in Fulham, London. Founded in 1905, the club competes in the Premier League, the top division of English football. Chelsea are among England&apos;s most successful clubs, having won over thirty competitive honours, including six league titles and six European trophies. Their home ground is Stamford Bridge.[4]</rdfs:comment>
        <rdfs:comment xml:lang="it">Il Chelsea Football Club, noto semplicemente come Chelsea (pron. &apos;tʃɛlsi), è una società calcistica inglese con sede nella città di Londra, nel borgo di Hammersmith e Fulham, militante nella massima serie del campionato inglese dalla stagione 1989-1990.</rdfs:comment>
        <rdfs:label xml:lang="en">Chelsea F.C.</rdfs:label>
        <rdfs:label xml:lang="it">Chelsea Football Club</rdfs:label>
    </owl:NamedIndividual>
    


    <!-- http://www.semanticweb.org/2021/ontologies/calcio#CopaDelRey -->

    <owl:NamedIndividual rdf:about="http://www.semanticweb.org/2021/ontologies/calcio#CopaDelRey">
        <rdf:type rdf:resource="http://www.semanticweb.org/2021/ontologies/calcio#Trofeo"/>
        <rdfs:comment xml:lang="it">La Coppa del Re (in spagnolo Copa del Rey, per esteso Campeonato de España - Copa de Su Majestad el Rey), nota anche come Coppa di Spagna, è la coppa nazionale calcistica spagnola riservata alle squadre professionistiche spagnole militanti nelle divisioni del campionato spagnolo.</rdfs:comment>
        <rdfs:comment xml:lang="en">The Campeonato de España–Copa de Su Majestad el Rey,[a] commonly known as Copa del Rey[b] or simply La Copa[c] and formerly known as Copa del Generalísimo (1939–76), is an annual knockout football competition in Spanish football, organized by the Royal Spanish Football Federation.</rdfs:comment>
        <rdfs:label xml:lang="en">Copa del Rey</rdfs:label>
        <rdfs:label xml:lang="it">Coppa del Re</rdfs:label>
    </owl:NamedIndividual>
    


    <!-- http://www.semanticweb.org/2021/ontologies/calcio#CoppaItalia -->

    <owl:NamedIndividual rdf:about="http://www.semanticweb.org/2021/ontologies/calcio#CoppaItalia">
        <rdf:type rdf:resource="http://www.semanticweb.org/2021/ontologies/calcio#trofeoDiClub"/>
        <rdfs:comment xml:lang="it">La Coppa Italia è la principale coppa calcistica italiana, nonché la seconda competizione professionistica nazionale per prestigio dopo il campionato di lega. Il torneo si tiene sotto la giurisdizione della FIGC ed è riconosciuto di fatto come una &quot;coppa federale&quot;, in maniera analoga alla FA Cup inglese, sebbene sia dal punto di vista organizzativo una &quot;coppa di lega&quot;, similarmente all&apos;English Football League Cup. La squadra detentrice della Coppa Italia può sfoggiare sulle proprie divise ufficiali, per i dodici mesi successivi la conquista del trofeo, la coccarda italiana tricolore come simbolo identificativo dell&apos;avvenuta vittoria.</rdfs:comment>
        <rdfs:comment xml:lang="en">The Coppa Italia (English: Italy Cup) is an Italian football annual cup competition. Its first edition was held in 1922 and was won by Vado. The second tournament, scheduled in the 1926–27 season, was cancelled during the round of 32. The third edition was not held until 1935–36 when it started being scheduled annually. The events of World War II interrupted the tournament after the 1942–43 season, and it did not resume again until 1958. Since then, it has been played every year.</rdfs:comment>
        <rdfs:label xml:lang="en">Coppa Italia</rdfs:label>
        <rdfs:label xml:lang="it">Coppa Italia</rdfs:label>
    </owl:NamedIndividual>
    


    <!-- http://www.semanticweb.org/2021/ontologies/calcio#CoupeDeFrance -->

    <owl:NamedIndividual rdf:about="http://www.semanticweb.org/2021/ontologies/calcio#CoupeDeFrance">
        <rdf:type rdf:resource="http://www.semanticweb.org/2021/ontologies/calcio#trofeoDiClub"/>
        <rdfs:comment xml:lang="it">La Coppa di Francia (in francese Coupe de France) è la coppa nazionale di calcio francese. Assegnata dalla Fédération Française de Football, la competizione è aperta a tutte le squadre calcistiche francesi (professionistiche e amatoriali) affiliate alla federazione. La vincitrice si qualifica di diritto alla fase a gironi di Europa League.</rdfs:comment>
        <rdfs:comment xml:lang="en">The Coupe de France, also known as the Coupe Charles Simon, is the premier knockout cup competition in French football organized by the French Football Federation (FFF). It was first held in 1917 and is open to all amateur and professional football clubs in France, including clubs based in the overseas departments and territories. Between 1917 and 1919, the competition was called the Coupe Charles Simon, in tribute of Charles Simon, a French sportsman and the founder of the French Interfederal Committee (the ancestor of the French Football Federation), who died in 1915 while serving in World War I. The final is played at the Stade de France and the winner qualifies for the group stage of the UEFA Europa League and a place in the Trophée des Champions match. A concurrent women&apos;s tournament is also held, the Coupe de France Féminine.</rdfs:comment>
        <rdfs:label xml:lang="it">Coppa di Francia</rdfs:label>
        <rdfs:label xml:lang="en">Coupe de France</rdfs:label>
    </owl:NamedIndividual>
    


    <!-- http://www.semanticweb.org/2021/ontologies/calcio#Cristiano_Ronaldo -->

    <owl:NamedIndividual rdf:about="http://www.semanticweb.org/2021/ontologies/calcio#Cristiano_Ronaldo">
        <giocaPer rdf:resource="http://www.semanticweb.org/2021/ontologies/calcio#Juventus"/>
        <haRuolo rdf:resource="http://www.semanticweb.org/2021/ontologies/calcio#attaccanteJuventus"/>
        <haEtà rdf:datatype="http://www.w3.org/2001/XMLSchema#integer">35</haEtà>
        <haNazionalità>Portogallo</haNazionalità>
        <stipendioCorrente rdf:datatype="http://www.w3.org/2001/XMLSchema#long">60000000</stipendioCorrente>
        <rdfs:comment xml:lang="en">Cristiano Ronaldo dos Santos Aveiro GOIH ComM (Portuguese pronunciation: [kɾiʃˈtjɐnu ʁɔˈnaɫdu]; born 5 February 1985) is a Portuguese professional footballer who plays as a forward for Serie A club Juventus and captains the Portugal national team. Often considered the best player in the world and widely regarded as one of the greatest players of all time, Ronaldo has won five Ballon d&apos;Or awards[note 3] and four European Golden Shoes, both of which are records for a European player. He has won 31 major trophies in his career, including seven league titles, five UEFA Champions Leagues, one UEFA European Championship, and one UEFA Nations League title. Ronaldo holds the records for the most goals (134) and assists (41) in the history of the UEFA Champions League.[11] He is one of the few recorded players to have made over 1,000 professional career appearances and has scored over 750 senior career goals for club and country.[12] He is also the second male to score 100 international goals, and the first European man to achieve the feat.[13]</rdfs:comment>
        <rdfs:comment xml:lang="it">Cristiano Ronaldo dos Santos Aveiro, meglio noto come Cristiano Ronaldo (pronuncia portoghese [kɾɨʃˈtjɐnu ʁuˈnaɫdu]; Funchal, 5 febbraio 1985), è un calciatore portoghese, attaccante della Juventus e della nazionale portoghese, della quale è capitano. Con quest&apos;ultima si è laureato vice-campione d&apos;Europa nel 2004 e campione d&apos;Europa nel 2016 vincendo anche la UEFA Nations League 2018-2019.</rdfs:comment>
        <rdfs:label xml:lang="en">Cristiano Ronaldo</rdfs:label>
        <rdfs:label xml:lang="it">Cristiano Ronaldo</rdfs:label>
    </owl:NamedIndividual>
    


    <!-- http://www.semanticweb.org/2021/ontologies/calcio#DFB-Pokal -->

    <owl:NamedIndividual rdf:about="http://www.semanticweb.org/2021/ontologies/calcio#DFB-Pokal">
        <rdf:type rdf:resource="http://www.semanticweb.org/2021/ontologies/calcio#trofeoDiClub"/>
        <rdfs:comment xml:lang="it">La Coppa di Germania, il cui nome ufficiale in tedesco è DFB-Pokal (dalle iniziali di Deutscher Fußball Bund Pokal, cioè Coppa della Federazione calcistica tedesca) è un torneo calcistico ad eliminazione diretta che si svolge in Germania con cadenza annuale. È il secondo trofeo nazionale per importanza dopo la Bundesliga. Il vincitore si qualifica per il DFL-Supercup e la UEFA Europa League, a meno che non sia già qualificato a una coppa europea grazie alla posizione in campionato.</rdfs:comment>
        <rdfs:comment xml:lang="en">The DFB-Pokal [ˈdeː ʔɛf beː poˈkaːl] (until 1943 Tschammer-Pokal [tʃaːmɐ poˈkaːl]) (English: German Cup) is a German knockout football cup competition held annually by the Deutscher Fußball-Bund (DFB) (English: German Football Association). Sixty-four teams participate in the competition, including all clubs from the Bundesliga and the 2. Bundesliga. It is considered the second-most important club title in German football after the Bundesliga championship. Taking place from August until May, the winner qualifies for the DFL-Supercup and the UEFA Europa League unless the winner already qualifies for the UEFA Champions League in the Bundesliga.</rdfs:comment>
        <rdfs:label xml:lang="en">DFB-Pokal</rdfs:label>
        <rdfs:label xml:lang="it">DFB-Pokal</rdfs:label>
    </owl:NamedIndividual>
    


    <!-- http://www.semanticweb.org/2021/ontologies/calcio#Daniele_Orsato -->

    <owl:NamedIndividual rdf:about="http://www.semanticweb.org/2021/ontologies/calcio#Daniele_Orsato">
        <rdf:type rdf:resource="http://www.semanticweb.org/2021/ontologies/calcio#Arbitro"/>
        <rdfs:comment xml:lang="it">Daniele Orsato (Montecchio Maggiore, 23 novembre 1975) è un arbitro di calcio italiano.

È stato eletto miglior arbitro al mondo dall&apos;IFFHS nel 2020.[1]</rdfs:comment>
        <rdfs:comment xml:lang="en">Daniele Orsato (born 23 November 1975)[1] is an Italian football referee.</rdfs:comment>
        <rdfs:label xml:lang="en">Daniele Orsato</rdfs:label>
        <rdfs:label xml:lang="it">Daniele Orsato</rdfs:label>
    </owl:NamedIndividual>
    


    <!-- http://www.semanticweb.org/2021/ontologies/calcio#Davide_Calabria -->

    <owl:NamedIndividual rdf:about="http://www.semanticweb.org/2021/ontologies/calcio#Davide_Calabria">
        <giocaPer rdf:resource="http://www.semanticweb.org/2021/ontologies/calcio#ACMilan"/>
        <rdfs:comment xml:lang="it">Davide Calabria (Adro, 6 dicembre 1996) è un calciatore italiano, difensore del Milan e della nazionale italiana[3].</rdfs:comment>
        <rdfs:comment xml:lang="en">Davide Calabria (born 6 December 1996) is an Italian professional footballer, who plays for Milan and the Italy national team as a full-back, mainly on the right side of the pitch.</rdfs:comment>
        <rdfs:label xml:lang="en">Davide Calabria</rdfs:label>
        <rdfs:label xml:lang="it">Davide Calabria</rdfs:label>
    </owl:NamedIndividual>
    


    <!-- http://www.semanticweb.org/2021/ontologies/calcio#Diogo_Dalot -->

    <owl:NamedIndividual rdf:about="http://www.semanticweb.org/2021/ontologies/calcio#Diogo_Dalot">
        <giocaPer rdf:resource="http://www.semanticweb.org/2021/ontologies/calcio#ACMilan"/>
        <rdfs:comment xml:lang="en">José Diogo Dalot Teixeira (Portuguese pronunciation: [diˈoɡu dɐˈlo];[2] born 18 March 1999) is a Portuguese professional footballer who plays as a full-back and occasionally as a winger[3][4] for Milan, on loan from Premier League club Manchester United.</rdfs:comment>
        <rdfs:comment xml:lang="it">José Diogo Dalot Teixeira, noto semplicemente come Diogo Dalot (Braga, 18 marzo 1999), è un calciatore portoghese, difensore del Milan, in prestito dal Manchester Utd, e della nazionale under-21 portoghese.</rdfs:comment>
        <rdfs:label xml:lang="en">Diogo Dalot</rdfs:label>
        <rdfs:label xml:lang="it">Diogo Dalot</rdfs:label>
    </owl:NamedIndividual>
    


    <!-- http://www.semanticweb.org/2021/ontologies/calcio#Erling_Braut_Haaland -->

    <owl:NamedIndividual rdf:about="http://www.semanticweb.org/2021/ontologies/calcio#Erling_Braut_Haaland">
        <giocaPer rdf:resource="http://www.semanticweb.org/2021/ontologies/calcio#BorussiaDortmund"/>
        <rdfs:comment xml:lang="en">Erling Braut Haaland (né Håland, [ˈhòːlɑn]; born 21 July 2000) is a Norwegian professional footballer who plays as a striker for Bundesliga club Borussia Dortmund and the Norway national team. A prolific goalscorer, he is recognised for his pace, athleticism, strength and precise off-the-ball movement, and he has been considered as one of the best young footballers in the world.[5][6]</rdfs:comment>
        <rdfs:comment xml:lang="it">Erling Braut Håland (Leeds, 21 luglio 2000) è un calciatore norvegese, attaccante del Borussia Dortmund e della nazionale norvegese.</rdfs:comment>
        <rdfs:label xml:lang="en">Erling Haaland</rdfs:label>
        <rdfs:label xml:lang="it">Erling Håland</rdfs:label>
    </owl:NamedIndividual>
    


    <!-- http://www.semanticweb.org/2021/ontologies/calcio#Euro_2008 -->

    <owl:NamedIndividual rdf:about="http://www.semanticweb.org/2021/ontologies/calcio#Euro_2008">
        <rdf:type rdf:resource="http://www.semanticweb.org/2021/ontologies/calcio#trofeoDiNazione"/>
        <rdfs:comment xml:lang="it">Il campionato europeo di calcio 2008 (in francese: Championnat d&apos;Europe de football 2008, in tedesco: Fußball-Europameisterschaft 2008, in romancio: Campiunadi d&apos;Europa da ballape 2008, in inglese: European Football Championship 2008), noto anche come UEFA Euro 2008 o Austria-Svizzera 2008, è stata la 13ª edizione della massima competizione continentale calcistica per Nazioni organizzato dall&apos;Union of European Football Associations (UEFA), il campionato europeo di calcio.</rdfs:comment>
        <rdfs:comment xml:lang="en">The 2008 UEFA European Football Championship, commonly referred to as UEFA Euro 2008 or simply Euro 2008, was the 13th UEFA European Football Championship, a quadrennial football tournament contested by the member nations of UEFA (the Union of European Football Associations). It took place in Austria and Switzerland (both hosting the tournament for the first time) from 7 to 29 June 2008.</rdfs:comment>
        <rdfs:label xml:lang="it">Campionato europeo di calcio 2008</rdfs:label>
        <rdfs:label xml:lang="en">UEFA Euro 2008</rdfs:label>
    </owl:NamedIndividual>
    


    <!-- http://www.semanticweb.org/2021/ontologies/calcio#EuropaLeague -->

    <owl:NamedIndividual rdf:about="http://www.semanticweb.org/2021/ontologies/calcio#EuropaLeague">
        <rdf:type rdf:resource="http://www.semanticweb.org/2021/ontologies/calcio#trofeoDiClub"/>
        <rdfs:comment xml:lang="it">La UEFA Europa League, meglio nota come Europa League, è una competizione calcistica continentale per squadre di club organizzata dalla UEFA, la seconda per prestigio dopo la Champions League.

La denominazione di Europa League sostituì nel 2009 quella storica di Coppa UEFA, istituita nel 1971 dalla confederazione calcistica europea. Questo torneo, a sua volta, aveva preso il posto de facto della Coppa delle Fiere, inizialmente disputata su invito, e non per diritto acquisito, da rappresentative di grandi città dell&apos;Europa che ospitavano fiere commerciali. L&apos;UEFA ha definito la Coppa delle Fiere come antenata della successiva Coppa UEFA/Europa League; tuttavia, non essendone stata l&apos;organizzatrice, non è mai stata riconosciuta de iure come manifestazione ufficiale dalla confederazione continentale. Per tale motivo la Coppa delle Fiere non viene inclusa neppure nelle statistiche riguardanti la Coppa UEFA/Europa League.</rdfs:comment>
        <rdfs:comment xml:lang="en">The UEFA Europa League (abbreviated as UEL) is an annual football club competition organised by UEFA since 1971 for eligible European football clubs. Clubs qualify for the competition based on their performance in their national leagues and cup competitions. It is now the second-tier competition of European club football, ranking below the UEFA Champions League, after being a third-tier competition from 1971 to 1999 before the UEFA Cup Winners&apos; Cup was discontinued.[1]</rdfs:comment>
        <rdfs:label xml:lang="en">UEFA Europa League</rdfs:label>
        <rdfs:label xml:lang="it">UEFA Europa League</rdfs:label>
    </owl:NamedIndividual>
    


    <!-- http://www.semanticweb.org/2021/ontologies/calcio#FACup -->

    <owl:NamedIndividual rdf:about="http://www.semanticweb.org/2021/ontologies/calcio#FACup">
        <rdf:type rdf:resource="http://www.semanticweb.org/2021/ontologies/calcio#trofeoDiClub"/>
        <rdfs:comment xml:lang="it">La Football Association Challenge Cup, meglio conosciuta come FA Cup (in italiano nota come Coppa d&apos;Inghilterra), è la principale coppa nazionale di calcio inglese, nonché la più antica competizione calcistica ufficiale al mondo, essendo stata istituita nel 1871.</rdfs:comment>
        <rdfs:comment xml:lang="en">The Football Association Challenge Cup, more commonly known as the FA Cup, is an annual knockout football competition in men&apos;s domestic English football. First played during the 1871–72 season, it is the oldest national football competition in the world.[1] It is organised by and named after The Football Association (The FA). Since 2015, it has been known as The Emirates FA Cup after its headline sponsor. A concurrent women&apos;s tournament is also held, the Women&apos;s FA Cup.</rdfs:comment>
        <rdfs:label xml:lang="en">FA Cup</rdfs:label>
        <rdfs:label xml:lang="it">FA Cup</rdfs:label>
    </owl:NamedIndividual>
    


    <!-- http://www.semanticweb.org/2021/ontologies/calcio#Francia -->

    <owl:NamedIndividual rdf:about="http://www.semanticweb.org/2021/ontologies/calcio#Francia">
        <rdf:type rdf:resource="http://www.semanticweb.org/2021/ontologies/calcio#squadraNazionale"/>
        <rdfs:comment xml:lang="it">La nazionale di calcio della Francia (fr. Équipe de France de football) è la selezione calcistica[3] rappresentativa della Francia posta sotto l&apos;egida della Federazione calcistica francese.

Ha vinto due campionati del mondo (Francia 1998 e Russia 2018), due campionati d&apos;Europa (Francia 1984 e Belgio-Paesi Bassi 2000) e due Confederations Cup (Corea del Sud-Giappone 2001 e Francia 2003).</rdfs:comment>
        <rdfs:comment xml:lang="en">The France national football team (French: Équipe de France de football) represents France in men&apos;s international football and is controlled by the French Football Federation, also known as FFF, or in French: Fédération française de football. The team&apos;s colours are blue, white and red, and the coq gaulois its symbol. France are colloquially known as Les Bleus (The Blues). They are the reigning world champions, having won the most recent World Cup final in 2018.</rdfs:comment>
        <rdfs:label xml:lang="en">France national football team</rdfs:label>
        <rdfs:label xml:lang="it">Nazionale di calcio della Francia</rdfs:label>
    </owl:NamedIndividual>
    


    <!-- http://www.semanticweb.org/2021/ontologies/calcio#Franck_Kessié -->

    <owl:NamedIndividual rdf:about="http://www.semanticweb.org/2021/ontologies/calcio#Franck_Kessié">
        <giocaPer rdf:resource="http://www.semanticweb.org/2021/ontologies/calcio#ACMilan"/>
        <rdfs:comment xml:lang="it">Franck Yannick Kessié (Ouragahio, 19 dicembre 1996) è un calciatore ivoriano, centrocampista del Milan e della nazionale ivoriana.</rdfs:comment>
        <rdfs:comment xml:lang="en">Franck Yannick Kessié (born 19 December 1996) is an Ivorian professional footballer who plays as a central midfielder for Italian club Milan and the Ivory Coast national team.</rdfs:comment>
        <rdfs:label xml:lang="en">Franck Kessié</rdfs:label>
        <rdfs:label xml:lang="it">Franck Kessié</rdfs:label>
    </owl:NamedIndividual>
    


    <!-- http://www.semanticweb.org/2021/ontologies/calcio#Frederic_Massara -->

    <owl:NamedIndividual rdf:about="http://www.semanticweb.org/2021/ontologies/calcio#Frederic_Massara">
        <rdf:type rdf:resource="http://www.semanticweb.org/2021/ontologies/calcio#Dirigente"/>
        <collegaDi rdf:resource="http://www.semanticweb.org/2021/ontologies/calcio#Paolo_Maldini"/>
        <rdfs:comment xml:lang="it">Frederic Massara (Torino, 11 novembre 1968) è un dirigente sportivo, allenatore di calcio ed ex calciatore italiano, di ruolo attaccante, direttore sportivo del Milan.</rdfs:comment>
        <rdfs:comment xml:lang="en">Frederic Massara (born 11 November 1968) is an Italian football director, coach and former player. He is currently the director of football of AC Milan.</rdfs:comment>
        <rdfs:label xml:lang="en">Frederic Massara</rdfs:label>
        <rdfs:label xml:lang="it">Frederic Massara</rdfs:label>
    </owl:NamedIndividual>
    


    <!-- http://www.semanticweb.org/2021/ontologies/calcio#Germania -->

    <owl:NamedIndividual rdf:about="http://www.semanticweb.org/2021/ontologies/calcio#Germania">
        <rdf:type rdf:resource="http://www.semanticweb.org/2021/ontologies/calcio#squadraNazionale"/>
        <rdfs:comment xml:lang="it">La nazionale di calcio della Germania (in tedesco Deutsche Fußballnationalmannschaft) è la rappresentativa calcistica della Germania ed è posta sotto l&apos;egida della Deutscher Fussball-Bund.

È una delle nazionali di calcio più blasonate al mondo oltreché la più titolata d&apos;Europa, essendosi aggiudicata per quattro volte il campionato mondiale, per tre volte il campionato europeo e per una volta la Confederations Cup. Nelle due principali competizioni per nazionali (Mondiale ed Europeo) è giunta a disputare la partita finale rispettivamente otto e sei volte: in entrambi i casi si tratta di un record. A livello europeo condivide con la Spagna il primato di vittorie nella manifestazione continentale (3) e con l’Italia quello di vittorie nel mondiale (4). La nazionale tedesca è una delle due selezioni europee, insieme alla nazionale francese, ad avere vinto almeno una volta le tre maggiori competizioni internazionali (Europeo, Mondiale e Confederations Cup).</rdfs:comment>
        <rdfs:comment xml:lang="en">The Germany national football team (German: Deutsche Fußballnationalmannschaft or Die Mannschaft) represents Germany in men&apos;s international football and played its first match in 1908.[5] The team is governed by the German Football Association (Deutscher Fußball-Bund), founded in 1900.[9][10] Between 1949 and 1990, separate German national teams were recognised by FIFA due to Allied occupation and division: the DFB&apos;s team representing the Federal Republic of Germany (named West Germany from 1949 to 1990), the Saarland team representing the Saar Protectorate (1950–1956) and the East German team representing the German Democratic Republic (1952–1990). The latter two were absorbed along with their records;[11][12] the present team represents the reunified Federal Republic. The official name and code &quot;Germany FR (FRG)&quot; was shortened to &quot;Germany (GER)&quot; following reunification in 1990.</rdfs:comment>
        <rdfs:label xml:lang="en">Germany national football team</rdfs:label>
        <rdfs:label xml:lang="it">Nazionale di calcio della Germania</rdfs:label>
    </owl:NamedIndividual>
    


    <!-- http://www.semanticweb.org/2021/ontologies/calcio#Gianluigi_Donnarumma -->

    <owl:NamedIndividual rdf:about="http://www.semanticweb.org/2021/ontologies/calcio#Gianluigi_Donnarumma">
        <rdfs:comment xml:lang="it">Gianluigi Donnarumma (Castellammare di Stabia, 25 febbraio 1999) è un calciatore italiano, portiere del Milan e della nazionale italiana.

Talento precoce, ha esordito in Serie A a 16 anni e 8 mesi,[1] affermandosi fin dall&apos;inizio come portiere titolare del Milan, con cui ha vinto una Supercoppa italiana. Nel 2016, non ancora maggiorenne, ha debuttato dapprima nell&apos;Italia Under-21 e poi nella nazionale maggiore, entrando stabilmente nel giro di quest&apos;ultima.</rdfs:comment>
        <rdfs:comment xml:lang="en">Gianluigi Donnarumma (Italian pronunciation: [dʒanluˈiːdʒi ˌdɔnnaˈrumma]; born 25 February 1999) is an Italian professional footballer who plays as a goalkeeper for Serie A club Milan and the Italy national team.</rdfs:comment>
        <rdfs:label xml:lang="en">Gianluigi Donnarumma</rdfs:label>
        <rdfs:label xml:lang="it">Gianluigi Donnarumma</rdfs:label>
    </owl:NamedIndividual>
    


    <!-- http://www.semanticweb.org/2021/ontologies/calcio#Giuseppe_Marotta -->

    <owl:NamedIndividual rdf:about="http://www.semanticweb.org/2021/ontologies/calcio#Giuseppe_Marotta">
        <rdf:type rdf:resource="http://www.semanticweb.org/2021/ontologies/calcio#Dirigente"/>
        <rdfs:comment xml:lang="en">Giuseppe &quot;Beppe&quot; Marotta (born 25 March 1957) is an Italian football executive who is currently the CEO for sport of Italian football club Internazionale. In 2014, he was inducted into the Italian Football Hall of Fame.[1]</rdfs:comment>
        <rdfs:comment xml:lang="it">Giuseppe Marotta, detto Beppe (Varese, 25 marzo 1957), è un dirigente sportivo italiano, amministratore delegato dell&apos;Inter e consigliere della Lega Nazionale Professionisti Serie A.</rdfs:comment>
        <rdfs:label xml:lang="en">Giuseppe Marotta</rdfs:label>
        <rdfs:label xml:lang="it">Giuseppe Marotta</rdfs:label>
    </owl:NamedIndividual>
    


    <!-- http://www.semanticweb.org/2021/ontologies/calcio#Hakan_Çalhanoğlu -->

    <owl:NamedIndividual rdf:about="http://www.semanticweb.org/2021/ontologies/calcio#Hakan_Çalhanoğlu">
        <rdfs:comment xml:lang="it">Hakan Çalhanoğlu (AFI: [ˈhaːkan ˈt͡ʃaɫhanoːɫu]; Mannheim, 8 febbraio 1994) è un calciatore turco con cittadinanza tedesca, centrocampista o attaccante del Milan e della nazionale turca.</rdfs:comment>
        <rdfs:comment xml:lang="en">Hakan Çalhanoğlu (Turkish pronunciation: [ˈhaːkan ˈtʃaɫhanoːɫu], born 8 February 1994) is a Turkish professional footballer who plays as an attacking midfielder for Serie A club Milan and the Turkish national team.</rdfs:comment>
        <rdfs:label xml:lang="en">Hakan Çalhanoğlu</rdfs:label>
        <rdfs:label xml:lang="it">Hakan Çalhanoğlu</rdfs:label>
    </owl:NamedIndividual>
    


    <!-- http://www.semanticweb.org/2021/ontologies/calcio#Inter -->

    <owl:NamedIndividual rdf:about="http://www.semanticweb.org/2021/ontologies/calcio#Inter">
        <giocaInStadio rdf:resource="http://www.semanticweb.org/2021/ontologies/calcio#San_Siro"/>
        <rdfs:comment xml:lang="en">Football Club Internazionale Milano, commonly referred to as Internazionale (pronounced [ˌinternattsjoˈnaːle]) or simply Inter, and known as Inter Milan outside Italy,[9][10] is an Italian professional football club based in Milan, Lombardy. Inter is the only Italian club never to have been relegated from the top flight of Italian football.</rdfs:comment>
        <rdfs:comment xml:lang="it">Il Football Club Internazionale Milano, meglio conosciuto come Internazionale (/internaʦʦjoˈnale/)[1] o più semplicemente come Inter, è una società calcistica italiana con sede nella città di Milano.</rdfs:comment>
        <rdfs:label xml:lang="it">Football Club Internazionale Milano</rdfs:label>
        <rdfs:label xml:lang="en">Inter Milan</rdfs:label>
    </owl:NamedIndividual>
    


    <!-- http://www.semanticweb.org/2021/ontologies/calcio#Ismaël_Bennacer -->

    <owl:NamedIndividual rdf:about="http://www.semanticweb.org/2021/ontologies/calcio#Ismaël_Bennacer">
        <giocaPer rdf:resource="http://www.semanticweb.org/2021/ontologies/calcio#ACMilan"/>
        <rdfs:comment xml:lang="en">Ismaël Bennacer (Arabic: إسماعيل بن ناصر‎; born 1 December 1997) is an Algerian professional footballer who plays as a midfielder for Serie A club Milan and the Algeria national team.</rdfs:comment>
        <rdfs:comment xml:lang="it">Ismaël Bennacer (Arles, 1º dicembre 1997) è un calciatore algerino con cittadinanza francese, centrocampista del Milan e della nazionale algerina, con cui si è laureato campione d’Africa nel 2019.

È stato inoltre eletto migliore giocatore della Coppa d&apos;Africa 2019 e inserito nella migliore squadra della stessa competizione.</rdfs:comment>
        <rdfs:label xml:lang="en">Ismaël Bennacer</rdfs:label>
        <rdfs:label xml:lang="it">Ismaël Bennacer</rdfs:label>
    </owl:NamedIndividual>
    


    <!-- http://www.semanticweb.org/2021/ontologies/calcio#Italia -->

    <owl:NamedIndividual rdf:about="http://www.semanticweb.org/2021/ontologies/calcio#Italia">
        <rdf:type rdf:resource="http://www.semanticweb.org/2021/ontologies/calcio#squadraNazionale"/>
        <haVinto rdf:resource="http://www.semanticweb.org/2021/ontologies/calcio#WorldCup_1934"/>
        <haVinto rdf:resource="http://www.semanticweb.org/2021/ontologies/calcio#WorldCup_1938"/>
        <haVinto rdf:resource="http://www.semanticweb.org/2021/ontologies/calcio#WorldCup_1982"/>
        <rdfs:comment xml:lang="it">La nazionale di calcio dell&apos;Italia è la selezione maggiore maschile di calcio della Federazione Italiana Giuoco Calcio, il cui nome ufficiale è nazionale A,[3] che rappresenta l&apos;Italia nelle varie competizioni ufficiali o amichevoli riservate a squadre nazionali.</rdfs:comment>
        <rdfs:comment xml:lang="en">The Italy national football team (Italian: Nazionale di calcio dell&apos;Italia) has officially represented Italy in international football since their first match in 1910. The squad is under the global jurisdiction of FIFA and is governed in Europe by UEFA—the latter of which was co-founded by the Italian team&apos;s supervising body, the Italian Football Federation (FIGC). Italy&apos;s home matches are played at various stadiums throughout Italy, and their primary training ground, Centro Tecnico Federale di Coverciano, is located at the FIGC technical headquarters in Coverciano, Florence.</rdfs:comment>
        <rdfs:label xml:lang="en">Italy national football team</rdfs:label>
        <rdfs:label xml:lang="it">Nazionale di calcio dell&apos;Italia</rdfs:label>
    </owl:NamedIndividual>
    


    <!-- http://www.semanticweb.org/2021/ontologies/calcio#Jens_Petter_Hauge -->

    <owl:NamedIndividual rdf:about="http://www.semanticweb.org/2021/ontologies/calcio#Jens_Petter_Hauge">
        <giocaPer rdf:resource="http://www.semanticweb.org/2021/ontologies/calcio#ACMilan"/>
        <rdfs:comment xml:lang="it">Jens Petter Hauge (Bodø, 12 ottobre 1999) è un calciatore norvegese, attaccante del Milan e della nazionale norvegese.</rdfs:comment>
        <rdfs:comment xml:lang="en">Jens Petter Hauge (Norwegian: [ˈjɛns ˈpɛ̀tːər ˈhœ̂ʏɡə]; born 12 October 1999) is a Norwegian professional footballer who plays as a winger for Italian Serie A club Milan and the Norway national team.</rdfs:comment>
        <rdfs:label xml:lang="en">Jens Petter Hauge</rdfs:label>
        <rdfs:label xml:lang="it">Jens Petter Hauge</rdfs:label>
    </owl:NamedIndividual>
    


    <!-- http://www.semanticweb.org/2021/ontologies/calcio#Juventus -->

    <owl:NamedIndividual rdf:about="http://www.semanticweb.org/2021/ontologies/calcio#Juventus">
        <appartieneALega rdf:resource="http://www.semanticweb.org/2021/ontologies/calcio#SerieA"/>
        <rdfs:comment xml:lang="en">Juventus Football Club (from Latin: iuventūs, &quot;youth&quot;; Italian pronunciation: [juˈvɛntus]), colloquially known as Juve (pronounced [ˈjuːve]),[3] is a professional football club based in Turin, Piedmont, Italy, that competes in the Serie A, the top flight of Italian football. Founded in 1897 by a group of Torinese students, the club has worn a black and white striped home kit since 1903 and has played home matches in different grounds around its city, the latest being the 41,507-capacity Juventus Stadium. Nicknamed Vecchia Signora (&quot;the Old Lady&quot;), the club has won 36 official league titles, 13 Coppa Italia titles and nine Supercoppa Italiana titles, being the record holder for all these competitions; two Intercontinental Cups, two European Cups / UEFA Champions Leagues, one European Cup Winners&apos; Cup, a joint national record of three UEFA Cups, two UEFA Super Cups and a joint national record of one UEFA Intertoto Cup.[4][5] Consequently, the side leads the historical Federazione Italiana Giuoco Calcio (FIGC) ranking[a] whilst on the international stage occupies the sixth position in Europe and the twelfth in the world for most confederation titles won with eleven trophies,[7] having led the UEFA ranking during seven seasons since its inception in 1979, the most for an Italian team and joint second overall.</rdfs:comment>
        <rdfs:comment xml:lang="it">La Juventus Football Club (dal latino: iuventūs, «gioventù»), meglio nota come Juventus (/juˈvɛntus/),[1] è una società calcistica italiana con sede nella città di Torino.</rdfs:comment>
        <rdfs:label xml:lang="en">Juventus F.C.</rdfs:label>
        <rdfs:label xml:lang="it">Juventus Football Club</rdfs:label>
    </owl:NamedIndividual>
    


    <!-- http://www.semanticweb.org/2021/ontologies/calcio#Kylian_Mbappé -->

    <owl:NamedIndividual rdf:about="http://www.semanticweb.org/2021/ontologies/calcio#Kylian_Mbappé">
        <giocaPer rdf:resource="http://www.semanticweb.org/2021/ontologies/calcio#ParisSaintGermain"/>
        <rdfs:comment xml:lang="it">Kylian Mbappé Lottin (Bondy, 20 dicembre 1998) è un calciatore francese attaccante del Paris Saint-Germain e della nazionale francese, con cui si è laureato campione del mondo nel 2018.</rdfs:comment>
        <rdfs:comment xml:lang="en">Kylian Mbappé Lottin (born 20 December 1998) is a French professional footballer who plays as a forward for Ligue 1 club Paris Saint-Germain and the France national team. Widely considered as one of the best players in the world, he is known for his dribbling, explosive speed, and clinical finishing.</rdfs:comment>
        <rdfs:label xml:lang="en">Kylian Mbappé</rdfs:label>
        <rdfs:label xml:lang="it">Kylian Mbappé</rdfs:label>
    </owl:NamedIndividual>
    


    <!-- http://www.semanticweb.org/2021/ontologies/calcio#LaLiga -->

    <owl:NamedIndividual rdf:about="http://www.semanticweb.org/2021/ontologies/calcio#LaLiga">
        <rdfs:comment xml:lang="it">Il Campeonato Nacional de Liga de Primera División, noto anche come LaLiga e LaLiga Santander per ragioni di sponsorizzazione, è la massima serie calcistica spagnola, che si colloca al vertice del sistema del campionato di calcio spagnolo ed è gestita dalla Liga de Fútbol Profesional (LFP). Dalla stagione 2008-2009 a quella 2016-2017 ha assunto la denominazione commerciale di Liga BBVA.

La squadra campione in carica è il Real Madrid, che nella stagione 2019-2020 ha vinto per la 34ª volta il campionato.</rdfs:comment>
        <rdfs:comment xml:lang="en">The Campeonato Nacional de Liga de Primera División,[a] commonly known as La Liga[b] (LaLiga Santander for sponsorship reasons with Santander),[2] stylized as LaLiga, is the men&apos;s top professional football division of the Spanish football league system.[3] Administered by the Liga Nacional de Fútbol Profesional,[c] is contested by 20 teams, with the three lowest-placed teams at the end of each season relegated to the Segunda División and replaced by the top two teams and a play-off winner in that division.</rdfs:comment>
        <rdfs:label xml:lang="en">La Liga</rdfs:label>
        <rdfs:label xml:lang="it">Primera División</rdfs:label>
    </owl:NamedIndividual>
    


    <!-- http://www.semanticweb.org/2021/ontologies/calcio#Le_Parc_des_Princes -->

    <owl:NamedIndividual rdf:about="http://www.semanticweb.org/2021/ontologies/calcio#Le_Parc_des_Princes">
        <rdf:type rdf:resource="http://www.semanticweb.org/2021/ontologies/calcio#Stadio"/>
        <haCapienza rdf:datatype="http://www.w3.org/2001/XMLSchema#integer">47929</haCapienza>
        <rdfs:comment xml:lang="it">Parco dei Principi (in francese Parc des Princes o Parc-des-Princes, più formalmente Stade du Parc des Princes) è il nome di tre impianti sportivi polivalenti di Parigi, capitale della Francia, edificati in successione tra il 1897 e il 1972 sulla stessa area di circa 60000 m² nel XVI arrondissement, nella periferia sudoccidentale della città al confine con Boulogne-Billancourt.</rdfs:comment>
        <rdfs:comment xml:lang="en">The Parc des Princes (French pronunciation: ​[paʁk de pʁɛ̃s], &quot;Princes’ Park&quot; in English) is an all-seater football stadium in Paris, France,[1] in the south-west of the French capital, inside the 16th arrondissement, near the Stade Jean-Bouin and Stade Roland Garros.</rdfs:comment>
        <rdfs:label xml:lang="en">Parc des Princes</rdfs:label>
        <rdfs:label xml:lang="it">Parco dei Principi</rdfs:label>
    </owl:NamedIndividual>
    


    <!-- http://www.semanticweb.org/2021/ontologies/calcio#Ligue1 -->

    <owl:NamedIndividual rdf:about="http://www.semanticweb.org/2021/ontologies/calcio#Ligue1">
        <rdfs:comment xml:lang="it">La Ligue 1, nota come Division 1 fino al 2002, è il massimo livello professionistico del campionato di calcio francese.</rdfs:comment>
        <rdfs:comment xml:lang="en">Ligue 1[b], officially known as Ligue 1 Uber Eats for sponsorship reasons,[1][2][3] is a French professional league for men&apos;s association football clubs. At the top of the French football league system, it is the country&apos;s primary football competition. Administrated by the Ligue de Football Professionnel, Ligue 1 is contested by 20 clubs and operates on a system of promotion and relegation from and to Ligue 2.</rdfs:comment>
        <rdfs:label xml:lang="en">Ligue 1</rdfs:label>
        <rdfs:label xml:lang="it">Ligue 1</rdfs:label>
    </owl:NamedIndividual>
    


    <!-- http://www.semanticweb.org/2021/ontologies/calcio#Ligue2 -->

    <owl:NamedIndividual rdf:about="http://www.semanticweb.org/2021/ontologies/calcio#Ligue2">
        <rdfs:comment xml:lang="it">La Ligue 2, nota anche come Ligue 2 BKT per motivi di sponsorizzazione[2], è la seconda divisione del campionato francese di calcio.</rdfs:comment>
        <rdfs:comment xml:lang="en">Ligue 2 (French pronunciation: ​[liɡ dø], League 2), also known as Ligue 2 BKT due to sponsorship by Balkrishna Industries, is a French professional football league. The league serves as the second division of French football and is one of two divisions making up the Ligue de Football Professionnel (LFP), the other being Ligue 1, the country&apos;s top football division. Contested by 20 clubs, it operates on a system of promotion and relegation with both Ligue 1 and the third division Championnat National. Seasons run from August to May, with teams playing 38 games each totalling 380 games in the season. Most games are played on Fridays and Mondays, with a few games played during weekday and weekend evenings. Play is regularly suspended the last weekend before Christmas for two weeks before returning in the second week of January.</rdfs:comment>
        <rdfs:label xml:lang="en">Ligue 2</rdfs:label>
        <rdfs:label xml:lang="it">Ligue 2</rdfs:label>
    </owl:NamedIndividual>
    


    <!-- http://www.semanticweb.org/2021/ontologies/calcio#Lille -->

    <owl:NamedIndividual rdf:about="http://www.semanticweb.org/2021/ontologies/calcio#Lille">
        <rdf:type rdf:resource="http://www.semanticweb.org/2021/ontologies/calcio#squadraDiClub"/>
        <rdfs:comment xml:lang="it">Il Lille Olympique Sporting Club, noto come LOSC o semplicemente come Lille (in italiano anche Lilla), è una società calcistica francese della città di Lilla, capoluogo del dipartimento del Nord. Milita attualmente nella Ligue 1, massima divisione del campionato francese di calcio.</rdfs:comment>
        <rdfs:comment xml:lang="en">Lille Olympique Sporting Club (French pronunciation: ​[lil ɔlɛ̃pik spɔːʳtɪŋ klœb]), commonly called LOSC, also referred to as LOSC Lille, Lille OSC or simply Lille, is a French professional football club based in Lille in Hauts-de-France. The club was founded in 1944 as a result of a merger and plays in Ligue 1, the top tier of French football. Lille has played its home matches since 2012 at Stade Pierre-Mauroy in nearby Villeneuve d&apos;Ascq, which replaced the club&apos;s previous home of Stade Lille-Metropole in the same community.</rdfs:comment>
        <rdfs:label xml:lang="it">LOSC Lille</rdfs:label>
        <rdfs:label xml:lang="en">Lille OSC</rdfs:label>
    </owl:NamedIndividual>
    


    <!-- http://www.semanticweb.org/2021/ontologies/calcio#Lione -->

    <owl:NamedIndividual rdf:about="http://www.semanticweb.org/2021/ontologies/calcio#Lione">
        <rdf:type rdf:resource="http://www.semanticweb.org/2021/ontologies/calcio#squadraDiClub"/>
        <appartieneALega rdf:resource="http://www.semanticweb.org/2021/ontologies/calcio#Ligue1"/>
        <rdfs:comment xml:lang="it">L&apos;Olympique Lyonnais, noto in italiano come Olympique Lione o più semplicemente Lione, è una società polisportiva francese con sede nella città di Lione, nota soprattutto per la sua sezione calcistica, militante nella Ligue 1, la massima divisione del campionato francese di calcio.</rdfs:comment>
        <rdfs:comment xml:lang="en">Olympique Lyonnais (French pronunciation: ​[ɔlɛ̃pik ljɔnɛ]) (officially Olympique lyonnais in French), commonly referred to as simply Lyon (French pronunciation: ​[ljɔ̃]) or OL, is a French professional football club based in Lyon in Auvergne-Rhône-Alpes, it plays in France&apos;s highest football division, Ligue 1. The club was established in 1950.[1] The club won its first Ligue 1 championship in 2002, starting a national record-setting streak of seven successive titles. Lyon has also won eight Trophées des Champions, five Coupes de France, and three Ligue 2 titles.</rdfs:comment>
        <rdfs:label xml:lang="en">Olympique Lyonnais</rdfs:label>
        <rdfs:label xml:lang="it">Olympique Lyonnais</rdfs:label>
    </owl:NamedIndividual>
    


    <!-- http://www.semanticweb.org/2021/ontologies/calcio#Lionel_Messi -->

    <owl:NamedIndividual rdf:about="http://www.semanticweb.org/2021/ontologies/calcio#Lionel_Messi">
        <rdf:type rdf:resource="http://www.semanticweb.org/2021/ontologies/calcio#Calciatore"/>
        <haRuolo rdf:resource="http://www.semanticweb.org/2021/ontologies/calcio#attaccanteBarcellona"/>
        <calciatoreHaValoreDiMercato rdf:datatype="http://www.w3.org/2001/XMLSchema#long">80000000</calciatoreHaValoreDiMercato>
        <dataUltimoTrasferimento rdf:datatype="http://www.w3.org/2001/XMLSchema#dateTime">2005-07-01T00:00:00</dataUltimoTrasferimento>
        <haEtà rdf:datatype="http://www.w3.org/2001/XMLSchema#integer">33</haEtà>
        <haNazionalità>Argentina</haNazionalità>
        <haNome rdf:datatype="http://www.w3.org/2001/XMLSchema#string">Lionel Andrés Messi Cuccitini</haNome>
        <stipendioCorrente rdf:datatype="http://www.w3.org/2001/XMLSchema#long">78500000</stipendioCorrente>
        <rdfs:comment xml:lang="it">Lionel Andrés Messi Cuccittini, detto Leo (pronuncia spagnola [ljoˈnel ˈmesi]; Rosario, 24 giugno 1987), è un calciatore argentino, centrocampista o attaccante del Barcellona e della nazionale argentina, delle quali è capitano. Con l&apos;Albiceleste è stato vicecampione del mondo nel 2014 e del Sud America negli anni 2007, 2015 e 2016; inoltre con la nazionale olimpica ha vinto la medaglia d&apos;oro ai Giochi olimpici di Pechino nel 2008 e con la nazionale Under-20 è stato campione del mondo di categoria nel 2005.</rdfs:comment>
        <rdfs:comment xml:lang="en">Lionel Andrés Messi[note 1] (Spanish pronunciation: [ljoˈnel anˈdɾes ˈmesi] (About this soundlisten);[A] born 24 June 1987) is an Argentine professional footballer who plays as a forward and captains both the Spanish club Barcelona and the Argentina national team. Often considered as the best player in the world and widely regarded as one of the greatest players of all time, Messi has won a record six Ballon d&apos;Or awards[note 2] and a record six European Golden Shoes. He has spent his entire professional career with Barcelona, where he has won a club-record 33 trophies, including ten La Liga titles, four UEFA Champions League titles and six Copas del Rey. A prolific goalscorer and creative playmaker, Messi holds the records for most goals in La Liga (455), a La Liga and European league season (50), most hat-tricks in La Liga (36) and the UEFA Champions League (8), and most assists in La Liga (185), a La Liga and European league season (21)[9] and the Copa América (12). He has scored over 700 senior career goals for club and country.</rdfs:comment>
        <rdfs:label xml:lang="en">Lionel Messi</rdfs:label>
        <rdfs:label xml:lang="it">Lionel Messi</rdfs:label>
    </owl:NamedIndividual>
    


    <!-- http://www.semanticweb.org/2021/ontologies/calcio#Liverpool -->

    <owl:NamedIndividual rdf:about="http://www.semanticweb.org/2021/ontologies/calcio#Liverpool">
        <rdf:type rdf:resource="http://www.semanticweb.org/2021/ontologies/calcio#squadraDiClub"/>
        <appartieneALega rdf:resource="http://www.semanticweb.org/2021/ontologies/calcio#PremierLeague"/>
        <giocaInStadio rdf:resource="http://www.semanticweb.org/2021/ontologies/calcio#Anfield"/>
        <rdfs:comment xml:lang="it">Il Liverpool Football Club, o noto più comunemente solo come Liverpool, è una società calcistica inglese con sede a Liverpool; milita nella Premier League, della quale è stata uno dei fondatori, ed è affiliato alla Football Association.</rdfs:comment>
        <rdfs:comment xml:lang="en">Liverpool Football Club is a professional football club in Liverpool, England, that competes in the Premier League, the top tier of English football. Domestically, the club has won nineteen League titles, seven FA Cups, a record eight League Cups and fifteen FA Community Shields. In international competitions, the club has won six European Cups, more than any other English club, three UEFA Cups, four UEFA Super Cups (also English records) and one FIFA Club World Cup.</rdfs:comment>
        <rdfs:label xml:lang="en">Liverpool F.C</rdfs:label>
        <rdfs:label xml:lang="it">Liverpool Football Club</rdfs:label>
    </owl:NamedIndividual>
    


    <!-- http://www.semanticweb.org/2021/ontologies/calcio#ManchesterCity -->

    <owl:NamedIndividual rdf:about="http://www.semanticweb.org/2021/ontologies/calcio#ManchesterCity">
        <rdf:type rdf:resource="http://www.semanticweb.org/2021/ontologies/calcio#squadraDiClub"/>
        <appartieneALega rdf:resource="http://www.semanticweb.org/2021/ontologies/calcio#PremierLeague"/>
        <rdfs:comment xml:lang="it">Il Manchester City Football Club, più comunemente noto come Manchester City, è una società calcistica inglese con sede nella città di Manchester, militante in Premier League, la massima divisione del campionato inglese.</rdfs:comment>
        <rdfs:comment xml:lang="en">Manchester City Football Club is an English football club based in Manchester that competes in the Premier League, the top flight of English football. Founded in 1880 as St. Mark&apos;s (West Gorton), it became Ardwick Association Football Club in 1887 and Manchester City in 1894. The club&apos;s home ground is the City of Manchester Stadium in east Manchester, to which it moved in 2003, having played at Maine Road since 1923. The club adopted their sky blue home shirts in 1894 in the first season of the club&apos;s current iteration, that have been used ever since.[4]</rdfs:comment>
        <rdfs:label xml:lang="en">Manchester City F.C</rdfs:label>
        <rdfs:label xml:lang="it">Manchester City Football Club</rdfs:label>
    </owl:NamedIndividual>
    


    <!-- http://www.semanticweb.org/2021/ontologies/calcio#ManchesterUnited -->

    <owl:NamedIndividual rdf:about="http://www.semanticweb.org/2021/ontologies/calcio#ManchesterUnited">
        <rdf:type rdf:resource="http://www.semanticweb.org/2021/ontologies/calcio#squadraDiClub"/>
        <appartieneALega rdf:resource="http://www.semanticweb.org/2021/ontologies/calcio#PremierLeague"/>
        <giocaInStadio rdf:resource="http://www.semanticweb.org/2021/ontologies/calcio#Old_Trafford"/>
        <rdfs:comment xml:lang="it">Il Manchester United Football Club (NYSE: MANU), noto semplicemente come Manchester United, è una società calcistica inglese con sede nella città di Manchester. Milita in Premier League, la massima serie del campionato inglese di calcio, dal 1975.</rdfs:comment>
        <rdfs:comment xml:lang="en">Manchester United Football Club is a professional football club based in Old Trafford, Greater Manchester, England, that competes in the Premier League, the top flight of English football. Nicknamed &quot;the Red Devils&quot;, the club was founded as Newton Heath LYR Football Club in 1878, changed its name to Manchester United in 1902 and moved to its current stadium, Old Trafford, in 1910.</rdfs:comment>
        <rdfs:label xml:lang="en">Manchester United F.C.</rdfs:label>
        <rdfs:label xml:lang="it">Manchester United Football Club</rdfs:label>
    </owl:NamedIndividual>
    


    <!-- http://www.semanticweb.org/2021/ontologies/calcio#Marsiglia -->

    <owl:NamedIndividual rdf:about="http://www.semanticweb.org/2021/ontologies/calcio#Marsiglia">
        <rdf:type rdf:resource="http://www.semanticweb.org/2021/ontologies/calcio#squadraDiClub"/>
        <rdfs:comment xml:lang="it">L&apos;Olympique de Marseille, noto in italiano come Olympique Marsiglia o semplicemente Marsiglia, è una società calcistica francese con sede nella città di Marsiglia, militante in Ligue 1, la massima divisione del campionato francese di calcio. Gioca le proprie partite casalinghe allo stadio Vélodrome, impianto da oltre 67 000 posti a sedere.</rdfs:comment>
        <rdfs:comment xml:lang="en">Olympique de Marseille (French pronunciation: ​[ɔlɛ̃pik də maʁsɛj], locally [ɔlɛ̃ˈpikə də maχˈsɛjə]; Occitan: Olimpic de Marselha, pronounced [ulimˈpi de maʀˈsejɔ]), also known as OM (IPA: [o.ɛm], locally [oˈɛmə]) or simply Marseille, is a French professional football club based in Marseille. Founded in 1899, the club plays in Ligue 1 and have spent most of their history in the top tier of French football. The club has won ten official league titles (nine times in Ligue 1), ten Coupes de France and three Coupes de la Ligue. In 1993, coach Raymond Goethals led the team to become the first and only French club to win the UEFA Champions League, defeating AC Milan 1–0 in the final. In 2010, Marseille won its first Ligue 1 title in 18 years under the management of former club captain Didier Deschamps.[2]</rdfs:comment>
        <rdfs:label xml:lang="en">Olympique de Marseille</rdfs:label>
        <rdfs:label xml:lang="it">Olympique de Marseille</rdfs:label>
    </owl:NamedIndividual>
    


    <!-- http://www.semanticweb.org/2021/ontologies/calcio#Massimiliano_Irrati -->

    <owl:NamedIndividual rdf:about="http://www.semanticweb.org/2021/ontologies/calcio#Massimiliano_Irrati">
        <rdf:type rdf:resource="http://www.semanticweb.org/2021/ontologies/calcio#Arbitro"/>
        <rdfs:comment xml:lang="it">Massimiliano Irrati (Firenze, 27 giugno 1979) è un arbitro di calcio italiano.</rdfs:comment>
        <rdfs:comment xml:lang="en">Massimiliano Irrati (Italian pronunciation: [massimiˈljaːno irˈraːti]; born 27 June 1979) is an Italian football referee.</rdfs:comment>
        <rdfs:label xml:lang="en">Massimiliano Irrati</rdfs:label>
        <rdfs:label xml:lang="it">Massimiliano Irrati</rdfs:label>
    </owl:NamedIndividual>
    


    <!-- http://www.semanticweb.org/2021/ontologies/calcio#MondialePerClub -->

    <owl:NamedIndividual rdf:about="http://www.semanticweb.org/2021/ontologies/calcio#MondialePerClub">
        <rdf:type rdf:resource="http://www.semanticweb.org/2021/ontologies/calcio#Trofeo"/>
        <rdfs:comment xml:lang="it">La Coppa del mondo per club FIFA (in inglese FIFA Club World Cup) è una competizione calcistica per club che assegna il titolo di campione del mondo.</rdfs:comment>
        <rdfs:comment xml:lang="en">The FIFA Club World Cup is an international men&apos;s association football competition organised by the Fédération Internationale de Football Association (FIFA), the sport&apos;s global governing body. The competition was first contested in 2000 as the FIFA Club World Championship. It was not held from 2001 to 2004 due to a combination of factors, most importantly the collapse of FIFA&apos;s marketing partner International Sport and Leisure (ISL), but since 2005 it has been held every year, and has been hosted by Brazil, Japan, the United Arab Emirates, Morocco and Qatar. Views differ as to the cup&apos;s prestige: it struggles to attract interest in most of Europe, and is the object of heated debate in Brazil and Argentina.</rdfs:comment>
        <rdfs:label xml:lang="it">Coppa del mondo per club FIFA</rdfs:label>
        <rdfs:label xml:lang="en">FIFA Club World Cup</rdfs:label>
    </owl:NamedIndividual>
    


    <!-- http://www.semanticweb.org/2021/ontologies/calcio#Neymar -->

    <owl:NamedIndividual rdf:about="http://www.semanticweb.org/2021/ontologies/calcio#Neymar">
        <rdf:type rdf:resource="http://www.semanticweb.org/2021/ontologies/calcio#Calciatore"/>
        <giocaPer rdf:resource="http://www.semanticweb.org/2021/ontologies/calcio#ParisSaintGermain"/>
        <haEtà rdf:datatype="http://www.w3.org/2001/XMLSchema#integer">28</haEtà>
        <haNazionalità>Brasile</haNazionalità>
        <haNome>Neymar da Silva Santos Júnior</haNome>
        <stipendioCorrente rdf:datatype="http://www.w3.org/2001/XMLSchema#long">67000000</stipendioCorrente>
        <rdfs:comment xml:lang="en">Neymar da Silva Santos Júnior (Brazilian Portuguese: [nejˈmaʁ dɐ ˈsiwvɐ ˈsɐ̃tus ˈʒũɲoʁ]; born 5 February 1992), known as Neymar, is a Brazilian professional footballer who plays as a forward for Ligue 1 club Paris Saint-Germain and the Brazil national team. He is widely regarded as one of the best players in the world.</rdfs:comment>
        <rdfs:comment xml:lang="it">Neymar da Silva Santos Júnior, noto come Neymar o Neymar Jr. (Mogi das Cruzes, 5 febbraio 1992), è un calciatore brasiliano, attaccante del Paris Saint-Germain e della nazionale brasiliana.</rdfs:comment>
        <rdfs:label xml:lang="en">Neymar</rdfs:label>
        <rdfs:label xml:lang="it">Neymar</rdfs:label>
    </owl:NamedIndividual>
    


    <!-- http://www.semanticweb.org/2021/ontologies/calcio#Old_Trafford -->

    <owl:NamedIndividual rdf:about="http://www.semanticweb.org/2021/ontologies/calcio#Old_Trafford">
        <rdf:type rdf:resource="http://www.semanticweb.org/2021/ontologies/calcio#Stadio"/>
        <haCapienza rdf:datatype="http://www.w3.org/2001/XMLSchema#integer">76000</haCapienza>
        <rdfs:comment xml:lang="it">L&apos;Old Trafford è uno stadio calcistico inglese di Manchester, situato nel quartiere omonimo della città di Trafford (Greater Manchester). Ospita le partite casalinghe del Manchester United fin dal 1910.</rdfs:comment>
        <rdfs:comment xml:lang="en">Old Trafford (/ˈtræfərd/) is a football stadium in Old Trafford, Greater Manchester, England, and the home of Manchester United. With a capacity of 74,140 seats,[1] it is the largest club football stadium (and second-largest football stadium overall after Wembley Stadium) in the United Kingdom, and the eleventh-largest in Europe.[2] It is about 0.5 miles (800 m) from Old Trafford Cricket Ground and the adjacent tram stop.</rdfs:comment>
        <rdfs:label xml:lang="en">Old Trafford</rdfs:label>
        <rdfs:label xml:lang="it">Old Trafford</rdfs:label>
    </owl:NamedIndividual>
    


    <!-- http://www.semanticweb.org/2021/ontologies/calcio#Paolo_Maldini -->

    <owl:NamedIndividual rdf:about="http://www.semanticweb.org/2021/ontologies/calcio#Paolo_Maldini">
        <rdf:type rdf:resource="http://www.semanticweb.org/2021/ontologies/calcio#Dirigente"/>
        <collegaDi rdf:resource="http://www.semanticweb.org/2021/ontologies/calcio#Stefano_Pioli"/>
        <lavoraPer rdf:resource="http://www.semanticweb.org/2021/ontologies/calcio#ACMilan"/>
        <haEtà rdf:datatype="http://www.w3.org/2001/XMLSchema#integer">52</haEtà>
        <haNazionalità>Italia</haNazionalità>
        <haNome>Paolo Maldini</haNome>
        <rdfs:comment xml:lang="en">Paolo Cesare Maldini (Italian pronunciation: [ˈpaːolo malˈdiːni]; born 26 June 1968) is an Italian former professional footballer who played as a left back and central defender for A.C. Milan and the Italy national team. He is widely regarded as one of the greatest ever defenders, with some considering him to be the best ever, and as one of the greatest players of all time.[6][7][8][9][10][11] As the Milan and Italy captain for many years he was nicknamed &quot;Il Capitano&quot; (&quot;The Captain&quot;). Maldini held the record for most appearances in Serie A, with 647, until 2020, when he was overtaken by Gianluigi Buffon.[12] He is currently serving as technical director for Milan, as well as being co-owner of USL Championship club Miami FC.</rdfs:comment>
        <rdfs:comment xml:lang="it">Paolo Cesare Maldini (Milano, 26 giugno 1968) è un dirigente sportivo ed ex calciatore italiano, di ruolo difensore, direttore tecnico del Milan. È stato vicecampione del mondo nel 1994 e vicecampione d&apos;Europa nel 2000 con la nazionale italiana.</rdfs:comment>
        <rdfs:label xml:lang="en">Paolo Maldini</rdfs:label>
        <rdfs:label xml:lang="it">Paolo Maldini</rdfs:label>
    </owl:NamedIndividual>
    


    <!-- http://www.semanticweb.org/2021/ontologies/calcio#ParisSaintGermain -->

    <owl:NamedIndividual rdf:about="http://www.semanticweb.org/2021/ontologies/calcio#ParisSaintGermain">
        <appartieneALega rdf:resource="http://www.semanticweb.org/2021/ontologies/calcio#Ligue1"/>
        <giocaInStadio rdf:resource="http://www.semanticweb.org/2021/ontologies/calcio#Le_Parc_des_Princes"/>
        <rdfs:comment xml:lang="it">Il Paris Saint-Germain Football Club (pronuncia francese: /paʁi sɛ̃ ʒɛʁmɛ̃/), meglio conosciuto come Paris Saint-Germain o più semplicemente con la sigla PSG, è una società calcistica francese con sede a Parigi e a Saint-Germain-en-Laye.</rdfs:comment>
        <rdfs:comment xml:lang="en">Paris Saint-Germain Football Club (French pronunciation: ​[paʁi sɛ̃ ʒɛʁmɛ̃]), commonly referred to as Paris Saint-Germain, Paris SG, or simply Paris or PSG, is a French professional football club based in Paris. They compete in Ligue 1, the top division of French football. PSG are France&apos;s most successful club, having won more than 40 official honours, including nine league titles and one major European trophy. Their home ground is the Parc des Princes.</rdfs:comment>
        <rdfs:label xml:lang="en">Paris Saint-Germain F.C.</rdfs:label>
        <rdfs:label xml:lang="it">Paris Saint-Germain Football Club</rdfs:label>
    </owl:NamedIndividual>
    


    <!-- http://www.semanticweb.org/2021/ontologies/calcio#Pierre_Kalulu -->

    <owl:NamedIndividual rdf:about="http://www.semanticweb.org/2021/ontologies/calcio#Pierre_Kalulu">
        <giocaPer rdf:resource="http://www.semanticweb.org/2021/ontologies/calcio#ACMilan"/>
        <rdfs:comment xml:lang="en">Pierre Kalulu Kyatengwa (born 5 June 2000) is a French professional footballer, who plays for Serie A club A.C. Milan as a defender; mainly a right-back, he can also play in central defense.</rdfs:comment>
        <rdfs:comment xml:lang="it">Pierre Kazaye Kalulu Kyatengwa (Lione, 5 giugno 2000) è un calciatore francese con cittadinanza della Repubblica Democratica del Congo, difensore del Milan.</rdfs:comment>
        <rdfs:label xml:lang="en">Pierre Kalulu</rdfs:label>
        <rdfs:label xml:lang="it">Pierre Kalulu</rdfs:label>
    </owl:NamedIndividual>
    


    <!-- http://www.semanticweb.org/2021/ontologies/calcio#Portogallo -->

    <owl:NamedIndividual rdf:about="http://www.semanticweb.org/2021/ontologies/calcio#Portogallo">
        <rdf:type rdf:resource="http://www.semanticweb.org/2021/ontologies/calcio#squadraNazionale"/>
        <rdfs:comment xml:lang="it">La nazionale di calcio del Portogallo è la rappresentativa calcistica del Portogallo ed è gestita dalla Federação Portuguesa de Futebol. Nella sua bacheca figurano un campionato europeo e l&apos;edizione inaugurale della UEFA Nations League.</rdfs:comment>
        <rdfs:comment xml:lang="en">The Portugal national football team (Portuguese: Seleção Portuguesa de Futebol) has represented Portugal in international men&apos;s football competition since 1921. It is controlled by the Portuguese Football Federation, the governing body for football in Portugal.</rdfs:comment>
        <rdfs:label xml:lang="it">Nazionale di calcio del Portogallo</rdfs:label>
        <rdfs:label xml:lang="en">Portugal national football team</rdfs:label>
    </owl:NamedIndividual>
    


    <!-- http://www.semanticweb.org/2021/ontologies/calcio#PremierLeague -->

    <owl:NamedIndividual rdf:about="http://www.semanticweb.org/2021/ontologies/calcio#PremierLeague">
        <rdfs:comment xml:lang="it">La Premier League, nota anche come English Premier League, abbreviato EPL, al di fuori dell&apos;Inghilterra; è la massima serie del campionato inglese di calcio.[1] La Premier nacque il 20 febbraio 1992, dopo che le 22 squadre affiliate alla First Division (l&apos;allora massimo campionato inglese) decisero di uscire dalla Football League per ragioni economiche.</rdfs:comment>
        <rdfs:comment xml:lang="en">The Premier League, often referred to outside the British Isles as the English Premier League, or sometimes the EPL, is the top level of the English football league system. Contested by 20 clubs, it operates on a system of promotion and relegation with the English Football League (EFL). Seasons run from August to May with each team playing 38 matches (playing all 19 other teams both home and away).[1] Most games are played on Saturday and Sunday afternoons.</rdfs:comment>
        <rdfs:label xml:lang="en">Premier League</rdfs:label>
        <rdfs:label xml:lang="it">Premier League</rdfs:label>
    </owl:NamedIndividual>
    


    <!-- http://www.semanticweb.org/2021/ontologies/calcio#RBLeipzig -->

    <owl:NamedIndividual rdf:about="http://www.semanticweb.org/2021/ontologies/calcio#RBLeipzig">
        <rdf:type rdf:resource="http://www.semanticweb.org/2021/ontologies/calcio#squadraDiClub"/>
        <rdfs:comment xml:lang="it">Il RasenBallsport Leipzig, meglio noto come RB Leipzig e in italiano come Lipsia o RB Lipsia (nonché impropriamente come Red Bull Lipsia), è una società calcistica tedesca con sede nella città di Lipsia, in Sassonia. Milita nella Bundesliga, la massima serie del campionato tedesco di calcio.</rdfs:comment>
        <rdfs:comment xml:lang="en">RasenBallsport Leipzig e.V. (lit. &apos;Lawn Ball Sports Leipzig&apos;), commonly known as RB Leipzig, is a German professional football club based in Leipzig, Saxony. The club was founded in 2009 by the initiative of the company Red Bull GmbH, which purchased the playing rights of fifth-tier side SSV Markranstädt with the intent of advancing the new club to the top-flight Bundesliga within eight years. The men&apos;s professional football club is run by the spin-off organization RasenBallsport Leipzig GmbH.[1] RB Leipzig plays its home matches at the Red Bull Arena.</rdfs:comment>
        <rdfs:label xml:lang="en">RB Leipzig</rdfs:label>
        <rdfs:label xml:lang="it">RB Leipzig</rdfs:label>
    </owl:NamedIndividual>
    


    <!-- http://www.semanticweb.org/2021/ontologies/calcio#Rafael_Leão -->

    <owl:NamedIndividual rdf:about="http://www.semanticweb.org/2021/ontologies/calcio#Rafael_Leão">
        <giocaPer rdf:resource="http://www.semanticweb.org/2021/ontologies/calcio#ACMilan"/>
        <rdfs:comment xml:lang="en">Rafael Alexandre Conceição Leão is a Portuguese professional footballer who plays for Italian club A.C. Milan as a forward.</rdfs:comment>
        <rdfs:comment xml:lang="it">Rafael Alexandre da Conceição Leão, noto semplicemente come Rafael Leão (Almada, 10 giugno 1999), è un calciatore portoghese di origini angolane, attaccante del Milan e della nazionale Under-21 portoghese.</rdfs:comment>
        <rdfs:label xml:lang="en">Rafael Leão</rdfs:label>
        <rdfs:label xml:lang="it">Rafael Leão</rdfs:label>
    </owl:NamedIndividual>
    


    <!-- http://www.semanticweb.org/2021/ontologies/calcio#RealMadrid -->

    <owl:NamedIndividual rdf:about="http://www.semanticweb.org/2021/ontologies/calcio#RealMadrid">
        <rdf:type rdf:resource="http://www.semanticweb.org/2021/ontologies/calcio#squadraDiClub"/>
        <appartieneALega rdf:resource="http://www.semanticweb.org/2021/ontologies/calcio#LaLiga"/>
        <giocaInStadio rdf:resource="http://www.semanticweb.org/2021/ontologies/calcio#Santiago_Bernabéu_Stadium"/>
        <rdfs:comment xml:lang="it">Il Real Madrid Club de Fútbol, conosciuto semplicemente come Real Madrid, è una società polisportiva spagnola con sede nella città di Madrid, nota soprattutto per la sua sezione calcistica. Fondata a Madrid il 6 marzo 1902 con la denominazione ufficiale di Madrid Club de Fútbol, si vide assegnare il titolo di Real nel 1920 dal re Alfonso XIII di Spagna, insieme alla nota corona a decorarne lo stemma.</rdfs:comment>
        <rdfs:comment xml:lang="en">Real Madrid Club de Fútbol (Spanish pronunciation: [reˈal maˈðɾið ˈkluβ ðe ˈfuðβol] (About this soundlisten), meaning Royal Madrid Football Club), commonly referred to as Real Madrid, is a Spanish professional football club based in Madrid.</rdfs:comment>
        <rdfs:label xml:lang="en">Real Madrid CF</rdfs:label>
        <rdfs:label xml:lang="it">Real Madrid Club de Fútbol</rdfs:label>
    </owl:NamedIndividual>
    


    <!-- http://www.semanticweb.org/2021/ontologies/calcio#Roberto_Mancini -->

    <owl:NamedIndividual rdf:about="http://www.semanticweb.org/2021/ontologies/calcio#Roberto_Mancini">
        <allenaSquadraNazionale rdf:resource="http://www.semanticweb.org/2021/ontologies/calcio#Italia"/>
        <rdfs:comment xml:lang="en">Roberto Mancini (Italian pronunciation: [roˈbɛrto manˈtʃiːni]; born 27 November 1964) is an Italian football manager and former player who is the manager of the Italy national team. As a player, Mancini operated as a deep-lying forward, and was best known for his time at Sampdoria, where he played more than 550 matches, and helped the team win the Serie A league title, four Coppa Italia titles, and the European Cup Winners&apos; Cup. He was capped 36 times for Italy, taking part at UEFA Euro 1988 and the 1990 FIFA World Cup, achieving semi-final finishes in both tournaments. In 1997, after 15 years at Sampdoria, Mancini left the club to join Lazio, where he won a further Scudetto, as well as the Cup Winners&apos; Cup, the UEFA Super Cup and two more Coppa Italia titles.</rdfs:comment>
        <rdfs:comment xml:lang="it">Roberto Mancini (Jesi, 27 novembre 1964) è un allenatore di calcio ed ex calciatore italiano, di ruolo centrocampista o attaccante, commissario tecnico della nazionale italiana.</rdfs:comment>
        <rdfs:label xml:lang="en">Roberto Mancini</rdfs:label>
        <rdfs:label xml:lang="it">Roberto Mancini</rdfs:label>
    </owl:NamedIndividual>
    


    <!-- http://www.semanticweb.org/2021/ontologies/calcio#Roma -->

    <owl:NamedIndividual rdf:about="http://www.semanticweb.org/2021/ontologies/calcio#Roma">
        <rdf:type rdf:resource="http://www.semanticweb.org/2021/ontologies/calcio#squadraDiClub"/>
        <appartieneALega rdf:resource="http://www.semanticweb.org/2021/ontologies/calcio#SerieA"/>
        <rdfs:comment xml:lang="en">Associazione Sportiva Roma (BIT: ASR, LSE: 0MT1; Rome Sport Association), commonly referred to as Roma (Italian pronunciation: [ˈroːma]), is an Italian professional football club based in Rome. Founded by a merger in 1927, Roma have participated in the top-tier of Italian football for all of their existence except for 1951–52 season. Roma have won Serie A three times, in 1941–42, 1982–83 and 2000–01, as well as winning nine Coppa Italia titles and two Supercoppa Italiana titles. In European competitions, Roma won the Inter-Cities Fairs Cup in 1960–61 and were runners-up in the 1983–84 European Cup and the 1990–91 UEFA Cup.</rdfs:comment>
        <rdfs:comment xml:lang="it">L&apos;Associazione Sportiva Roma (AFI: /assoʧaʦˈʦjone sporˈtiva ˈroma/), nota anche come AS Roma o, più semplicemente, Roma, è una società calcistica italiana con sede nella città di Roma. Nella stagione 2020-2021 milita nel campionato di Serie A, massimo livello della piramide calcistica italiana.</rdfs:comment>
        <rdfs:label xml:lang="en">A.S. Roma</rdfs:label>
        <rdfs:label xml:lang="it">Associazione Sportiva Roma</rdfs:label>
    </owl:NamedIndividual>
    


    <!-- http://www.semanticweb.org/2021/ontologies/calcio#Ronald_Koeman -->

    <owl:NamedIndividual rdf:about="http://www.semanticweb.org/2021/ontologies/calcio#Ronald_Koeman">
        <rdfs:comment xml:lang="en">Ronald Koeman (Dutch pronunciation: [ˈroːnɑlt ˈkumɑn] (About this soundlisten); born 21 March 1963) is a Dutch professional football manager and former player, who is the current head coach of La Liga club FC Barcelona. He is the younger brother of his former international teammate Erwin Koeman and the son of former Dutch international Martin Koeman. Koeman was capable of playing both as a defender and as a midfielder; he frequently played as a sweeper, although he was equally known for his goalscoring, long–range shooting, and accuracy from free kicks and penalties.</rdfs:comment>
        <rdfs:comment xml:lang="it">Ronald Koeman (Zaandam, 21 marzo 1963) è un allenatore di calcio ed ex calciatore olandese, di ruolo difensore o centrocampista, tecnico del Barcellona. È stato campione d&apos;Europa con i Paesi Bassi nel 1988.</rdfs:comment>
        <rdfs:label xml:lang="en">Ronald Koeman</rdfs:label>
        <rdfs:label xml:lang="it">Ronald Koeman</rdfs:label>
    </owl:NamedIndividual>
    


    <!-- http://www.semanticweb.org/2021/ontologies/calcio#Rosario_Abisso -->

    <owl:NamedIndividual rdf:about="http://www.semanticweb.org/2021/ontologies/calcio#Rosario_Abisso">
        <arbitraIn rdf:resource="http://www.semanticweb.org/2021/ontologies/calcio#SerieA"/>
        <haEtà rdf:datatype="http://www.w3.org/2001/XMLSchema#integer">35</haEtà>
        <haNazionalità>Italia</haNazionalità>
        <haNome>Rosario Abisso</haNome>
        <rdfs:comment xml:lang="en">Rosario Abisso is an italian refree</rdfs:comment>
        <rdfs:comment xml:lang="it">Rosario Abisso è un arbitro di calcio italiano.</rdfs:comment>
        <rdfs:label xml:lang="en">Rosario Abisso</rdfs:label>
        <rdfs:label xml:lang="it">Rosario Abisso</rdfs:label>
    </owl:NamedIndividual>
    


    <!-- http://www.semanticweb.org/2021/ontologies/calcio#Samu_Castillejo -->

    <owl:NamedIndividual rdf:about="http://www.semanticweb.org/2021/ontologies/calcio#Samu_Castillejo">
        <giocaPer rdf:resource="http://www.semanticweb.org/2021/ontologies/calcio#ACMilan"/>
        <rdfs:comment xml:lang="en">Samuel Castillejo Azuaga (born 18 January 1995) is a Spanish professional footballer who plays as a winger for Italian club A.C. Milan.</rdfs:comment>
        <rdfs:comment xml:lang="it">Samuel Castillejo Azuaga, conosciuto come Samu Castillejo (Malaga, 18 gennaio 1995), è un calciatore spagnolo, attaccante del Milan.</rdfs:comment>
        <rdfs:label xml:lang="en">Samu Castillejo</rdfs:label>
        <rdfs:label xml:lang="it">Samu Castillejo</rdfs:label>
    </owl:NamedIndividual>
    


    <!-- http://www.semanticweb.org/2021/ontologies/calcio#San_Siro -->

    <owl:NamedIndividual rdf:about="http://www.semanticweb.org/2021/ontologies/calcio#San_Siro">
        <rdf:type rdf:resource="http://www.semanticweb.org/2021/ontologies/calcio#Stadio"/>
        <haCapienza rdf:datatype="http://www.w3.org/2001/XMLSchema#int">80018</haCapienza>
        <vann:preferredNamespaceUri xml:lang="it">Lo stadio Giuseppe Meazza è un impianto calcistico italiano di proprietà del comune di Milano, che ospita le gare interne del Milan e dell&apos;Inter.

In ragione del quartiere dove sorge, è noto anche come stadio San Siro, nome che ebbe ufficialmente dal 19 settembre 1926 (giorno dell&apos;inaugurazione)[1] al 3 marzo 1980, quando fu intitolato alla memoria di Giuseppe Meazza, gloria del calcio milanese e italiano.</vann:preferredNamespaceUri>
        <rdfs:comment xml:lang="en">San Siro, officially known as Stadio Giuseppe Meazza, is a football stadium in the San Siro district of Milan, which is the home of A.C. Milan and Internazionale. It has a seating capacity of 75,923, making it one of the largest stadiums in Europe, and the largest in Italy.</rdfs:comment>
        <rdfs:label xml:lang="en">San Siro</rdfs:label>
        <rdfs:label xml:lang="it">Stadio Giuseppe Meazza</rdfs:label>
    </owl:NamedIndividual>
    


    <!-- http://www.semanticweb.org/2021/ontologies/calcio#Sandro_Tonali -->

    <owl:NamedIndividual rdf:about="http://www.semanticweb.org/2021/ontologies/calcio#Sandro_Tonali">
        <rdf:type rdf:resource="http://dbpedia.org/ontology/SoccerPlayer"/>
        <giocaPer rdf:resource="http://www.semanticweb.org/2021/ontologies/calcio#ACMilan"/>
        <rdfs:comment xml:lang="en">Sandro Tonali (Italian pronunciation: [ˈsandro toˈnaːli]; born 8 May 2000) is an Italian professional footballer who plays as a midfielder for Serie A club Milan, on loan from Brescia, and the Italy national football team.</rdfs:comment>
        <rdfs:comment xml:lang="it">Sandro Tonali (Lodi, 8 maggio 2000) è un calciatore italiano, centrocampista del Milan, in prestito dal Brescia, della nazionale italiana e della nazionale Under-21 italiana.</rdfs:comment>
        <rdfs:label xml:lang="en">Sandro Tonali</rdfs:label>
        <rdfs:label xml:lang="it">Sandro Tonali</rdfs:label>
    </owl:NamedIndividual>
    


    <!-- http://www.semanticweb.org/2021/ontologies/calcio#Santiago_Bernabéu_Stadium -->

    <owl:NamedIndividual rdf:about="http://www.semanticweb.org/2021/ontologies/calcio#Santiago_Bernabéu_Stadium">
        <rdf:type rdf:resource="http://www.semanticweb.org/2021/ontologies/calcio#Stadio"/>
        <haCapienza rdf:datatype="http://www.w3.org/2001/XMLSchema#integer">81044</haCapienza>
        <rdfs:comment xml:lang="it">Lo stadio Santiago Bernabéu (in spagnolo Estadio Santiago Bernabéu) è un impianto calcistico spagnolo di Madrid. Di proprietà del Real Madrid Club de Fútbol, ospita gli incontri casalinghi della sua prima squadra dal 1947.</rdfs:comment>
        <rdfs:comment xml:lang="en">The Santiago Bernabéu Stadium (Spanish: Estadio Santiago Bernabéu, [esˈtaðjo sanˈtjaɣo βeɾnaˈβew] is a football stadium in Madrid, Spain. With a current seating capacity of 81,044,[5] it has been the home stadium of Real Madrid since its completion in 1947.[2] It is the second-largest stadium in Spain and largest in the Community of Madrid.</rdfs:comment>
        <rdfs:label xml:lang="en">Santiago Bernabéu Stadium</rdfs:label>
        <rdfs:label xml:lang="it">Stadio Santiago Bernabéu</rdfs:label>
    </owl:NamedIndividual>
    


    <!-- http://www.semanticweb.org/2021/ontologies/calcio#SegundaDivisión -->

    <owl:NamedIndividual rdf:about="http://www.semanticweb.org/2021/ontologies/calcio#SegundaDivisión">
        <rdfs:comment xml:lang="it">La Segunda División (in lingua spagnola Seconda Divisione) è per importanza il secondo campionato professionistico del calcio spagnolo. È gestita dalla Liga de Fútbol Profesional (LFP).</rdfs:comment>
        <rdfs:comment xml:lang="en">The Campeonato Nacional de Liga de Segunda División,[a] commercially known as LaLiga 2[b] and stylized as LaLiga SmartBank for sponsorship reasons,[1] is the men&apos;s second professional association football division of the Spanish football league system. Administrated by the Liga de Fútbol Profesional, it is contested by 22 teams, with the top two teams plus the winner of a play-off promoted to LaLiga and replaced by the three lowest-placed teams in that division.</rdfs:comment>
        <rdfs:label xml:lang="en">Segunda División</rdfs:label>
        <rdfs:label xml:lang="it">Segunda División</rdfs:label>
    </owl:NamedIndividual>
    


    <!-- http://www.semanticweb.org/2021/ontologies/calcio#SerieA -->

    <owl:NamedIndividual rdf:about="http://www.semanticweb.org/2021/ontologies/calcio#SerieA">
        <numeroSquadre rdf:datatype="http://www.w3.org/2001/XMLSchema#int">20</numeroSquadre>
        <numeroSquadreRetrocesse rdf:datatype="http://www.w3.org/2001/XMLSchema#int">3</numeroSquadreRetrocesse>
        <numeroSquadreTop rdf:datatype="http://www.w3.org/2001/XMLSchema#int">4</numeroSquadreTop>
        <rdfs:comment xml:lang="it">La Serie A, ufficialmente chiamata Serie A TIM per ragioni di sponsorizzazione,[1] è il più alto livello professionistico del campionato italiano di calcio.[2] Viene gestito dalla Lega Nazionale Professionisti Serie A.</rdfs:comment>
        <rdfs:comment xml:lang="en">Serie A (Italian pronunciation: [ˈsɛːrje ˈa]), also called Serie A TIM due to sponsorship by TIM,[1] is a professional league competition for football clubs located at the top of the Italian football league system and the winner is awarded the Scudetto and the Coppa Campioni d&apos;Italia. It has been operating as a round-robin tournament for over ninety years since the 1929–30 season. It had been organized by the Direttorio Divisioni Superiori until 1943 and the Lega Calcio until 2010, when the Lega Serie A was created for the 2010–11 season. Serie A is regarded as one of the best football leagues in the world and it is often depicted as the most tactical and defensively sound national league.[2] Serie A was the world&apos;s strongest national league in 2020 according to IFFHS,[3] and is ranked third among European leagues according to UEFA&apos;s league coefficient, behind La Liga and the Premier League and ahead of the Bundesliga and Ligue 1, which is based on the performance of Italian clubs in the Champions League and the Europa League during the previous five years.[4] Serie A led the UEFA ranking from 1986 to 1988 and from 1990 to 1999.</rdfs:comment>
        <rdfs:label xml:lang="en">Serie A</rdfs:label>
        <rdfs:label xml:lang="it">Serie A</rdfs:label>
    </owl:NamedIndividual>
    


    <!-- http://www.semanticweb.org/2021/ontologies/calcio#SerieB -->

    <owl:NamedIndividual rdf:about="http://www.semanticweb.org/2021/ontologies/calcio#SerieB">
        <rdfs:comment xml:lang="it">La Serie B, ufficialmente nota come Serie BKT per ragioni di sponsorizzazione[2], è il secondo livello professionistico del campionato italiano di calcio, gestito dalla Lega Nazionale Professionisti B.</rdfs:comment>
        <rdfs:comment xml:lang="en">Serie B (Italian pronunciation: [ˈsɛːrje ˈbi]), currently named Serie BKT for sponsorship reasons,[1] is the second-highest division in the Italian football league system after the Serie A. It has been operating for over ninety years since the 1929–30 season. It had been organized by Lega Calcio until 2010, when the Lega Serie B was created for the 2010–11 season. Common nicknames for the league are campionato cadetto and cadetteria, since cadetto is the Italian name for junior or cadet.</rdfs:comment>
        <rdfs:label xml:lang="en">Serie B</rdfs:label>
        <rdfs:label xml:lang="it">Serie B</rdfs:label>
    </owl:NamedIndividual>
    


    <!-- http://www.semanticweb.org/2021/ontologies/calcio#SerieC -->

    <owl:NamedIndividual rdf:about="http://www.semanticweb.org/2021/ontologies/calcio#SerieC">
        <rdfs:comment xml:lang="it">La Serie C è il terzo livello del campionato italiano di calcio, il più basso a carattere professionistico.

Dal 2014 è l&apos;unico campionato organizzato dalla Lega Italiana Calcio Professionistico, dopo l&apos;unificazione tra Prima e Seconda Divisione in una divisione unica denominata Lega Pro fino al 2017, che ha ripristinato il formato esistente fra il 1935 e il 1978 (anno in cui la C si scisse nelle Serie C1 e C2).

Il 25 maggio 2017 l&apos;assemblea di Lega Pro ha approvato all&apos;unanimità il ritorno alla denominazione originaria, in quanto è stato ritenuto il nome originario quello più rappresentativo per tifosi e appassionati.</rdfs:comment>
        <rdfs:comment xml:lang="en">Serie C (Italian pronunciation: [ˈsɛːrje ˈtʃi]) is the third-highest division in the Italian football league system after the Serie B and Serie A. The Lega Italiana Calcio Professionistico (Lega Pro) is the governing body that runs the Serie C. The unification of the Lega Pro Prima Divisione and the Lega Pro Seconda Divisione as Lega Pro Divisione Unica (often also abbreviated as Lega Pro) in 2014[1] reintroduced the format of the original Serie C that existed between 1935 and 1978 (before the split into Serie C1 and Serie C2). On 25 May 2017 the Lega Pro assembly unanimously approved the return to the original name of the competition to Serie C.</rdfs:comment>
        <rdfs:label xml:lang="en">Serie C</rdfs:label>
        <rdfs:label xml:lang="it">Serie C</rdfs:label>
    </owl:NamedIndividual>
    


    <!-- http://www.semanticweb.org/2021/ontologies/calcio#Simon_Kjær -->

    <owl:NamedIndividual rdf:about="http://www.semanticweb.org/2021/ontologies/calcio#Simon_Kjær">
        <giocaPer rdf:resource="http://www.semanticweb.org/2021/ontologies/calcio#ACMilan"/>
        <rdfs:comment xml:lang="it">Simon Thorup Kjær (Horsens, 26 marzo 1989) è un calciatore danese, difensore del Milan e della nazionale danese, di cui è capitano.</rdfs:comment>
        <rdfs:comment xml:lang="en">Simon Thorup Kjær (pronounced [ˈsimɔn ˈkʰeˀɐ̯]; born 26 March 1989) is a Danish professional footballer who plays as a centre back for Italian club Milan and captains the Denmark national team.</rdfs:comment>
        <rdfs:label xml:lang="en">Simon Kjær</rdfs:label>
        <rdfs:label xml:lang="it">Simon Kjær</rdfs:label>
    </owl:NamedIndividual>
    


    <!-- http://www.semanticweb.org/2021/ontologies/calcio#Spagna -->

    <owl:NamedIndividual rdf:about="http://www.semanticweb.org/2021/ontologies/calcio#Spagna">
        <rdf:type rdf:resource="http://www.semanticweb.org/2021/ontologies/calcio#squadraNazionale"/>
        <haVintoNazionale rdf:resource="http://www.semanticweb.org/2021/ontologies/calcio#Euro_2008"/>
        <haVintoNazionale rdf:resource="http://www.semanticweb.org/2021/ontologies/calcio#WorldCup_2010"/>
        <rdfs:comment xml:lang="it">La nazionale di calcio della Spagna (spagnolo: Selección de fútbol de España) è la rappresentativa calcistica della Spagna, controllata dalla Real Federación Española de Fútbol.</rdfs:comment>
        <rdfs:comment xml:lang="en">The Spain national football team (Spanish: Selección Española de Fútbol) represents Spain in international men&apos;s football competitions since 1920. It is governed by the Royal Spanish Football Federation, the governing body for Football in Spain.</rdfs:comment>
        <rdfs:label xml:lang="it">Nazionale di calcio della Spagna</rdfs:label>
        <rdfs:label xml:lang="en">Spain national football team</rdfs:label>
    </owl:NamedIndividual>
    


    <!-- http://www.semanticweb.org/2021/ontologies/calcio#Stefano_Pioli -->

    <owl:NamedIndividual rdf:about="http://www.semanticweb.org/2021/ontologies/calcio#Stefano_Pioli">
        <haEtà rdf:datatype="http://www.w3.org/2001/XMLSchema#integer">55</haEtà>
        <haNazionalità>Italia</haNazionalità>
        <haNome>Stefano Pioli</haNome>
        <stipendioCorrente rdf:datatype="http://www.w3.org/2001/XMLSchema#long">2300000</stipendioCorrente>
        <rdfs:comment xml:lang="en">Stefano Pioli (Italian pronunciation: [ˈsteːfano ˈpjɔːli]; born 20 October 1965) is an Italian football manager and a former footballer who played as a defender. He is the head coach at Serie A club A.C. Milan.</rdfs:comment>
        <rdfs:comment xml:lang="it">Stefano Pioli (Parma, 20 ottobre 1965) è un allenatore di calcio ed ex calciatore italiano, di ruolo difensore, tecnico del Milan.</rdfs:comment>
        <rdfs:label xml:lang="en">Stefano Pioli</rdfs:label>
        <rdfs:label xml:lang="it">Stefano Pioli</rdfs:label>
    </owl:NamedIndividual>
    


    <!-- http://www.semanticweb.org/2021/ontologies/calcio#SuperCup -->

    <owl:NamedIndividual rdf:about="http://www.semanticweb.org/2021/ontologies/calcio#SuperCup">
        <rdf:type rdf:resource="http://www.semanticweb.org/2021/ontologies/calcio#trofeoDiClub"/>
        <rdfs:comment xml:lang="it">La Supercoppa UEFA (ingl. UEFA Super Cup; fr. Supercoupe de l&apos;UEFA), comunemente denominata Supercoppa europea o Supercoppa d&apos;Europa, è una competizione calcistica continentale per squadre di club organizzata dalla UEFA, che vede in palio un trofeo conteso annualmente tra le squadre vincitrici rispettivamente della Champions League e dell&apos;Europa League.</rdfs:comment>
        <rdfs:comment xml:lang="en">The UEFA Super Cup is an annual super cup football match organised by UEFA and contested by the reigning champions of the two main European club competitions, the UEFA Champions League and the UEFA Europa League. It is not recognised as one of UEFA&apos;s &apos;major&apos; competitions.[1][2] The competition&apos;s official name was originally the European Super Cup; it was renamed the UEFA Super Cup before the 1995 edition, following a policy of rebranding by UEFA.</rdfs:comment>
        <rdfs:label xml:lang="it">Supercoppa UEFA</rdfs:label>
        <rdfs:label xml:lang="en">UEFA Super Cup</rdfs:label>
    </owl:NamedIndividual>
    


    <!-- http://www.semanticweb.org/2021/ontologies/calcio#The_UEFA_European_Football_Championship -->

    <owl:NamedIndividual rdf:about="http://www.semanticweb.org/2021/ontologies/calcio#The_UEFA_European_Football_Championship">
        <rdf:type rdf:resource="http://www.semanticweb.org/2021/ontologies/calcio#Trofeo"/>
        <rdfs:comment xml:lang="it">Il Campionato europeo di calcio UEFA (in inglese UEFA European Football Championship) è il massimo torneo calcistico europeo per squadre nazionali maschili. Ufficialmente la fase finale è nota con il nome commerciale di UEFA EURO seguito dall&apos;anno dell&apos;edizione. Nato nel 1960 da un&apos;idea del dirigente sportivo francese Henri Delaunay, è organizzato dalla UEFA e si disputa ogni quattro anni.</rdfs:comment>
        <rdfs:comment xml:lang="en">The UEFA European Football Championship,[1] commonly known as the UEFA European Championship and informally as the Euros, is the primary association football competition contested by the senior men&apos;s national teams of the members of the Union of European Football Associations (UEFA), determining the continental champion of Europe. The competition has been held every four years since 1960, except for 2020, when it was postponed due to the ongoing COVID-19 pandemic in Europe. Scheduled to be in the even-numbered year between World Cup tournaments, it was originally called the European Nations&apos; Cup, changing to the current name in 1968. Starting with the 1996 tournament, specific championships are often referred to in the form &quot;UEFA Euro [year]&quot;; this format has since been retroactively applied to earlier tournaments.</rdfs:comment>
        <rdfs:label xml:lang="it">Campionato europeo di calcio</rdfs:label>
        <rdfs:label xml:lang="en">UEFA European Championship</rdfs:label>
    </owl:NamedIndividual>
    


    <!-- http://www.semanticweb.org/2021/ontologies/calcio#Theo_Hernández -->

    <owl:NamedIndividual rdf:about="http://www.semanticweb.org/2021/ontologies/calcio#Theo_Hernández">
        <rdfs:comment xml:lang="en">Theo Bernard François Hernandez (French pronunciation: ​[teo ɛʁnɑ̃dɛz, - ɛʁnandɛs]; born 6 October 1997) is a French professional footballer who plays as a left back for Italian Serie A club A.C. Milan.</rdfs:comment>
        <rdfs:comment xml:lang="it">Theo Bernard François Hernández (Marsiglia, 6 ottobre 1997) è un calciatore francese, difensore del Milan.

Prodotto delle giovanili dell&apos;Atletico Madrid, è in seguito passato ai rivali cittadini del Real Madrid e ha fatto parte della squadra che nel 2017 si è aggiudicata la Supercoppa di Spagna, la Supercoppa UEFA e il Mondiale per Club FIFA, vincendo anche la UEFA Champions League 2017-2018. Ha anche vestito le maglie dell&apos;Alavés, della Real Sociedad; dal 2019 milita nel Milan.</rdfs:comment>
        <rdfs:label xml:lang="en">Theo Hernandez</rdfs:label>
        <rdfs:label xml:lang="it">Theo Hernández</rdfs:label>
    </owl:NamedIndividual>
    


    <!-- http://www.semanticweb.org/2021/ontologies/calcio#Villareal -->

    <owl:NamedIndividual rdf:about="http://www.semanticweb.org/2021/ontologies/calcio#Villareal">
        <rdf:type rdf:resource="http://www.semanticweb.org/2021/ontologies/calcio#squadraDiClub"/>
        <rdfs:comment xml:lang="en">Villarreal Club de Fútbol, S.A.D. (Valencian: Vila-real Club de Futbol, S.A.D.), usually abbreviated to Villarreal CF or just Villarreal, is a Spanish professional football club based in Villarreal that plays in La Liga, the top flight of Spanish football.</rdfs:comment>
        <rdfs:comment xml:lang="it">l Villarreal Club de Fútbol, meglio noto come Villarreal CF, Vila-real o più semplicemente Villarreal, è una società calcistica spagnola con sede nella città di Vila-real, nella provincia di Castellón. Milita nella Primera División, la massima serie del campionato di calcio spagnolo.</rdfs:comment>
        <rdfs:label xml:lang="en">Villarreal CF</rdfs:label>
        <rdfs:label xml:lang="it">Villarreal Club de Fútbol</rdfs:label>
    </owl:NamedIndividual>
    


    <!-- http://www.semanticweb.org/2021/ontologies/calcio#WorldCup_1934 -->

    <owl:NamedIndividual rdf:about="http://www.semanticweb.org/2021/ontologies/calcio#WorldCup_1934">
        <rdf:type rdf:resource="http://www.semanticweb.org/2021/ontologies/calcio#trofeoDiNazione"/>
        <rdfs:comment xml:lang="it">Il campionato mondiale di calcio 1934 o Coppa del mondo Jules Rimet 1934 (in inglese: World Cup Jules Rimet 1934), noto anche come Italia &apos;34, fu la seconda edizione del torneo organizzato dalla FIFA per rappresentative maschili.</rdfs:comment>
        <rdfs:comment xml:lang="en">The 1934 FIFA World Cup was the second edition of the FIFA World Cup, the quadrennial international football championship for senior men&apos;s national teams. It took place in Italy from 27 May to 10 June 1934.</rdfs:comment>
        <rdfs:label xml:lang="en">1934 FIFA World Cup</rdfs:label>
        <rdfs:label xml:lang="it">Campionato mondiale di calcio 1934</rdfs:label>
    </owl:NamedIndividual>
    


    <!-- http://www.semanticweb.org/2021/ontologies/calcio#WorldCup_1938 -->

    <owl:NamedIndividual rdf:about="http://www.semanticweb.org/2021/ontologies/calcio#WorldCup_1938">
        <rdf:type rdf:resource="http://www.semanticweb.org/2021/ontologies/calcio#trofeoDiNazione"/>
        <rdfs:comment xml:lang="it">Il campionato mondiale di calcio 1938 o Coppa del mondo Jules Rimet 1938 (in francese: Coupe du monde de football de 1938, in inglese: World Cup Jules Rimet 1938), noto anche come Francia &apos;38, fu la terza edizione del campionato mondiale di calcio per squadre nazionali maggiori maschili organizzato dalla FIFA ogni quattro anni.[1] Si disputò dal 4 al 19 giugno 1938 in Francia e fu vinto dall&apos;Italia.</rdfs:comment>
        <rdfs:comment xml:lang="en">The 1938 FIFA World Cup was the third edition of the World Cup, the quadrennial international football championship for senior men&apos;s national teams and was held in France from 4-19 June 1938. Italy defended its title in the final, beating Hungary 4–2. Italy&apos;s 1934 and 1938 teams hold the distinction of the sole World Cup champions under the same coach, Vittorio Pozzo.</rdfs:comment>
        <rdfs:label xml:lang="en">1938 FIFA World Cup</rdfs:label>
        <rdfs:label xml:lang="it">Campionato mondiale di calcio 1938</rdfs:label>
    </owl:NamedIndividual>
    


    <!-- http://www.semanticweb.org/2021/ontologies/calcio#WorldCup_1982 -->

    <owl:NamedIndividual rdf:about="http://www.semanticweb.org/2021/ontologies/calcio#WorldCup_1982">
        <rdf:type rdf:resource="http://www.semanticweb.org/2021/ontologies/calcio#trofeoDiNazione"/>
        <rdfs:comment xml:lang="it">Il campionato mondiale di calcio 1982 o Coppa del Mondo FIFA del 1982 (in spagnolo: Copa Mundial de Fútbol de 1982, in inglese: 1982 FIFA World Cup), noto anche come Spagna &apos;82, è stata la dodicesima edizione del campionato mondiale di calcio per squadre nazionali maggiori maschili organizzato dalla FIFA ogni quattro anni.</rdfs:comment>
        <rdfs:comment xml:lang="en">The 1982 FIFA World Cup was the 12th FIFA World Cup and was played in Spain between 13 June and 11 July 1982. The tournament was won by Italy, who defeated West Germany 3–1 in the final, held in the Santiago Bernabéu Stadium in the Spanish capital of Madrid. It was Italy&apos;s third World Cup title, but their first since 1938. The defending champions, Argentina, were eliminated in the second group round. Algeria, Cameroon, Honduras, Kuwait and New Zealand made their first appearances in the finals.</rdfs:comment>
        <rdfs:label xml:lang="en">1982 FIFA World Cup</rdfs:label>
        <rdfs:label xml:lang="it">Campionato mondiale di calcio 1982</rdfs:label>
    </owl:NamedIndividual>
    


    <!-- http://www.semanticweb.org/2021/ontologies/calcio#WorldCup_2006 -->

    <owl:NamedIndividual rdf:about="http://www.semanticweb.org/2021/ontologies/calcio#WorldCup_2006">
        <vintoDaNazionale rdf:resource="http://www.semanticweb.org/2021/ontologies/calcio#Italia"/>
        <rdfs:comment xml:lang="it">Il campionato mondiale di calcio 2006 o Coppa del Mondo FIFA del 2006 (in tedesco: Fußball-Weltmeisterschaft 2006, in inglese: 2006 FIFA World Cup), noto anche come Germania 2006, è stata la diciottesima edizione del campionato mondiale di calcio per squadre nazionali maggiori maschili organizzato dalla FIFA e la cui fase finale si disputò dal 9 giugno al 9 luglio 2006 in Germania.[1] Il motto dell&apos;evento era Il mondo a casa di amici (Die Welt zu Gast bei Freunden).</rdfs:comment>
        <rdfs:comment xml:lang="en">The 2006 FIFA World Cup was the 18th FIFA World Cup, the quadrennial international football world championship tournament. It was held from 9 June to 9 July 2006 in Germany, which won the right to host the event in July 2000. Teams representing 198 national football associations from all six populated continents participated in the qualification process which began in September 2003. Thirty-one teams qualified from this process, along with the host nation, Germany, for the finals tournament. It was the second time that Germany staged the competition, the first as a unified country (the other was in 1974 at the then-West Germany), and the tenth time that it was held in Europe.</rdfs:comment>
        <rdfs:label xml:lang="en">2006 FIFA World Cup</rdfs:label>
        <rdfs:label xml:lang="it">Campionato mondiale di calcio 2006</rdfs:label>
    </owl:NamedIndividual>
    


    <!-- http://www.semanticweb.org/2021/ontologies/calcio#WorldCup_2010 -->

    <owl:NamedIndividual rdf:about="http://www.semanticweb.org/2021/ontologies/calcio#WorldCup_2010">
        <rdf:type rdf:resource="http://www.semanticweb.org/2021/ontologies/calcio#trofeoDiNazione"/>
        <rdfs:comment xml:lang="it">Il campionato mondiale di calcio 2010 o Coppa del Mondo FIFA del 2010 (in afrikaans: FIFA Sokker-Wêreldbekertoernooi in 2010, in inglese: 2010 FIFA World Cup), noto anche come Sudafrica 2010, fu il 19º torneo mondiale per squadre nazionali maggiori maschili organizzato dalla FIFA, la cui fase finale si svolse in Sudafrica dall&apos;11 giugno all&apos;11 luglio 2010.</rdfs:comment>
        <rdfs:comment xml:lang="en">The 2010 FIFA World Cup was the 19th FIFA World Cup, the world championship for men&apos;s national association football teams. It took place in South Africa from 11 June to 11 July 2010. The bidding process for hosting the tournament finals was open only to African nations. In 2004, the international football federation, FIFA, selected South Africa over Egypt and Morocco to become the first African nation to host the finals.</rdfs:comment>
        <rdfs:label xml:lang="en">2010 FIFA World Cup</rdfs:label>
        <rdfs:label xml:lang="it">Campionato mondiale di calcio 2010</rdfs:label>
    </owl:NamedIndividual>
    


    <!-- http://www.semanticweb.org/2021/ontologies/calcio#Zlatan_Ibrahimović -->

    <owl:NamedIndividual rdf:about="http://www.semanticweb.org/2021/ontologies/calcio#Zlatan_Ibrahimović">
        <allenatoDa rdf:resource="http://www.semanticweb.org/2021/ontologies/calcio#Stefano_Pioli"/>
        <haRuolo rdf:resource="http://www.semanticweb.org/2021/ontologies/calcio#attaccanteMilan"/>
        <calciatoreHaValoreDiMercato rdf:datatype="http://www.w3.org/2001/XMLSchema#long">5000000</calciatoreHaValoreDiMercato>
        <dataUltimoTrasferimento rdf:datatype="http://www.w3.org/2001/XMLSchema#dateTime">2020-01-02T00:00:00</dataUltimoTrasferimento>
        <haEtà rdf:datatype="http://www.w3.org/2001/XMLSchema#integer">39</haEtà>
        <haNazionalità>Svezia</haNazionalità>
        <haNome>Zlatan Ibrahimović</haNome>
        <stipendioCorrente rdf:datatype="http://www.w3.org/2001/XMLSchema#long">6000000</stipendioCorrente>
        <rdfs:comment xml:lang="it">Zlatan Ibrahimović (AFI: [ˈzlatan ibraˈxiːmɔʋitɕ]; Malmö, 3 ottobre 1981) è un calciatore svedese, attaccante del Milan.</rdfs:comment>
        <rdfs:comment xml:lang="en">Zlatan Ibrahimović (Swedish pronunciation: [ˈslǎːtan ɪbraˈhǐːmovɪtɕ]; Bosnian pronunciation: [zlǎtan ibraxǐːmoʋitɕ]; born 3 October 1981) is a Swedish professional footballer who plays as a striker for Serie A club Milan. Ibrahimović is widely regarded as one of the best strikers of all time. He is one of the most decorated active footballers in the world,[a] having won 31 trophies in his career.[10] He has scored over 560 career goals, and has scored in each of the last four decades.</rdfs:comment>
        <rdfs:label xml:lang="en">Zlatan Ibrahimović</rdfs:label>
        <rdfs:label xml:lang="it">Zlatan Ibrahimović</rdfs:label>
    </owl:NamedIndividual>
    


    <!-- http://www.semanticweb.org/2021/ontologies/calcio#attaccanteBarcellona -->

    <owl:NamedIndividual rdf:about="http://www.semanticweb.org/2021/ontologies/calcio#attaccanteBarcellona">
        <rdf:type rdf:resource="http://www.semanticweb.org/2021/ontologies/calcio#Attaccante"/>
        <ruoloInSquadra rdf:resource="http://www.semanticweb.org/2021/ontologies/calcio#Barcellona"/>
        <rdfs:comment xml:lang="it">calciatore con ruolo attaccante nel Barcellona FC</rdfs:comment>
        <rdfs:comment xml:lang="en">soccer player with a forward role in Barcelona Football Club</rdfs:comment>
        <rdfs:label xml:lang="it">attaccante FC Barcellona</rdfs:label>
        <rdfs:label xml:lang="en">forward FC Barcellona</rdfs:label>
    </owl:NamedIndividual>
    


    <!-- http://www.semanticweb.org/2021/ontologies/calcio#attaccanteJuventus -->

    <owl:NamedIndividual rdf:about="http://www.semanticweb.org/2021/ontologies/calcio#attaccanteJuventus">
        <rdf:type rdf:resource="http://www.semanticweb.org/2021/ontologies/calcio#Attaccante"/>
        <rdfs:comment xml:lang="it">calciatore con ruolo attaccante nella Juventus FC</rdfs:comment>
        <rdfs:comment xml:lang="en">soccer player with a forward role in Juventus FC</rdfs:comment>
        <rdfs:label xml:lang="it">attaccante Juventus</rdfs:label>
        <rdfs:label xml:lang="en">forward Juventus</rdfs:label>
    </owl:NamedIndividual>
    


    <!-- http://www.semanticweb.org/2021/ontologies/calcio#attaccanteMilan -->

    <owl:NamedIndividual rdf:about="http://www.semanticweb.org/2021/ontologies/calcio#attaccanteMilan">
        <rdf:type rdf:resource="http://www.semanticweb.org/2021/ontologies/calcio#Attaccante"/>
        <ruoloInSquadra rdf:resource="http://www.semanticweb.org/2021/ontologies/calcio#ACMilan"/>
        <rdfs:comment xml:lang="it">calciatore con ruolo attaccante nell&apos; AC Milan</rdfs:comment>
        <rdfs:comment xml:lang="en">soccer player with a forward role in AC Milan</rdfs:comment>
        <rdfs:label xml:lang="it">attaccante AC Milan</rdfs:label>
        <rdfs:label xml:lang="en">forward AC Milan</rdfs:label>
    </owl:NamedIndividual>
    


    <!-- http://www.semanticweb.org/2021/ontologies/calcio#centrocampistaMilan -->

    <owl:NamedIndividual rdf:about="http://www.semanticweb.org/2021/ontologies/calcio#centrocampistaMilan">
        <rdf:type rdf:resource="http://www.semanticweb.org/2021/ontologies/calcio#RuoloCalciatore"/>
        <rdfs:comment xml:lang="it">calciatore con ruolo di centrocampista nell&apos;AC Milan</rdfs:comment>
        <rdfs:comment xml:lang="en">soccer player with a midfileder role in AC Milan</rdfs:comment>
        <rdfs:label xml:lang="it">centrocampista AC Milan</rdfs:label>
        <rdfs:label xml:lang="en">midfielder AC Milan</rdfs:label>
    </owl:NamedIndividual>
    


    <!-- http://www.semanticweb.org/2021/ontologies/calcio#difensoreMilan -->

    <owl:NamedIndividual rdf:about="http://www.semanticweb.org/2021/ontologies/calcio#difensoreMilan">
        <rdf:type rdf:resource="http://www.semanticweb.org/2021/ontologies/calcio#Difensore"/>
        <rdfs:comment xml:lang="it">calciatore con ruolo difensore nell&apos; AC Milan</rdfs:comment>
        <rdfs:comment xml:lang="en">soccer player with a defender role in AC Milan</rdfs:comment>
        <rdfs:label xml:lang="en">defender AC Milan</rdfs:label>
        <rdfs:label xml:lang="it">difensore AC Milan</rdfs:label>
    </owl:NamedIndividual>
    


    <!-- http://www.semanticweb.org/2021/ontologies/calcio#portiereMilan -->

    <owl:NamedIndividual rdf:about="http://www.semanticweb.org/2021/ontologies/calcio#portiereMilan">
        <rdf:type rdf:resource="http://www.semanticweb.org/2021/ontologies/calcio#Portiere"/>
        <rdfs:comment xml:lang="it">calciatore con ruolo portiere nell&apos;AC Milan</rdfs:comment>
        <rdfs:comment xml:lang="en">soccer player with a goolkeeper role in AC Milan</rdfs:comment>
        <rdfs:label xml:lang="en">goalkeeper AC Milan</rdfs:label>
        <rdfs:label xml:lang="it">portiere AC Milan</rdfs:label>
    </owl:NamedIndividual>
    


    <!-- http://www.semanticweb.org/2021/ontologies/calcio#2.Bundesliga -->

    <owl:NamedIndividual rdf:about="http://www.semanticweb.org/2021/ontologies/calcio#2.Bundesliga">
        <rdfs:comment xml:lang="it">La 2. Fußball-Bundesliga, spesso abbreviata in 2. Bundesliga o Zweite Liga (Seconda Lega), è la seconda divisione professionistica del campionato tedesco di calcio, categoria cadetta della Bundesliga. La stessa denominazione è usata per la seconda serie di altri sport come football americano, hockey su ghiaccio e basket.</rdfs:comment>
        <rdfs:comment xml:lang="en">The 2. Bundesliga is the second division of professional football in Germany. The 2. Bundesliga is ranked below the Bundesliga and above the 3. Liga in the German football league system. All of the 2. Bundesliga clubs qualify for the DFB-Pokal, the annual German Cup competition.</rdfs:comment>
        <rdfs:label xml:lang="en">2. Bundesliga</rdfs:label>
        <rdfs:label xml:lang="it">Zweite Bundesliga</rdfs:label>
    </owl:NamedIndividual>
    


    <!-- http://www.wikidata.org/entity/Q1543 -->

    <owl:NamedIndividual rdf:about="http://www.wikidata.org/entity/Q1543">
        <rdfs:comment xml:lang="en">(wikidata) italian association football club based in the city of Milan founded in 1899</rdfs:comment>
        <rdfs:comment xml:lang="it">(wikidata) società calcistica italiana</rdfs:comment>
        <rdfs:label xml:lang="en">A.C. Milan</rdfs:label>
        <rdfs:label xml:lang="it">AC Milan</rdfs:label>
    </owl:NamedIndividual>
    


    <!-- http://www.wikidata.org/entity/Q7156 -->

    <owl:NamedIndividual rdf:about="http://www.wikidata.org/entity/Q7156">
        <rdfs:comment xml:lang="en">(wikidata) association football club based in Barcelona, Spain</rdfs:comment>
        <rdfs:comment xml:lang="it">(wikidata) società polisportiva spagnola</rdfs:comment>
        <rdfs:label xml:lang="en">FC Barcelona</rdfs:label>
        <rdfs:label xml:lang="it">Futbol Club Barcelona</rdfs:label>
    </owl:NamedIndividual>
    


    <!-- 
    ///////////////////////////////////////////////////////////////////////////////////////
    //
    // General axioms
    //
    ///////////////////////////////////////////////////////////////////////////////////////
     -->

    <rdf:Description>
        <rdf:type rdf:resource="http://www.w3.org/2002/07/owl#AllDisjointClasses"/>
        <owl:members rdf:parseType="Collection">
            <rdf:Description rdf:about="http://www.semanticweb.org/2021/ontologies/calcio#legheFrancesi"/>
            <rdf:Description rdf:about="http://www.semanticweb.org/2021/ontologies/calcio#legheInglesi"/>
            <rdf:Description rdf:about="http://www.semanticweb.org/2021/ontologies/calcio#legheItaliane"/>
            <rdf:Description rdf:about="http://www.semanticweb.org/2021/ontologies/calcio#legheSpagnole"/>
            <rdf:Description rdf:about="http://www.semanticweb.org/2021/ontologies/calcio#legheTedesche"/>
        </owl:members>
    </rdf:Description>
    <rdf:Description>
        <rdf:type rdf:resource="http://www.w3.org/2002/07/owl#AllDisjointClasses"/>
        <owl:members rdf:parseType="Collection">
            <rdf:Description rdf:about="http://www.semanticweb.org/2021/ontologies/calcio#squadraFrancese"/>
            <rdf:Description rdf:about="http://www.semanticweb.org/2021/ontologies/calcio#squadraInglese"/>
            <rdf:Description rdf:about="http://www.semanticweb.org/2021/ontologies/calcio#squadraItaliana"/>
            <rdf:Description rdf:about="http://www.semanticweb.org/2021/ontologies/calcio#squadraSpagnola"/>
            <rdf:Description rdf:about="http://www.semanticweb.org/2021/ontologies/calcio#squadraTedesca"/>
        </owl:members>
    </rdf:Description>
    <rdf:Description>
        <rdf:type rdf:resource="http://www.w3.org/2002/07/owl#AllDisjointClasses"/>
        <owl:members rdf:parseType="Collection">
            <rdf:Description rdf:about="http://www.semanticweb.org/2021/ontologies/calcio#stadioMedio"/>
            <rdf:Description rdf:about="http://www.semanticweb.org/2021/ontologies/calcio#stadioPiccolo"/>
            <rdf:Description rdf:about="http://www.semanticweb.org/2021/ontologies/calcio#stadioTop"/>
        </owl:members>
    </rdf:Description>
    <rdf:Description>
        <rdf:type rdf:resource="http://www.w3.org/2002/07/owl#AllDifferent"/>
        <owl:distinctMembers rdf:parseType="Collection">
            <rdf:Description rdf:about="http://www.semanticweb.org/2021/ontologies/calcio#ACMilan"/>
            <rdf:Description rdf:about="http://www.semanticweb.org/2021/ontologies/calcio#Argentina"/>
            <rdf:Description rdf:about="http://www.semanticweb.org/2021/ontologies/calcio#AtleticoMadrid"/>
            <rdf:Description rdf:about="http://www.semanticweb.org/2021/ontologies/calcio#Barcellona"/>
            <rdf:Description rdf:about="http://www.semanticweb.org/2021/ontologies/calcio#BayernMonaco"/>
            <rdf:Description rdf:about="http://www.semanticweb.org/2021/ontologies/calcio#BorussiaDortmund"/>
            <rdf:Description rdf:about="http://www.semanticweb.org/2021/ontologies/calcio#Brasile"/>
            <rdf:Description rdf:about="http://www.semanticweb.org/2021/ontologies/calcio#Chelsea"/>
            <rdf:Description rdf:about="http://www.semanticweb.org/2021/ontologies/calcio#Francia"/>
            <rdf:Description rdf:about="http://www.semanticweb.org/2021/ontologies/calcio#Germania"/>
            <rdf:Description rdf:about="http://www.semanticweb.org/2021/ontologies/calcio#Inter"/>
            <rdf:Description rdf:about="http://www.semanticweb.org/2021/ontologies/calcio#Italia"/>
            <rdf:Description rdf:about="http://www.semanticweb.org/2021/ontologies/calcio#Juventus"/>
            <rdf:Description rdf:about="http://www.semanticweb.org/2021/ontologies/calcio#Lille"/>
            <rdf:Description rdf:about="http://www.semanticweb.org/2021/ontologies/calcio#Lione"/>
            <rdf:Description rdf:about="http://www.semanticweb.org/2021/ontologies/calcio#Liverpool"/>
            <rdf:Description rdf:about="http://www.semanticweb.org/2021/ontologies/calcio#ManchesterCity"/>
            <rdf:Description rdf:about="http://www.semanticweb.org/2021/ontologies/calcio#ManchesterUnited"/>
            <rdf:Description rdf:about="http://www.semanticweb.org/2021/ontologies/calcio#Marsiglia"/>
            <rdf:Description rdf:about="http://www.semanticweb.org/2021/ontologies/calcio#Portogallo"/>
            <rdf:Description rdf:about="http://www.semanticweb.org/2021/ontologies/calcio#RBLeipzig"/>
            <rdf:Description rdf:about="http://www.semanticweb.org/2021/ontologies/calcio#RealMadrid"/>
            <rdf:Description rdf:about="http://www.semanticweb.org/2021/ontologies/calcio#Roma"/>
            <rdf:Description rdf:about="http://www.semanticweb.org/2021/ontologies/calcio#Spagna"/>
            <rdf:Description rdf:about="http://www.semanticweb.org/2021/ontologies/calcio#Villareal"/>
        </owl:distinctMembers>
    </rdf:Description>
    <rdf:Description>
        <rdf:type rdf:resource="http://www.w3.org/2002/07/owl#AllDifferent"/>
        <owl:distinctMembers rdf:parseType="Collection">
            <rdf:Description rdf:about="http://www.semanticweb.org/2021/ontologies/calcio#Andrea_Pirlo"/>
            <rdf:Description rdf:about="http://www.semanticweb.org/2021/ontologies/calcio#Antonio_Conte"/>
            <rdf:Description rdf:about="http://www.semanticweb.org/2021/ontologies/calcio#Ronald_Koeman"/>
            <rdf:Description rdf:about="http://www.semanticweb.org/2021/ontologies/calcio#Stefano_Pioli"/>
        </owl:distinctMembers>
    </rdf:Description>
    <rdf:Description>
        <rdf:type rdf:resource="http://www.w3.org/2002/07/owl#AllDifferent"/>
        <owl:distinctMembers rdf:parseType="Collection">
            <rdf:Description rdf:about="http://www.semanticweb.org/2021/ontologies/calcio#Anfield"/>
            <rdf:Description rdf:about="http://www.semanticweb.org/2021/ontologies/calcio#Camp_Nou"/>
            <rdf:Description rdf:about="http://www.semanticweb.org/2021/ontologies/calcio#Le_Parc_des_Princes"/>
            <rdf:Description rdf:about="http://www.semanticweb.org/2021/ontologies/calcio#Old_Trafford"/>
            <rdf:Description rdf:about="http://www.semanticweb.org/2021/ontologies/calcio#San_Siro"/>
            <rdf:Description rdf:about="http://www.semanticweb.org/2021/ontologies/calcio#Santiago_Bernabéu_Stadium"/>
        </owl:distinctMembers>
    </rdf:Description>
    <rdf:Description>
        <rdf:type rdf:resource="http://www.w3.org/2002/07/owl#AllDifferent"/>
        <owl:distinctMembers rdf:parseType="Collection">
            <rdf:Description rdf:about="http://www.semanticweb.org/2021/ontologies/calcio#Bundesliga"/>
            <rdf:Description rdf:about="http://www.semanticweb.org/2021/ontologies/calcio#Championship"/>
            <rdf:Description rdf:about="http://www.semanticweb.org/2021/ontologies/calcio#DFB-Pokal"/>
            <rdf:Description rdf:about="http://www.semanticweb.org/2021/ontologies/calcio#LaLiga"/>
            <rdf:Description rdf:about="http://www.semanticweb.org/2021/ontologies/calcio#Ligue1"/>
            <rdf:Description rdf:about="http://www.semanticweb.org/2021/ontologies/calcio#Ligue2"/>
            <rdf:Description rdf:about="http://www.semanticweb.org/2021/ontologies/calcio#PremierLeague"/>
            <rdf:Description rdf:about="http://www.semanticweb.org/2021/ontologies/calcio#SegundaDivisión"/>
            <rdf:Description rdf:about="http://www.semanticweb.org/2021/ontologies/calcio#SerieA"/>
            <rdf:Description rdf:about="http://www.semanticweb.org/2021/ontologies/calcio#SerieB"/>
            <rdf:Description rdf:about="http://www.semanticweb.org/2021/ontologies/calcio#SerieC"/>
            <rdf:Description rdf:about="http://www.semanticweb.org/2021/ontologies/calcio#2.Bundesliga"/>
        </owl:distinctMembers>
    </rdf:Description>
    <rdf:Description>
        <rdf:type rdf:resource="http://www.w3.org/2002/07/owl#AllDifferent"/>
        <owl:distinctMembers rdf:parseType="Collection">
            <rdf:Description rdf:about="http://www.semanticweb.org/2021/ontologies/calcio#ChampionsLeague_2003"/>
            <rdf:Description rdf:about="http://www.semanticweb.org/2021/ontologies/calcio#ChampionsLeague_2007"/>
            <rdf:Description rdf:about="http://www.semanticweb.org/2021/ontologies/calcio#ChampionsLeague_63"/>
            <rdf:Description rdf:about="http://www.semanticweb.org/2021/ontologies/calcio#ChampionsLeague_69"/>
            <rdf:Description rdf:about="http://www.semanticweb.org/2021/ontologies/calcio#ChampionsLeague_89"/>
            <rdf:Description rdf:about="http://www.semanticweb.org/2021/ontologies/calcio#ChampionsLeague_90"/>
            <rdf:Description rdf:about="http://www.semanticweb.org/2021/ontologies/calcio#ChampionsLeague_94"/>
            <rdf:Description rdf:about="http://www.semanticweb.org/2021/ontologies/calcio#CopaDelRey"/>
            <rdf:Description rdf:about="http://www.semanticweb.org/2021/ontologies/calcio#CoppaItalia"/>
            <rdf:Description rdf:about="http://www.semanticweb.org/2021/ontologies/calcio#CoupeDeFrance"/>
            <rdf:Description rdf:about="http://www.semanticweb.org/2021/ontologies/calcio#DFB-Pokal"/>
            <rdf:Description rdf:about="http://www.semanticweb.org/2021/ontologies/calcio#Euro_2008"/>
            <rdf:Description rdf:about="http://www.semanticweb.org/2021/ontologies/calcio#EuropaLeague"/>
            <rdf:Description rdf:about="http://www.semanticweb.org/2021/ontologies/calcio#FACup"/>
            <rdf:Description rdf:about="http://www.semanticweb.org/2021/ontologies/calcio#SuperCup"/>
            <rdf:Description rdf:about="http://www.semanticweb.org/2021/ontologies/calcio#The_UEFA_European_Football_Championship"/>
            <rdf:Description rdf:about="http://www.semanticweb.org/2021/ontologies/calcio#WorldCup_1934"/>
            <rdf:Description rdf:about="http://www.semanticweb.org/2021/ontologies/calcio#WorldCup_1938"/>
            <rdf:Description rdf:about="http://www.semanticweb.org/2021/ontologies/calcio#WorldCup_1982"/>
            <rdf:Description rdf:about="http://www.semanticweb.org/2021/ontologies/calcio#WorldCup_2006"/>
            <rdf:Description rdf:about="http://www.semanticweb.org/2021/ontologies/calcio#WorldCup_2010"/>
        </owl:distinctMembers>
    </rdf:Description>
    <rdf:Description>
        <rdf:type rdf:resource="http://www.w3.org/2002/07/owl#AllDifferent"/>
        <owl:distinctMembers rdf:parseType="Collection">
            <rdf:Description rdf:about="http://www.semanticweb.org/2021/ontologies/calcio#Daniele_Orsato"/>
            <rdf:Description rdf:about="http://www.semanticweb.org/2021/ontologies/calcio#Massimiliano_Irrati"/>
            <rdf:Description rdf:about="http://www.semanticweb.org/2021/ontologies/calcio#Rosario_Abisso"/>
        </owl:distinctMembers>
    </rdf:Description>
    <rdf:Description>
        <rdf:type rdf:resource="http://www.w3.org/2002/07/owl#AllDifferent"/>
        <owl:distinctMembers rdf:parseType="Collection">
            <rdf:Description rdf:about="http://www.semanticweb.org/2021/ontologies/calcio#attaccanteBarcellona"/>
            <rdf:Description rdf:about="http://www.semanticweb.org/2021/ontologies/calcio#attaccanteJuventus"/>
            <rdf:Description rdf:about="http://www.semanticweb.org/2021/ontologies/calcio#attaccanteMilan"/>
            <rdf:Description rdf:about="http://www.semanticweb.org/2021/ontologies/calcio#centrocampistaMilan"/>
        </owl:distinctMembers>
    </rdf:Description>
    


    <!-- 
    ///////////////////////////////////////////////////////////////////////////////////////
    //
    // Rules
    //
    ///////////////////////////////////////////////////////////////////////////////////////
     -->

    <rdf:Description rdf:about="http://www.semanticweb.org/2021/ontologies/calcio#a">
        <rdf:type rdf:resource="http://www.w3.org/2003/11/swrl#Variable"/>
    </rdf:Description>
    <rdf:Description rdf:about="http://www.semanticweb.org/2021/ontologies/calcio#d">
        <rdf:type rdf:resource="http://www.w3.org/2003/11/swrl#Variable"/>
    </rdf:Description>
    <rdf:Description rdf:about="http://www.semanticweb.org/2021/ontologies/calcio#c">
        <rdf:type rdf:resource="http://www.w3.org/2003/11/swrl#Variable"/>
    </rdf:Description>
    <rdf:Description rdf:about="http://www.semanticweb.org/2021/ontologies/calcio#l">
        <rdf:type rdf:resource="http://www.w3.org/2003/11/swrl#Variable"/>
    </rdf:Description>
    <rdf:Description rdf:about="http://www.semanticweb.org/2021/ontologies/calcio#m">
        <rdf:type rdf:resource="http://www.w3.org/2003/11/swrl#Variable"/>
    </rdf:Description>
    <rdf:Description rdf:about="http://www.semanticweb.org/2021/ontologies/calcio#s">
        <rdf:type rdf:resource="http://www.w3.org/2003/11/swrl#Variable"/>
    </rdf:Description>
    <rdf:Description rdf:about="http://www.semanticweb.org/2021/ontologies/calcio#t">
        <rdf:type rdf:resource="http://www.w3.org/2003/11/swrl#Variable"/>
    </rdf:Description>
    <rdf:Description rdf:about="http://www.semanticweb.org/2021/ontologies/calcio#n">
        <rdf:type rdf:resource="http://www.w3.org/2003/11/swrl#Variable"/>
    </rdf:Description>
    <rdf:Description>
        <swrla:isRuleEnabled rdf:datatype="http://www.w3.org/2001/XMLSchema#boolean">true</swrla:isRuleEnabled>
        <rdfs:comment rdf:datatype="http://www.w3.org/2001/XMLSchema#string">Asserisce la conoscena tra un dirigente e un calciatore sulla base della relazione &quot;collegaDi&quot;  tra lo stesso dirigente e l&apos;allenatore di tale calciatore.</rdfs:comment>
        <rdfs:label rdf:datatype="http://www.w3.org/2001/XMLSchema#string">S3</rdfs:label>
        <rdf:type rdf:resource="http://www.w3.org/2003/11/swrl#Imp"/>
        <swrl:body>
            <rdf:Description>
                <rdf:type rdf:resource="http://www.w3.org/2003/11/swrl#AtomList"/>
                <rdf:first>
                    <rdf:Description>
                        <rdf:type rdf:resource="http://www.w3.org/2003/11/swrl#ClassAtom"/>
                        <swrl:classPredicate rdf:resource="http://www.semanticweb.org/2021/ontologies/calcio#Allenatore"/>
                        <swrl:argument1 rdf:resource="http://www.semanticweb.org/2021/ontologies/calcio#a"/>
                    </rdf:Description>
                </rdf:first>
                <rdf:rest>
                    <rdf:Description>
                        <rdf:type rdf:resource="http://www.w3.org/2003/11/swrl#AtomList"/>
                        <rdf:first>
                            <rdf:Description>
                                <rdf:type rdf:resource="http://www.w3.org/2003/11/swrl#ClassAtom"/>
                                <swrl:classPredicate rdf:resource="http://www.semanticweb.org/2021/ontologies/calcio#Dirigente"/>
                                <swrl:argument1 rdf:resource="http://www.semanticweb.org/2021/ontologies/calcio#d"/>
                            </rdf:Description>
                        </rdf:first>
                        <rdf:rest>
                            <rdf:Description>
                                <rdf:type rdf:resource="http://www.w3.org/2003/11/swrl#AtomList"/>
                                <rdf:first>
                                    <rdf:Description>
                                        <rdf:type rdf:resource="http://www.w3.org/2003/11/swrl#IndividualPropertyAtom"/>
                                        <swrl:propertyPredicate rdf:resource="http://www.semanticweb.org/2021/ontologies/calcio#collegaDi"/>
                                        <swrl:argument1 rdf:resource="http://www.semanticweb.org/2021/ontologies/calcio#a"/>
                                        <swrl:argument2 rdf:resource="http://www.semanticweb.org/2021/ontologies/calcio#d"/>
                                    </rdf:Description>
                                </rdf:first>
                                <rdf:rest>
                                    <rdf:Description>
                                        <rdf:type rdf:resource="http://www.w3.org/2003/11/swrl#AtomList"/>
                                        <rdf:first>
                                            <rdf:Description>
                                                <rdf:type rdf:resource="http://www.w3.org/2003/11/swrl#ClassAtom"/>
                                                <swrl:classPredicate rdf:resource="http://www.semanticweb.org/2021/ontologies/calcio#Calciatore"/>
                                                <swrl:argument1 rdf:resource="http://www.semanticweb.org/2021/ontologies/calcio#c"/>
                                            </rdf:Description>
                                        </rdf:first>
                                        <rdf:rest>
                                            <rdf:Description>
                                                <rdf:type rdf:resource="http://www.w3.org/2003/11/swrl#AtomList"/>
                                                <rdf:first>
                                                    <rdf:Description>
                                                        <rdf:type rdf:resource="http://www.w3.org/2003/11/swrl#IndividualPropertyAtom"/>
                                                        <swrl:propertyPredicate rdf:resource="http://www.semanticweb.org/2021/ontologies/calcio#allenatoDa"/>
                                                        <swrl:argument1 rdf:resource="http://www.semanticweb.org/2021/ontologies/calcio#c"/>
                                                        <swrl:argument2 rdf:resource="http://www.semanticweb.org/2021/ontologies/calcio#a"/>
                                                    </rdf:Description>
                                                </rdf:first>
                                                <rdf:rest rdf:resource="http://www.w3.org/1999/02/22-rdf-syntax-ns#nil"/>
                                            </rdf:Description>
                                        </rdf:rest>
                                    </rdf:Description>
                                </rdf:rest>
                            </rdf:Description>
                        </rdf:rest>
                    </rdf:Description>
                </rdf:rest>
            </rdf:Description>
        </swrl:body>
        <swrl:head>
            <rdf:Description>
                <rdf:type rdf:resource="http://www.w3.org/2003/11/swrl#AtomList"/>
                <rdf:first>
                    <rdf:Description>
                        <rdf:type rdf:resource="http://www.w3.org/2003/11/swrl#IndividualPropertyAtom"/>
                        <swrl:propertyPredicate rdf:resource="http://xmlns.com/foaf/0.1/knows"/>
                        <swrl:argument1 rdf:resource="http://www.semanticweb.org/2021/ontologies/calcio#d"/>
                        <swrl:argument2 rdf:resource="http://www.semanticweb.org/2021/ontologies/calcio#c"/>
                    </rdf:Description>
                </rdf:first>
                <rdf:rest rdf:resource="http://www.w3.org/1999/02/22-rdf-syntax-ns#nil"/>
            </rdf:Description>
        </swrl:head>
    </rdf:Description>
    <rdf:Description>
        <swrla:isRuleEnabled rdf:datatype="http://www.w3.org/2001/XMLSchema#boolean">true</swrla:isRuleEnabled>
        <rdfs:comment rdf:datatype="http://www.w3.org/2001/XMLSchema#string">Allinea gli individui della classe enumerata legheItaliane con i rispettivi individui di DBpedia.</rdfs:comment>
        <rdfs:label rdf:datatype="http://www.w3.org/2001/XMLSchema#string">S2</rdfs:label>
        <rdf:type rdf:resource="http://www.w3.org/2003/11/swrl#Imp"/>
        <swrl:body>
            <rdf:Description>
                <rdf:type rdf:resource="http://www.w3.org/2003/11/swrl#AtomList"/>
                <rdf:first>
                    <rdf:Description>
                        <rdf:type rdf:resource="http://www.w3.org/2003/11/swrl#ClassAtom"/>
                        <swrl:classPredicate rdf:resource="http://www.semanticweb.org/2021/ontologies/calcio#legheItaliane"/>
                        <swrl:argument1 rdf:resource="http://www.semanticweb.org/2021/ontologies/calcio#l"/>
                    </rdf:Description>
                </rdf:first>
                <rdf:rest rdf:resource="http://www.w3.org/1999/02/22-rdf-syntax-ns#nil"/>
            </rdf:Description>
        </swrl:body>
        <swrl:head>
            <rdf:Description>
                <rdf:type rdf:resource="http://www.w3.org/2003/11/swrl#AtomList"/>
                <rdf:first>
                    <rdf:Description>
                        <rdf:type rdf:resource="http://www.w3.org/2003/11/swrl#SameIndividualAtom"/>
                        <swrl:argument1 rdf:resource="http://www.semanticweb.org/2021/ontologies/calcio#SerieA"/>
                        <swrl:argument2 rdf:resource="http://dbpedia.org/resource/Serie_A"/>
                    </rdf:Description>
                </rdf:first>
                <rdf:rest>
                    <rdf:Description>
                        <rdf:type rdf:resource="http://www.w3.org/2003/11/swrl#AtomList"/>
                        <rdf:first>
                            <rdf:Description>
                                <rdf:type rdf:resource="http://www.w3.org/2003/11/swrl#SameIndividualAtom"/>
                                <swrl:argument1 rdf:resource="http://www.semanticweb.org/2021/ontologies/calcio#SerieB"/>
                                <swrl:argument2 rdf:resource="http://dbpedia.org/resource/Serie_B"/>
                            </rdf:Description>
                        </rdf:first>
                        <rdf:rest>
                            <rdf:Description>
                                <rdf:type rdf:resource="http://www.w3.org/2003/11/swrl#AtomList"/>
                                <rdf:first>
                                    <rdf:Description>
                                        <rdf:type rdf:resource="http://www.w3.org/2003/11/swrl#SameIndividualAtom"/>
                                        <swrl:argument1 rdf:resource="http://www.semanticweb.org/2021/ontologies/calcio#SerieC"/>
                                        <swrl:argument2 rdf:resource="http://dbpedia.org/resource/Serie_C"/>
                                    </rdf:Description>
                                </rdf:first>
                                <rdf:rest rdf:resource="http://www.w3.org/1999/02/22-rdf-syntax-ns#nil"/>
                            </rdf:Description>
                        </rdf:rest>
                    </rdf:Description>
                </rdf:rest>
            </rdf:Description>
        </swrl:head>
    </rdf:Description>
    <rdf:Description>
        <swrla:isRuleEnabled rdf:datatype="http://www.w3.org/2001/XMLSchema#boolean">true</swrla:isRuleEnabled>
        <rdfs:comment rdf:datatype="http://www.w3.org/2001/XMLSchema#string">Asserisce un allenatore di club famoso se l&apos;allenatore in questione allena una squadra appartenente a una lega &quot;TOP&quot;.</rdfs:comment>
        <rdfs:label rdf:datatype="http://www.w3.org/2001/XMLSchema#string">S1</rdfs:label>
        <rdf:type rdf:resource="http://www.w3.org/2003/11/swrl#Imp"/>
        <swrl:body>
            <rdf:Description>
                <rdf:type rdf:resource="http://www.w3.org/2003/11/swrl#AtomList"/>
                <rdf:first>
                    <rdf:Description>
                        <rdf:type rdf:resource="http://www.w3.org/2003/11/swrl#IndividualPropertyAtom"/>
                        <swrl:propertyPredicate rdf:resource="http://www.semanticweb.org/2021/ontologies/calcio#allenaSquadra"/>
                        <swrl:argument1 rdf:resource="http://www.semanticweb.org/2021/ontologies/calcio#a"/>
                        <swrl:argument2 rdf:resource="http://www.semanticweb.org/2021/ontologies/calcio#m"/>
                    </rdf:Description>
                </rdf:first>
                <rdf:rest>
                    <rdf:Description>
                        <rdf:type rdf:resource="http://www.w3.org/2003/11/swrl#AtomList"/>
                        <rdf:first>
                            <rdf:Description>
                                <rdf:type rdf:resource="http://www.w3.org/2003/11/swrl#IndividualPropertyAtom"/>
                                <swrl:propertyPredicate rdf:resource="http://www.semanticweb.org/2021/ontologies/calcio#appartieneALega"/>
                                <swrl:argument1 rdf:resource="http://www.semanticweb.org/2021/ontologies/calcio#m"/>
                                <swrl:argument2 rdf:resource="http://www.semanticweb.org/2021/ontologies/calcio#s"/>
                            </rdf:Description>
                        </rdf:first>
                        <rdf:rest>
                            <rdf:Description>
                                <rdf:type rdf:resource="http://www.w3.org/2003/11/swrl#AtomList"/>
                                <rdf:first>
                                    <rdf:Description>
                                        <rdf:type rdf:resource="http://www.w3.org/2003/11/swrl#ClassAtom"/>
                                        <swrl:classPredicate rdf:resource="http://www.semanticweb.org/2021/ontologies/calcio#topLega"/>
                                        <swrl:argument1 rdf:resource="http://www.semanticweb.org/2021/ontologies/calcio#s"/>
                                    </rdf:Description>
                                </rdf:first>
                                <rdf:rest rdf:resource="http://www.w3.org/1999/02/22-rdf-syntax-ns#nil"/>
                            </rdf:Description>
                        </rdf:rest>
                    </rdf:Description>
                </rdf:rest>
            </rdf:Description>
        </swrl:body>
        <swrl:head>
            <rdf:Description>
                <rdf:type rdf:resource="http://www.w3.org/2003/11/swrl#AtomList"/>
                <rdf:first>
                    <rdf:Description>
                        <rdf:type rdf:resource="http://www.w3.org/2003/11/swrl#ClassAtom"/>
                        <swrl:classPredicate rdf:resource="http://www.semanticweb.org/2021/ontologies/calcio#allenatoreDiClubFamoso"/>
                        <swrl:argument1 rdf:resource="http://www.semanticweb.org/2021/ontologies/calcio#a"/>
                    </rdf:Description>
                </rdf:first>
                <rdf:rest rdf:resource="http://www.w3.org/1999/02/22-rdf-syntax-ns#nil"/>
            </rdf:Description>
        </swrl:head>
    </rdf:Description>
    <rdf:Description>
        <swrla:isRuleEnabled rdf:datatype="http://www.w3.org/2001/XMLSchema#boolean">true</swrla:isRuleEnabled>
        <rdfs:comment rdf:datatype="http://www.w3.org/2001/XMLSchema#string">Asserice che un calciatore risulta essere &quot;molto pagato&quot; in base al suo stipendio corrente.</rdfs:comment>
        <rdfs:label rdf:datatype="http://www.w3.org/2001/XMLSchema#string">S4</rdfs:label>
        <rdf:type rdf:resource="http://www.w3.org/2003/11/swrl#Imp"/>
        <swrl:body>
            <rdf:Description>
                <rdf:type rdf:resource="http://www.w3.org/2003/11/swrl#AtomList"/>
                <rdf:first>
                    <rdf:Description>
                        <rdf:type rdf:resource="http://www.w3.org/2003/11/swrl#DatavaluedPropertyAtom"/>
                        <swrl:propertyPredicate rdf:resource="http://www.semanticweb.org/2021/ontologies/calcio#stipendioCorrente"/>
                        <swrl:argument1 rdf:resource="http://www.semanticweb.org/2021/ontologies/calcio#c"/>
                        <swrl:argument2 rdf:resource="http://www.semanticweb.org/2021/ontologies/calcio#s"/>
                    </rdf:Description>
                </rdf:first>
                <rdf:rest>
                    <rdf:Description>
                        <rdf:type rdf:resource="http://www.w3.org/2003/11/swrl#AtomList"/>
                        <rdf:first>
                            <rdf:Description>
                                <rdf:type rdf:resource="http://www.w3.org/2003/11/swrl#BuiltinAtom"/>
                                <swrl:builtin rdf:resource="http://www.w3.org/2003/11/swrlb#greaterThan"/>
                                <swrl:arguments>
                                    <rdf:Description>
                                        <rdf:type rdf:resource="http://www.w3.org/1999/02/22-rdf-syntax-ns#List"/>
                                        <rdf:first rdf:resource="http://www.semanticweb.org/2021/ontologies/calcio#s"/>
                                        <rdf:rest>
                                            <rdf:Description>
                                                <rdf:type rdf:resource="http://www.w3.org/1999/02/22-rdf-syntax-ns#List"/>
                                                <rdf:first rdf:datatype="http://www.w3.org/2001/XMLSchema#integer">5000000</rdf:first>
                                                <rdf:rest rdf:resource="http://www.w3.org/1999/02/22-rdf-syntax-ns#nil"/>
                                            </rdf:Description>
                                        </rdf:rest>
                                    </rdf:Description>
                                </swrl:arguments>
                            </rdf:Description>
                        </rdf:first>
                        <rdf:rest rdf:resource="http://www.w3.org/1999/02/22-rdf-syntax-ns#nil"/>
                    </rdf:Description>
                </rdf:rest>
            </rdf:Description>
        </swrl:body>
        <swrl:head>
            <rdf:Description>
                <rdf:type rdf:resource="http://www.w3.org/2003/11/swrl#AtomList"/>
                <rdf:first>
                    <rdf:Description>
                        <rdf:type rdf:resource="http://www.w3.org/2003/11/swrl#ClassAtom"/>
                        <swrl:classPredicate rdf:resource="http://www.semanticweb.org/2021/ontologies/calcio#calciatoreMoltoPagato"/>
                        <swrl:argument1 rdf:resource="http://www.semanticweb.org/2021/ontologies/calcio#c"/>
                    </rdf:Description>
                </rdf:first>
                <rdf:rest rdf:resource="http://www.w3.org/1999/02/22-rdf-syntax-ns#nil"/>
            </rdf:Description>
        </swrl:head>
    </rdf:Description>
    <rdf:Description>
        <swrla:isRuleEnabled rdf:datatype="http://www.w3.org/2001/XMLSchema#boolean">true</swrla:isRuleEnabled>
        <rdfs:comment rdf:datatype="http://www.w3.org/2001/XMLSchema#string">Asserisce se un trofeo può essere categorizzato come un trofeo UEFA.</rdfs:comment>
        <rdfs:label rdf:datatype="http://www.w3.org/2001/XMLSchema#string">S5</rdfs:label>
        <rdf:type rdf:resource="http://www.w3.org/2003/11/swrl#Imp"/>
        <swrl:body>
            <rdf:Description>
                <rdf:type rdf:resource="http://www.w3.org/2003/11/swrl#AtomList"/>
                <rdf:first>
                    <rdf:Description>
                        <rdf:type rdf:resource="http://www.w3.org/2003/11/swrl#DatavaluedPropertyAtom"/>
                        <swrl:propertyPredicate rdf:resource="http://www.semanticweb.org/2021/ontologies/calcio#trofeoHaNome"/>
                        <swrl:argument1 rdf:resource="http://www.semanticweb.org/2021/ontologies/calcio#t"/>
                        <swrl:argument2 rdf:resource="http://www.semanticweb.org/2021/ontologies/calcio#n"/>
                    </rdf:Description>
                </rdf:first>
                <rdf:rest>
                    <rdf:Description>
                        <rdf:type rdf:resource="http://www.w3.org/2003/11/swrl#AtomList"/>
                        <rdf:first>
                            <rdf:Description>
                                <rdf:type rdf:resource="http://www.w3.org/2003/11/swrl#BuiltinAtom"/>
                                <swrl:builtin rdf:resource="http://www.w3.org/2003/11/swrlb#containsIgnoreCase"/>
                                <swrl:arguments>
                                    <rdf:Description>
                                        <rdf:type rdf:resource="http://www.w3.org/1999/02/22-rdf-syntax-ns#List"/>
                                        <rdf:first rdf:resource="http://www.semanticweb.org/2021/ontologies/calcio#n"/>
                                        <rdf:rest>
                                            <rdf:Description>
                                                <rdf:type rdf:resource="http://www.w3.org/1999/02/22-rdf-syntax-ns#List"/>
                                                <rdf:first rdf:datatype="http://www.w3.org/2001/XMLSchema#string">UEFA</rdf:first>
                                                <rdf:rest rdf:resource="http://www.w3.org/1999/02/22-rdf-syntax-ns#nil"/>
                                            </rdf:Description>
                                        </rdf:rest>
                                    </rdf:Description>
                                </swrl:arguments>
                            </rdf:Description>
                        </rdf:first>
                        <rdf:rest rdf:resource="http://www.w3.org/1999/02/22-rdf-syntax-ns#nil"/>
                    </rdf:Description>
                </rdf:rest>
            </rdf:Description>
        </swrl:body>
        <swrl:head>
            <rdf:Description>
                <rdf:type rdf:resource="http://www.w3.org/2003/11/swrl#AtomList"/>
                <rdf:first>
                    <rdf:Description>
                        <rdf:type rdf:resource="http://www.w3.org/2003/11/swrl#ClassAtom"/>
                        <swrl:classPredicate rdf:resource="http://www.semanticweb.org/2021/ontologies/calcio#trofeoUEFA"/>
                        <swrl:argument1 rdf:resource="http://www.semanticweb.org/2021/ontologies/calcio#t"/>
                    </rdf:Description>
                </rdf:first>
                <rdf:rest rdf:resource="http://www.w3.org/1999/02/22-rdf-syntax-ns#nil"/>
            </rdf:Description>
        </swrl:head>
    </rdf:Description>
</rdf:RDF>



<!-- Generated by the OWL API (version 4.5.9.2019-02-01T07:24:44Z) https://github.com/owlcs/owlapi -->

